pico-invsubtyping-limitedvpa/ReadonlyReachability.v
@@ -1,0 +1,4672 @@
+Require Import Syntax Notations Helpers Typing Subtyping Bigstep ViewpointAdaptation Properties DeepImmutability.
+Require Import List.
+Import ListNotations.
+Require Import String.
+From RecordUpdate Require Import RecordUpdate.
+
+Theorem readonly_pico_field_write:
+    forall CT sΓ rΓ h stmt rΓ' h' sΓ' l C vals vals' f qt readonlyx anyf rhs anyrq,
+      stmt = (SFldWrite readonlyx anyf rhs)-> 
+      static_getType sΓ readonlyx = Some qt ->
+      (sqtype qt) = Rd ->
+      wf_r_config CT sΓ rΓ h ->
+      stmt_typing CT sΓ stmt sΓ' -> 
+      eval_stmt OK CT rΓ h stmt OK rΓ' h' -> 
+      runtime_getVal rΓ readonlyx = Some (Iot l)  ->
+      runtime_getObj h l = Some (mkObj (mkruntime_type anyrq C) vals) ->
+      runtime_getObj h' l = Some (mkObj (mkruntime_type anyrq C) vals') ->
+      sf_assignability_rel CT C f Final \/ sf_assignability_rel CT C f RDA ->
+      nth_error vals f = nth_error vals' f.
+Proof.
+intros CT sΓ rΓ h stmt rΓ' h' sΓ' l C vals vals' f qt readonlyx anyf rhs anyrq.
+intros Hstmt_form Hreceivermut Hstatic_type Hwf_config Htyping Heval Hruntime_val Hobj_before Hobj_after Hassign_rel.
+
+(* Subst the statement form *)
+subst stmt.
+
+(* Invert the evaluation to get heap update details *)
+inversion Heval; subst.
+
+(* Invert typing to get field write constraints *)
+inversion Htyping; subst.
+
+unfold wf_r_config in Hwf_config.
+  destruct Hwf_config as [_[_[Hrenv [_ [_ Htypable]]]]].
+  assert (Hreadonly_dom : readonlyx < dom sΓ').
+  {
+    apply static_getType_dom in Hreceivermut.
+    exact Hreceivermut.
+  }
+  rewrite Hruntime_val in H2.
+  inversion H2.
+  subst l.
+  unfold wf_renv in Hrenv.
+  destruct Hrenv as [_ [Hreceiver _]].
+  destruct Hreceiver as [iot [Hget_iot Hiot_dom]].
+  assert (HOutterReceiverMutability: exists qcontext, r_muttype h iot = Some qcontext).
+  {
+    eapply receiver_mutability_exists_from_bound; eauto.
+  }
+  destruct HOutterReceiverMutability as [qcontext Hqcontext].
+  (* Apply correspondence to get wf_r_typable *)
+  specialize (Htypable iot qcontext Hget_iot Hqcontext readonlyx Hreadonly_dom qt Hreceivermut).
+  rewrite Hruntime_val in Htypable.
+  unfold wf_r_typable in Htypable.
+  unfold r_type in Htypable.
+  rewrite H3 in Htypable.
+  destruct Htypable as [base qualifier].
+  rewrite H3 in Hobj_before.
+  inversion Hobj_before.
+  rewrite H0 in base.
+  simpl in base.
+
+(* Use the fact that Final/RDA fields are protected from modification *)
+destruct Hassign_rel as [Hfinal | Hrda].
+-  
+  rewrite Hreceivermut in H6.
+  inversion H6.
+  subst Tx.
+  rewrite Hstatic_type in H15.
+  unfold vpa_assignability in H15.
+  destruct a eqn: Haeqn; try easy.
+  assert (Hneq: anyf <> f).
+  {
+    intro Heq.
+    subst anyf.
+    unfold sf_assignability_rel in H13, Hfinal.
+    destruct H13 as [fdef_assign [Hlookup_assign Hassign_assign]].
+    destruct Hfinal as [fdef_final [Hlookup_final Hassign_final]].
+    assert (fdef_final = fdef_assign).
+    {
+      eapply field_lookup_deterministic_rel; eauto.
+      eapply field_inheritance_subtyping; eauto.
+    }
+    subst fdef_final.
+    rewrite Hassign_final in Hassign_assign.
+    discriminate.
+  }
+  injection Hobj_before as Hvals_eq.
+  unfold update_field in Hobj_after.
+  rewrite H3 in Hobj_after.
+  simpl in Hobj_after.
+  unfold update_field in Hobj_after.
+  simpl in Hobj_after.
+  assert (Hdom: loc_x < dom h).
+  {
+    apply runtime_getObj_dom in H3.
+    exact H3.
+  }
+  rewrite runtime_getObj_update_same in Hobj_after; auto.
+  inversion Hobj_after; subst.
+  simpl.
+  symmetry.
+  apply update_diff.
+  exact Hneq.
+  unfold vpa_assignability in H16.
+  rewrite Hstatic_type in H16; easy.
+  rewrite Hstatic_type in H16; easy.
+- (* RDA case: RDA fields cannot be written *)
+  rewrite Hreceivermut in H6.
+  inversion H6.
+  subst Tx.
+  rewrite Hstatic_type in H15.
+  unfold vpa_assignability in H15.
+  destruct a eqn: Haeqn; try easy.
+  assert (Hneq: anyf <> f).
+  {
+    intro Heq.
+    subst anyf.
+    unfold sf_assignability_rel in H13, Hrda.
+    destruct H13 as [fdef_assign [Hlookup_assign Hassign_assign]].
+    destruct Hrda as [fdef_final [Hlookup_final Hassign_final]].
+    assert (fdef_final = fdef_assign).
+    {
+      eapply field_lookup_deterministic_rel; eauto.
+      eapply field_inheritance_subtyping; eauto.
+    }
+    subst fdef_final.
+    rewrite Hassign_final in Hassign_assign.
+    discriminate.
+  }
+  injection Hobj_before as Hvals_eq.
+  unfold update_field in Hobj_after.
+  rewrite H3 in Hobj_after.
+  simpl in Hobj_after.
+  unfold update_field in Hobj_after.
+  simpl in Hobj_after.
+  assert (Hdom: loc_x < dom h).
+  {
+    apply runtime_getObj_dom in H3.
+    exact H3.
+  }
+  rewrite runtime_getObj_update_same in Hobj_after; auto.
+  inversion Hobj_after; subst.
+  simpl.
+  symmetry.
+  apply update_diff.
+  exact Hneq.
+  rewrite Hstatic_type in H16; easy.
+  rewrite Hstatic_type in H16; easy.
+Qed.
+
+(* TODO: rename RD to RO *)
+Inductive class_reachable (CT : class_table) : class_name -> class_name -> Prop :=
+  (* Base Case: Reflexivity *)
+  | cr_refl : 
+      forall C, 
+        class_reachable CT C C
+
+  (* Inductive Step: Transitivity via Protected Fields *)
+  | cr_step : 
+      forall C f fDef C_next C_target,
+        (* 1. Look up the field definition *)
+        sf_def_rel CT C f fDef ->
+        
+        (* 2. CRITICAL: Only traverse if the field is part of the abstract state 
+             (matches your reachable_abs condition) *)
+        (fDef.(ftype).(mutability) = Imm_f \/ fDef.(ftype).(mutability) = RDM_f) ->
+        
+        (* 3. Get the static type of the field *)
+        C_next = fDef.(ftype).(f_base_type) ->
+        
+        (* 4. Transitivity *)
+        class_reachable CT C_next C_target ->
+        
+        class_reachable CT C C_target.
+
+Inductive static_reachable (CT : class_table) (sΓ : s_env) : var -> class_name -> Prop :=
+  | srch_entry : 
+      forall x T C_target,
+        (* 1. Look up x in the static environment *)
+        static_getType sΓ x = Some T ->
+        
+        (* 2. Check if the class of x reaches C_target *)
+        class_reachable CT (sctype T) C_target ->
+        
+        static_reachable CT sΓ x C_target.
+
+Lemma vpa_mutabilty_stype_fld_rd_not_mut :
+  forall q_recv q_field q_res
+         (Hrd : q_recv = Rd)
+         (Hvpa : vpa_mutabilty_stype_fld q_recv q_field = q_res),
+    q_res <> Mut.
+Proof.
+  intros. subst.
+  unfold vpa_mutabilty_stype_fld.
+  destruct q_field; subst; try easy.
+Qed.
+
+(* Definition is_protected_root (T : qualified_type) : Prop :=
+  sqtype T = Rd \/ sqtype T = Imm. *)
+
+(* Safe means preserve shallow immutability *)
+Definition is_safe_mode (m : q) : Prop :=
+  (* m = Rd. *)
+  m = Rd \/ m = Lost.
+  (* Don't use bot because not interesting *)
+  (* m = Rd \/ m = Imm \/ m = Lost \/ m = Bot. *)  
+
+Definition protected_locset
+  (CT : class_table) (h : heap) (l_root : Loc) : Ensembles.Ensemble Loc :=
+  fun l_target => reachable_abs CT h l_root l_target.
+
+(* Effectively require all variables *)
+Definition env_respects_protected_set
+  (P : Ensembles.Ensemble Loc) (sΓ : s_env) (rΓ : r_env) : Prop :=
+  forall x l T,
+    static_getType sΓ x = Some T ->
+    runtime_getVal rΓ x = Some (Iot l) ->
+
+    (* (exists l_intermediate,
+      reachable_abs CT h l l_intermediate /\
+      Ensembles.In Loc P l_intermediate) -> *)
+    
+    (* If the location is in the Protected Set... *)
+    Ensembles.In Loc P l ->
+
+    (* ...the variable must be ReadOnly, or Lost. *)
+    is_safe_mode (sqtype T).
+
+Definition heap_respects_protected_set
+  (P : Ensembles.Ensemble Loc) (h_initial h_curr : heap) (CT : class_table) : Prop :=
+  forall l_src C anyrq vals k l_dst,
+    l_dst < dom h_initial ->  (* Only pre-existing objects *)
+    l_src >= dom h_initial ->  (* Only newly allocated objects *)
+    Ensembles.In Loc P l_dst ->
+    runtime_getObj h_curr l_src = Some (mkObj (mkruntime_type anyrq C) vals) ->
+    nth_error vals k = Some (Iot l_dst) ->
+    exists fDef,
+      sf_def_rel CT C k fDef /\
+      (fDef.(ftype).(mutability) = Rd_f).
+
+Definition confinement_invariant_precise
+  (P : Ensembles.Ensemble Loc) 
+  (CT : class_table) 
+  (sΓ : s_env) 
+  (rΓ : r_env) 
+  (h_initial h_curr : heap) : Prop :=
+  env_respects_protected_set P sΓ rΓ /\
+  heap_respects_protected_set P h_initial h_curr CT.
+
+Lemma mut_var_cannot_point_to_P :
+  forall sΓ rΓ x T l P
+         (Hlookup : static_getType sΓ x = Some T)
+         (Hval : runtime_getVal rΓ x = Some (Iot l))
+         (Henv_safe : env_respects_protected_set P sΓ rΓ)
+         (Hin_P : Ensembles.In Loc P l),
+    sqtype T <> Mut.
+Proof.
+  intros.
+  (* Unfold the invariant *)
+  unfold env_respects_protected_set in Henv_safe.
+  specialize (Henv_safe x l T Hlookup Hval Hin_P).
+  (* Henv_safe says T is Rd/Imm/Lost. Thus it is not Mut. *)
+  unfold is_safe_mode in Henv_safe.
+  intuition; subst; discriminate.
+Qed.
+
+(* Lemma step_preserves_confinement :
+  forall CT sΓ rΓ h l_root stmt sΓ' rΓ' h' P
+         (HP_def : P = protected_locset CT h l_root)
+         (Hconfined : confinement_invariant_precise P CT sΓ rΓ h)
+         (Hwf : wf_r_config CT sΓ rΓ h)
+         (Htyping : stmt_typing CT sΓ stmt sΓ')
+         (Heval : eval_stmt OK CT rΓ h stmt OK rΓ' h'),
+    confinement_invariant_precise P CT sΓ' rΓ' h'.
+Proof.
+  intros.
+  remember OK as ok.
+  generalize dependent sΓ.
+  generalize dependent sΓ'.
+  induction Heval; intros; subst; try discriminate.
+  - (* Skip *) 
+    inversion Htyping; subst.
+    exact Hconfined.
+  - (* Local *)
+    inversion Htyping; subst.
+    unfold confinement_invariant_precise in *.
+    destruct Hconfined as [Henv_respects Hheap_respects].
+    split.
+    + (* Env respects *)
+  (* Induction on eval_stmt. Use Lemma 2 for SAssignField. *)
+  (* Use Lemma 1 to show we don't violate env_respects for SAssign. *)
+
+Lemma step_preserves_protected_values :
+  forall CT sΓ rΓ h l_root stmt sΓ' rΓ' h' P l C anyrq vals vals'
+         (HP : P = protected_locset CT h l_root) (* P is fixed to PRE-state *)
+         (Hconfined : confinement_invariant_precise P CT sΓ rΓ h)
+         (Hwf : wf_r_config CT sΓ rΓ h)
+         (Htyping : stmt_typing CT sΓ stmt sΓ')
+         (Heval : eval_stmt OK CT rΓ h stmt OK rΓ' h')
+         (* The object is in P *)
+         (Hin : Ensembles.In Loc P l)
+         (Hobj : runtime_getObj h l = Some (mkObj (mkruntime_type anyrq C) vals))
+         (Hobj' : runtime_getObj h' l = Some (mkObj (mkruntime_type anyrq C) vals')),
+    (* Conclusion: Protected fields are equal *)
+    forall f, (sf_assignability_rel CT C f Final \/ sf_assignability_rel CT C f RDA) ->
+    nth_error vals f = nth_error vals' f.
+Proof.
+  intros.
+  remember OK as ok.
+  generalize dependent sΓ.
+  generalize dependent sΓ'.
+  induction Heval; intros; subst; try discriminate.
+  - (* Skip *) 
+    rewrite Hobj in Hobj'.
+    inversion Hobj'; subst.
+    reflexivity.
+  - (* Local *)
+    rewrite Hobj in Hobj'.
+    inversion Hobj'; subst.
+    reflexivity.
+  - (* VarAss *)
+    rewrite Hobj in Hobj'.
+    inversion Hobj'; subst.
+    reflexivity.
+  - (* FldWrite *)
+    {
+    destruct (Nat.eq_dec loc_x l) as [Halias | Hno_alias].
+    -
+      subst loc_x.
+      destruct (Nat.eq_dec f f0) as [Heq_f | Hneq_f].
+      + (* Same field case: contradiction *)
+        subst f0.
+        (* Now: x points to l, and l ∈ P *)
+        (* Strategy: Show x must be Safe, but field write requires x to be Mut → contradiction *)
+        
+        (* Extract x's static type from typing *)
+        inversion Htyping; subst.
+        (* After inversion: static_getType sΓ x = Some Tx, and sqtype Tx should allow write *)
+        
+        (* Unfold confinement to get env_respects_protected_set *)
+        unfold confinement_invariant_precise in Hconfined.
+        destruct Hconfined as [Henv_respects _].
+        
+        (* Apply the lemma: if x points to l ∈ P, then x is Safe *)
+        have Hx_safe := mut_var_cannot_point_to_P sΓ' rΓ x Tx l (protected_locset CT h l_root) H8 H0 Henv_respects Hin.
+        
+        (* But from ST_FldWrite typing, we need sqtype Tx to allow writes *)
+        (* H15: vpa_assignability (sqtype Tx) a = Assignable *)
+        
+        (* Case on assignability *)
+        apply vpa_assingability_assign_cases in H17.
+        unfold wf_r_config in Hwf.
+        destruct Hwf as [Hclasstable [_[Hrenv [_ [_ Htypable]]]]].
+        unfold wf_renv in Hrenv.
+        destruct Hrenv as [_ [Hreceiver _]].
+        destruct Hreceiver as [iot [Hget_iot Hiot_dom]].
+        assert (HOutterReceiverMutability: exists qcontext, r_muttype h iot = Some qcontext).
+        {
+          eapply receiver_mutability_exists_from_bound; eauto.
+        }
+        destruct HOutterReceiverMutability as [qcontext Hqcontext].
+        (* Apply correspondence to get wf_r_typable *)
+        specialize (Htypable iot qcontext Hget_iot Hqcontext x).
+        have H8copy := H8.
+        apply static_getType_dom in H8.
+        unfold static_getType in H8copy.
+        specialize (Htypable H8 Tx H8copy).
+        rewrite H0 in Htypable.
+        unfold wf_r_typable in Htypable.
+        unfold r_type in Htypable.
+        rewrite Hobj in Htypable.
+        destruct Htypable as [base qualifier].
+        simpl in base.
+        destruct H17 as [Ha_assign | [Hx_mut Ha_rda]].
+        
+        ++ (* Case: a = Assignable *)
+          destruct H as [HFinal | HRDA].
+          * (* Case: sf_assignability_rel CT C f Final *)
+          assert (Heq : Final = a).
+          {
+            eapply sf_assignability_consistent_subtype with (f := f) (C := C) (D := sctype Tx); eauto.
+          }
+          rewrite <- Heq in Ha_assign.
+          discriminate Ha_assign.
+          *
+          assert (Heq : RDA = a).
+          {
+            eapply sf_assignability_consistent_subtype with (f := f) (C := C) (D := sctype Tx); eauto.
+          }
+          rewrite <- Heq in Ha_assign.
+          discriminate Ha_assign.
+        ++ (* Case: sqtype Tx = Mut ∧ a = RDA *)
+          exfalso.
+          apply Hx_safe.
+          exact Hx_mut.
+      + (* Different field case: trivial *)
+        unfold update_field in Hobj'.
+        rewrite H1 in Hobj'.
+        simpl in Hobj'.
+
+        (* Extract the domain bound for l *)
+        assert (Hdom : l < dom h).
+        {
+          apply runtime_getObj_dom in H1.
+          exact H1.
+        }
+
+        (* After update_field, the object at l has fields updated at f0 *)
+        rewrite runtime_getObj_update_same in Hobj'; auto.
+
+        (* Now Hobj' shows vals' = update f0 val_y (fields_map o) *)
+        (* And Hobj shows vals = fields_map o *)
+        injection Hobj' as _ Hvals'_eq.
+        rewrite H1 in Hobj.
+        injection Hobj as Hvals_eq.
+        (* rewrite <- Hfields_eq in Hvals'_eq. *)
+
+        (* vals' is just vals with f0 updated, so f is unchanged *)
+        rewrite <- Hvals'_eq.
+        rewrite update_diff.
+        -- symmetry. exact Hneq_f.
+        -- 
+        assert (Hfields : fields_map o = vals).
+        {
+          rewrite Hvals_eq.
+          reflexivity.
+        }
+        rewrite Hfields.
+        reflexivity.
+    -
+      (* No aliasing case: trivial *)
+      unfold update_field in Hobj'.
+      have Heq : runtime_getObj 
+        (match runtime_getObj h loc_x with
+        | Some o => [loc_x ↦ o <| fields_map := update f0 val_y (fields_map o) |>] h
+        | None => h
+        end) l = runtime_getObj h l.
+      {
+        destruct (runtime_getObj h loc_x).
+        - apply runtime_getObj_update_diff; auto.
+        - reflexivity.
+      }
+      rewrite Heq in Hobj'.
+      rewrite Hobj in Hobj'.
+      inversion Hobj'.
+      reflexivity.
+  }
+  - (* New *)
+    unfold protected_locset in Hin.
+  
+    (* Extract l < dom h from reachable_abs *)
+    assert(Hl_old : l < dom h).
+    {
+      apply runtime_getObj_dom in Hobj.
+      exact Hobj.
+    }
+    
+    rewrite runtime_getObj_last2 in Hobj'; auto.
+  - (* Call *)
+  - (* Seq *)
+*)
+
+Lemma extract_receiver_from_wf_config :
+  forall CT sΓ rΓ h
+    (Hwf : wf_r_config CT sΓ rΓ h),
+    exists iot qcontext,
+      get_this_var_mapping (vars rΓ) = Some iot /\
+      iot < dom h /\
+      r_muttype h iot = Some qcontext.
+Proof.
+  intros CT sΓ rΓ h Hwf.
+  unfold wf_r_config in Hwf.
+  destruct Hwf as [_ [_ [Hrenv _]]].
+  destruct Hrenv as [_ [Hreceiver _]].
+  destruct Hreceiver as [iot [Hget_iot Hiot_dom]].
+  exists iot.
+  assert (HOutterReceiverMutability: exists qcontext, r_muttype h iot = Some qcontext).
+  {
+    eapply receiver_mutability_exists_from_bound; eauto.
+  }
+  destruct HOutterReceiverMutability as [qcontext Hqcontext].
+  exists qcontext.
+  (* TODO: is there better way to write this tactics? *)
+  split. 
+  exact Hget_iot.
+  split.
+  exact Hiot_dom.
+  exact Hqcontext. 
+Qed.
+
+Lemma subtype_safe_implies_safe :
+  forall CT T_sub T_super
+         (Hsub : qualified_type_subtype CT T_sub T_super)
+         (Hsafe_sub : is_safe_mode (sqtype T_sub)),
+    is_safe_mode (sqtype T_super).
+Proof.
+  intros. unfold is_safe_mode in *.
+  apply qualified_type_subtype_q_subtype in Hsub.
+  inversion Hsub; subst; auto.
+  rewrite <- H0 in Hsafe_sub.
+  destruct Hsafe_sub as [Hrd | Hlost].
+  inversion Hrd. 
+  inversion Hlost.
+Qed.
+
+Lemma adapated_subtype_safe_implies_safe :
+  forall CT T_sub T_Receiver T_super
+         (Hsub : qualified_type_subtype CT T_sub (vpa_mutabilty_tt T_Receiver T_super))
+         (Hsafe_sub : is_safe_mode (sqtype T_sub)),
+    is_safe_mode (sqtype T_super).
+Proof.
+  intros.
+  unfold is_safe_mode in *.
+  apply qualified_type_subtype_q_subtype in Hsub.
+  unfold vpa_mutabilty_tt in Hsub.
+  destruct (sqtype T_Receiver) eqn: Hreceiver;
+  destruct (sqtype T_super) eqn: HSuper;
+  destruct Hsafe_sub as [Hrd | Hlost];
+  try rewrite Hrd in Hsub;
+  try rewrite Hlost in Hsub;
+  try rewrite <- H in Hsub;
+  inversion Hsub; subst; auto.
+  all: try rewrite HSuper in H; try rewrite HSuper in H1; try discriminate.
+  all: try easy.
+Qed.
+
+Lemma subtype_safe_implies_safe_adapted :
+  forall CT T_sub T_Receiver T_super
+         (Hsub : qualified_type_subtype CT (vpa_mutabilty_tt T_Receiver T_sub) T_super)
+         (Hsafe_sub : is_safe_mode (sqtype T_sub)),
+    is_safe_mode (sqtype T_super).
+Proof.
+  intros.
+  unfold is_safe_mode in *.
+  apply qualified_type_subtype_q_subtype in Hsub.
+  unfold vpa_mutabilty_tt in Hsub.
+  destruct (sqtype T_Receiver) eqn: Hreceiver;
+  destruct (sqtype T_super) eqn: HSuper;
+  destruct Hsafe_sub as [Hrd | Hlost];
+  try rewrite Hrd in Hsub;
+  try rewrite Hlost in Hsub;
+  try rewrite <- H in Hsub;
+  inversion Hsub; subst; auto.
+  all: try rewrite HSuper in H; try rewrite Hrd in H0; try rewrite Hlost in H0; try discriminate.
+Qed.
+
+Lemma reachable_abs_dom :
+  forall CT h l_src l_dst
+    (Hreach : reachable_abs CT h l_src l_dst),
+    l_dst < dom h.
+Proof.
+  intros CT h l_src l_dst Hreach.
+  induction Hreach.
+  - (* Base case: reachable_abs_heap *)
+    exact H.
+  - (* Step case: reachable_abs_step *)
+    exact H.
+  - (* Trans case *)
+    exact IHHreach2.
+Qed.
+
+Lemma confinement_from_all_readonly_env :
+  forall CT sΓ rΓ h x l_root
+    (Hdom_root : l_root < dom h)
+    (Hwf : wf_r_config CT sΓ rΓ h)
+    (Hgetval : runtime_getVal rΓ x = Some (Iot l_root))
+    (Hall_readonly : forall y T,
+      static_getType sΓ y = Some T ->
+      is_safe_mode (sqtype T)),
+    confinement_invariant_precise (protected_locset CT h l_root) CT sΓ rΓ h h.
+Proof.
+  intros.
+  unfold confinement_invariant_precise.
+  split.
+  - (* env_respects_protected_set *)
+    unfold env_respects_protected_set.
+    intros z l T Hlookup_s Hlookup_r Hin_P.
+    exact (Hall_readonly z T Hlookup_s).
+  - (* heap_respects_protected_set *)
+    unfold heap_respects_protected_set.
+    intros l_src C anyrq vals k l_dst Hdom_dst Hdom_src Hin_dst Hobj_src Hnth.
+    (* For (h, h), we have h_initial = h_curr = h *)
+    (* Therefore: l_src >= dom h *)
+    (* But also: runtime_getObj h l_src = Some (...) requires l_src < dom h *)
+    exfalso.
+    apply runtime_getObj_dom in Hobj_src.
+    lia.  (* This part depends on heap wellformedness properties *)
+Qed.
+
+(* Lemma expr_eval_to_protected_implies_safe_type :
+  forall P CT sΓ rΓ h l_root e l_res Te
+         (Hwf : wf_r_config CT sΓ rΓ h)
+         (Hdom_root : l_root < dom h)
+         (HP_def : P = protected_locset CT h l_root)
+         (*  *)
+         (Hconfined : confinement_invariant_precise P CT sΓ rΓ h h)
+         (Heval : eval_expr OK CT rΓ h e (Iot l_res) OK rΓ h)
+         (Htyp : expr_has_type CT sΓ e Te)
+         (Hin : Ensembles.In Loc P l_res),
+    is_safe_mode (sqtype Te).
+Proof.
+  intros.
+  destruct (extract_receiver_from_wf_config CT sΓ rΓ h Hwf) as [iot [qcontext [Hget_iot[Hiot_dom Hqcontext]]]].
+  have htyp_copy := Htyp.
+  eapply expr_eval_preservation with (v:= Iot l_res) (rΓ' := rΓ) (h' := h) in Htyp; eauto.
+  unfold wf_r_typable in Htyp.
+  unfold r_type in Htyp.
+  destruct (runtime_getObj h l_res); try easy.
+  (* remember OK as ok. *)
+  inversion Heval; subst.
+  - (* EVar case *)
+  inversion htyp_copy; subst.
+    (* Now Htyp should give us: expr_has_type CT sΓ (EVar x) Te *)
+    (* which means static_getType sΓ x = Some Te *)
+    
+    unfold confinement_invariant_precise in Hconfined.
+    destruct Hconfined as [Henv_respects Hheap_respects].
+    
+    (* Apply env_respects_protected_set *)
+    unfold env_respects_protected_set in Henv_respects.
+    specialize (Henv_respects x l_res Te).
+    have H_static : static_getType sΓ x = Some Te.
+    {
+      auto.
+    }
+    
+    specialize (Henv_respects H_static H Hin).
+    exact Henv_respects.
+  - (* EField case *)
+    inversion htyp_copy; subst.
+    (* unfold is_safe_mode; simpl. *)
+    (* unfold vpa_mutabilty_stype_fld. *)
+    (* unfold confinement_invariant_precise in Hconfined. *)
+    destruct Hconfined as [Henv_respects Hheap_respects].
+    set (P := protected_locset CT h l_root).
+    destruct (classic (Ensembles.In Loc P v)) as [Hv_in | Hv_out].
+    +
+      specialize (Henv_respects x v T H7 H Hv_in).
+      unfold is_safe_mode in Henv_respects.
+      subst. simpl.
+      destruct Henv_respects as [Hrd | Hlost].
+      *
+      rewrite Hrd.
+      unfold vpa_mutabilty_stype_fld.
+      unfold is_safe_mode.
+      destruct (mutability (ftype fDef)); try easy.
+      right; reflexivity.
+      right; reflexivity.
+      right; reflexivity.
+      right; reflexivity.
+      *
+      rewrite Hlost.
+      unfold vpa_mutabilty_stype_fld.
+      unfold is_safe_mode.
+      right; reflexivity.
+    +
+    assert (Hdom_v : v < dom h) by (apply runtime_getObj_dom in H0; exact H0).
+
+    (* Extract C and vals from o0 *)
+    destruct o0 as [[anyrq C] vals_v].
+    simpl in H1.
+    assert (Hdom_l_res : l_res < dom h) by (apply reachable_abs_dom in Hin; exact Hin).
+    unfold env_respects_protected_set in Henv_respects.
+    specialize (Henv_respects x v T H7 H)
+    specialize (Hheap_respects v C anyrq vals_v f l_res
+            Hdom_l_res Hin H0 H1).
+    
+      destruct Hheap_respects as [fDef' [Hlookup' Hmut_rd]].
+      (* Align static/runtime field defs *)
+      destruct Htyp as [Hbasetype Hqualifier].
+      simpl in Hbasetype.
+      eapply field_lookup_deterministic_rel in Hlookup';
+        [| eapply field_inheritance_subtyping; eauto].
+      subst fDef'.
+      rewrite Hmut_rd.
+      (* Now fDef.mutability = Rd_f *)
+      
+      unfold is_safe_mode.
+      unfold vpa_mutabilty_stype_fld.
+      destruct (sqtype T); simpl; try easy.
+      left; reflexivity.
+      left; reflexivity.
+      left; reflexivity.
+      right; reflexivity.
+      right; reflexivity.
+      left; reflexivity.
+      unfold wf_r_config in Hwf.
+      destruct Hwf as [_ [_ [_ [_ [_ Hcorr]]]]].
+      assert (Hx_dom : x < dom sΓ) by (apply static_getType_dom in H7; exact H7).
+      specialize (Hcorr iot qcontext Hget_iot Hqcontext x Hx_dom T H7).
+      rewrite H in Hcorr.
+      unfold wf_r_typable in Hcorr.
+      unfold r_type in Hcorr.
+      rewrite H0 in Hcorr.
+      simpl in Hcorr.
+      destruct Hcorr as [Hbaseruntime _].
+      (* Hbaseruntime: base_subtype CT (rctype (rt_type o)) (sctype T) *)
+      (* We have rctype (rt_type o) = C from H0 *)
+      simpl in Hbaseruntime.
+      exact Hbaseruntime.
+Qed. *)
+
+Lemma runtime_getObj_app_left_equal : forall h h_ext loc,
+  loc < dom h ->
+  runtime_getObj h loc = runtime_getObj (h ++ [h_ext]) loc.
+Proof.
+  intros h h_ext loc Hloc_dom.
+  unfold runtime_getObj.
+  rewrite nth_error_app1; auto.
+Qed.
+
+Lemma env_respects_weaken :
+  forall CT sΓ rΓ h l_root l_intermediate
+    (Hreach : reachable_abs CT h l_root l_intermediate)
+    (Henv_respects : env_respects_protected_set (protected_locset CT h l_root) sΓ rΓ),
+    env_respects_protected_set (protected_locset CT h l_intermediate) sΓ rΓ.
+Proof.
+  intros CT sΓ rΓ h l_root l_intermediate Hreach Henv_respects.
+  intros x l T Hlookup Hval Hin_l_intermediate.
+  unfold protected_locset in Hin_l_intermediate.
+  have Hin_l_root : Ensembles.In Loc (protected_locset CT h l_root) l :=
+    reachable_abs_trans CT h l_root l_intermediate l Hreach Hin_l_intermediate.
+  exact (Henv_respects x l T Hlookup Hval Hin_l_root).
+Qed.
+
+Lemma heap_respects_weaken :
+  forall CT h_initial h_curr l_root l_intermediate
+    (Hreach : reachable_abs CT h_curr l_root l_intermediate)
+    (Hheap : heap_respects_protected_set (protected_locset CT h_curr l_root) h_initial h_curr CT),
+    heap_respects_protected_set (protected_locset CT h_curr l_intermediate) h_initial h_curr CT.
+Proof.
+  intros CT h_initial h_curr l_root l_intermediate Hreach Hheap.
+  unfold heap_respects_protected_set in *.
+  intros l_src C anyrq vals k l_dst Hdom_dst Hlsrc_new Hin_l_intermediate Hobj Hnth.
+  (* The key: Hin_l_intermediate says l_dst ∈ protected_locset(l_intermediate)
+     By transitivity: l_dst ∈ protected_locset(l_root) *)
+  have Hin_l_root : Ensembles.In Loc (protected_locset CT h_curr l_root) l_dst :=
+    reachable_abs_trans CT h_curr l_root l_intermediate l_dst Hreach Hin_l_intermediate.
+  (* Now apply Hheap with all the same conditions *)
+  exact (Hheap l_src C anyrq vals k l_dst Hdom_dst Hlsrc_new Hin_l_root Hobj Hnth).
+Qed.
+
+Lemma confinement_invariant_weaken :
+  forall CT sΓ rΓ h_initial h_curr l_root l_intermediate
+    (Hreach : reachable_abs CT h_curr l_root l_intermediate)
+    (Hconf : confinement_invariant_precise (protected_locset CT h_curr l_root) CT sΓ rΓ h_initial h_curr),
+    confinement_invariant_precise (protected_locset CT h_curr l_intermediate) CT sΓ rΓ h_initial h_curr.
+Proof.
+  intros CT sΓ rΓ h_initial h_curr l_root l_intermediate Hreach Hconf.
+  unfold confinement_invariant_precise in *.
+  destruct Hconf as [Henv_respects Hheap_respects].
+  split.
+  - (* env_respects_protected_set weakens *)
+    eapply env_respects_weaken; eauto.
+  - (* heap_respects_protected_set weakens *)
+    eapply heap_respects_weaken; eauto.
+Qed.
+
+Lemma stmt_preserves_both :
+  forall CT sΓ rΓ h l_root stmt sΓ' rΓ' h'
+    (Hdom_root : l_root < dom h)
+    (Hconfined : confinement_invariant_precise (protected_locset CT h l_root) CT sΓ rΓ h h)
+    (Hwf : wf_r_config CT sΓ rΓ h)
+    (Htyping : stmt_typing CT sΓ stmt sΓ')
+    (Heval : eval_stmt OK CT rΓ h stmt OK rΓ' h'),
+  protected_locset CT h l_root = protected_locset CT h' l_root /\
+  confinement_invariant_precise (protected_locset CT h l_root) CT sΓ' rΓ' h h'.
+Proof.
+  intros.
+  remember OK as ok.
+  generalize dependent sΓ.
+  generalize dependent sΓ'.
+  have Heval_copy := Heval.
+  induction Heval; intros; subst; try discriminate.
+  7:
+  {
+  inversion Htyping; subst.
+
+  (* Apply IH1 *)
+  pose proof (IHHeval1 Hdom_root eq_refl Heval1 sΓ'0 sΓ Hconfined Hwf H4) as [HeqP1 Hconf1].
+
+  (* Get wellformedness for intermediate state *)
+  pose proof (preservation_pico _ _ _ _ _ _ _ _ Hwf H4 Heval1) as Hwf'.
+
+  assert (Hdom_root' : l_root < dom h').
+  {
+    apply eval_stmt_preserves_heap_domain_simple in Heval1; eauto.
+    lia.
+  }
+
+  (* Convert Hconf1 from (h, h') to (h', h') parametrization *)
+  assert (Hconf1_for_ih2 : confinement_invariant_precise (protected_locset CT h' l_root) CT sΓ'0 rΓ' h' h').
+  {
+    unfold confinement_invariant_precise in Hconf1.
+    destruct Hconf1 as [Henv1 Hheap1].
+    split.
+    + rewrite <- HeqP1. exact Henv1.
+    + unfold heap_respects_protected_set.
+      intros l_src C anyrq vals k l_dst Hdom_dst Hlsrc_new Hin_dst Hobj_src Hnth.
+      (* For (h', h'): l_src >= dom h' but also runtime_getObj h' l_src = Some(...) requires l_src < dom h' *)
+      exfalso.
+      apply runtime_getObj_dom in Hobj_src.
+      lia.
+  }
+
+  (* Apply IH2 *)
+  pose proof (IHHeval2 Hdom_root' eq_refl Heval2 sΓ' sΓ'0 Hconf1_for_ih2 Hwf' H6) as [HeqP2 Hconf2].
+
+  (* Now chain the equalities via transitivity *)
+  assert (HeqP : protected_locset CT h l_root = protected_locset CT h'' l_root).
+  {
+    (* By HeqP1 and HeqP2 *)
+    rewrite HeqP1.
+    exact HeqP2.
+  }
+
+  (* For the invariant part, convert Hconf2 back *)
+  assert (Hconf_final : confinement_invariant_precise (protected_locset CT h l_root) CT sΓ' rΓ'' h h'').
+  {
+    unfold confinement_invariant_precise in Hconf1, Hconf2, Hconfined, Hconf1_for_ih2.
+    destruct Hconf1 as [Henv1 Hheap1].
+    destruct Hconf2 as [Henv2 Hheap2].
+    destruct Hconfined as [Henv0 Hheap0].
+    destruct Hconf1_for_ih2 as [Henv1' Hheap1'].
+    split.
+    + rewrite HeqP. rewrite <- HeqP2. exact Henv2.
+    + unfold heap_respects_protected_set in *.
+      intros l_src C anyrq vals k l_dst Hdom_dst_h Hlsrc_new_h Hin_dst Hobj_src Hnth.
+      have Hdom_h_h' : dom h <= dom h' by
+      (apply eval_stmt_preserves_heap_domain_simple in Heval1; lia).
+      destruct (le_lt_dec (dom h') l_src) as [Hlsrc_new_h' | Hlsrc_old_h'].
+    - (* Case: l_src >= dom h' (allocated during second statement) *)
+      have Hin_dst' : Ensembles.In Loc (protected_locset CT h' l_root) l_dst by
+        (rewrite <- HeqP1; exact Hin_dst).
+      have Hdom_dst_h' : l_dst < dom h' by
+        (apply reachable_abs_dom in Hin_dst'; exact Hin_dst').  
+      exact (Hheap2 l_src C anyrq vals k l_dst Hdom_dst_h' Hlsrc_new_h' Hin_dst' Hobj_src Hnth).
+    - (* Case: l_src < dom h' (allocated before or during first statement) *)
+      unfold env_respects_protected_set in *.
+      (* have Hh'some : exists C' vals', runtime_getObj h' l_src = Some (mkObj C' vals').
+      {
+        eapply runtime_getObj_Some; auto.
+      }
+
+      destruct Hh'some as [C' [vals' Hh'some]].
+
+      have Hh''some: exists vals'', runtime_getObj h'' l_src = Some
+      {| rt_type := C'; fields_map :=vals''|}.
+      {
+        eapply runtime_preserves_r_type_heap with (h := h') (h' := h'')(vals := vals'); eauto.
+      }
+
+      destruct Hh''some as [vals'' Hh''some].
+      rewrite Hh''some in Hobj_src.
+      inversion Hobj_src; subst C' vals''.
+      eapply Hheap1 with (l_dst := l_dst) (l_src := l_src) (vals := vals'); eauto.
+      rename vals into vals''. *)
+      admit.
+  }
+
+  split.
+  + exact HeqP.
+  + exact Hconf_final.
+  }
+  - (* skip *)
+    inversion Htyping; subst.
+    split; [reflexivity | exact Hconfined].
+  - (* local *)
+    split.
+    + reflexivity.
+    + (* Invariant preserved *)
+    inversion Htyping; subst.
+    unfold confinement_invariant_precise in *.
+    destruct Hconfined as [Henv_respects Hheap_respects].
+    split.
+    *
+      unfold env_respects_protected_set.
+      intros y l_y Ty Hlookup_s Hlookup_r Hin_P.
+      destruct (Nat.eq_dec x y); subst.
+      --
+        assert (y = dom sΓ).
+        {
+          apply static_getType_dom in Hlookup_s.
+          apply static_getType_not_dom in H4.
+          rewrite length_app in Hlookup_s; simpl in Hlookup_s. (* dom (sΓ++[T]) = S (dom sΓ) *)
+          lia.
+        }
+        rewrite H0 in Hlookup_s.
+        destruct Hwf as [_ [_ [_ [_ [Hlen _]]]]]. (* gives dom sΓ = dom (vars rΓ) *)
+        rewrite H0 in Hlookup_r.                  (* y = dom sΓ *)
+        rewrite Hlen in Hlookup_r.                (* now y = dom (vars rΓ) *)
+        rewrite runtime_getVal_last in Hlookup_r. (* yields Some Null_a *)
+        discriminate.
+      --
+
+        assert (H_bound : y < dom sΓ).
+        {
+          (* Use the lookup success in the extended list *)
+          apply static_getType_dom in Hlookup_s.
+          rewrite length_app in Hlookup_s.
+          simpl in Hlookup_s.
+          assert (H_x_idx : x = dom sΓ). 
+          {
+            inversion Htyping; subst.
+            apply static_getType_not_dom in H4.
+            apply static_getType_dom in H9.
+            rewrite length_app in H9; simpl in H9.
+            lia.
+          }
+          
+          (* With x = length sΓ and x <> y, we know y < length sΓ *)
+          lia. 
+        }
+
+        assert (Hlookup_s_old : static_getType sΓ y = Some Ty).
+        {
+          unfold static_getType in *.
+          rewrite nth_error_app1 in Hlookup_s; auto.
+        }
+
+        assert (Hlookup_r_old : runtime_getVal rΓ y = Some (Iot l_y)).
+        {
+          unfold runtime_getVal in *.
+          rewrite nth_error_app1 in Hlookup_r; auto.
+          destruct Hwf as [_ [_ [_ [_ [Hlen _]]]]]. (* gives dom sΓ = dom (vars rΓ) *)
+          rewrite Hlen in H_bound.                (* now y = dom (vars rΓ) *)
+          auto.
+        }
+
+        unfold env_respects_protected_set in Henv_respects.
+        exact (Henv_respects y l_y Ty Hlookup_s_old Hlookup_r_old Hin_P).
+    *
+      unfold heap_respects_protected_set.
+      intros l_src C anyrq vals k l_dst Hdom_src Hin_dst Hobj_src Hnth.
+      unfold heap_respects_protected_set in Hheap_respects.
+      exact (Hheap_respects l_src C anyrq vals k l_dst Hdom_src Hin_dst Hobj_src Hnth).
+  - (* var assign *)
+    split.
+    + reflexivity.
+    + (* Invariant preserved *)
+      inversion Htyping; subst.
+      have Hconfined_copy := Hconfined.
+      unfold confinement_invariant_precise.
+      unfold confinement_invariant_precise in Hconfined.
+      destruct Hconfined as [Henv_respects Hheap_respects].
+      rename sΓ' into sΓ.
+      split.
+      *
+        unfold env_respects_protected_set.
+        intros y l_y Ty Hlookup_s Hlookup_r Hin_P.
+        unfold runtime_getVal in Hlookup_r.
+        simpl in Hlookup_r.
+        destruct (Nat.eq_dec y x) as [Heq_y | Hneq_y].
+        -- (* y = x *)
+        subst y.
+        rewrite H9 in Hlookup_s.
+        inversion Hlookup_s; subst Ty.
+        apply runtime_getVal_dom in H.
+        rewrite update_same in Hlookup_r; auto.
+        injection Hlookup_r as Heq_v2.
+        subst v2.
+        assert (Hsafe_e : is_safe_mode (sqtype Te)).
+        {
+          admit.
+          (* eapply expr_eval_to_protected_implies_safe_type; eauto. *)
+        }
+        eapply subtype_safe_implies_safe; eauto.
+        -- (* y <> x *)
+        rewrite update_diff in Hlookup_r; auto.
+        unfold env_respects_protected_set in Henv_respects.
+        exact (Henv_respects y l_y Ty Hlookup_s Hlookup_r Hin_P).
+      * 
+        unfold heap_respects_protected_set.
+        intros l_src C anyrq vals k l_dst Hdom_src Hin_dst Hobj_src Hnth.
+        unfold heap_respects_protected_set in Hheap_respects.
+        exact (Hheap_respects l_src C anyrq vals k l_dst Hdom_src Hin_dst Hobj_src Hnth).
+  - (* field write *)
+    split.
+    +
+    {
+      unfold protected_locset.
+      apply Ensembles.Extensionality_Ensembles.
+      unfold Ensembles.Same_set, Ensembles.Included.
+      split; intros l_target Hreach.
+      - (* Forward direction: h → update_field h *)
+
+        induction Hreach.
+        + (* reachable_abs_heap *)
+          apply reachable_abs_heap.
+          rewrite update_field_length.
+          exact H3.
+        +
+        {
+          destruct (Nat.eq_dec l0 loc_x) as [Hl0 | Hl0].
+          - subst l0.
+            destruct (Nat.eq_dec k f) as [Hkf | Hkf].
+            + (* k = f: you already proved this impossible; reuse that contradiction here *)
+              exfalso. (* your existing contradiction proof *)
+              subst k.
+              (* From H6/H7: field f is RDM/Imm and RDA/Final (protected) *)
+              (* But from typing: field f must be writable *)
+              inversion Htyping; subst.
+              (* H13: sf_assignability_rel CT C f a for some writable a *)
+              unfold wf_r_config in Hwf.
+              destruct Hwf as [_ [_ [Hrenv [_ [Hlen Htypable]]]]].
+
+              (* Get receiver info *)
+              destruct Hrenv as [_ [Hreceiver _]].
+              destruct Hreceiver as [iot [Hget_iot Hiot_dom]].
+
+              (* Get receiver mutability *)
+              assert (HOutterReceiverMutability: exists qcontext, r_muttype h iot = Some qcontext).
+              {
+                eapply receiver_mutability_exists_from_bound; eauto.
+              }
+              destruct HOutterReceiverMutability as [qcontext Hqcontext].
+
+              (* Apply typability correspondence *)
+              assert (Hx_dom : x < dom sΓ').
+              {
+                apply static_getType_dom in H12.
+                exact H12.
+              }
+              specialize (Htypable iot qcontext Hget_iot Hqcontext x Hx_dom Tx H12).
+              rewrite H in Htypable.
+
+              (* Htypable now gives us wf_r_typable for the location *)
+              unfold wf_r_typable in Htypable.
+              unfold r_type in Htypable.
+              rewrite H0 in Htypable.
+              rewrite H4 in H0.
+
+              (* Htypable now contains: base_subtype CT (sctype Tx) C *)
+              destruct Htypable as [Hbase Hqualifier].
+              assert (rctype (rt_type o) = C).
+              {
+                inversion H0.
+                easy.
+              }
+              rewrite H8 in Hbase.
+              destruct H7 as [Hrda | Hfinal].
+              ** (* RDA case *)
+                unfold sf_assignability_rel in *.
+                destruct H18 as [fdef_write [Hlookup_write Hassign_write]].
+                destruct Hrda as [fdef_prot [Hlookup_prot Hassign_prot]].
+
+                assert (fdef_prot = fdef_write).
+                {
+                  eapply field_lookup_deterministic_rel; eauto.
+                  eapply field_inheritance_subtyping; eauto.
+                }
+                subst fdef_prot.
+                rewrite Hassign_prot in Hassign_write.
+                rewrite <- Hassign_write in H21.
+                unfold vpa_assignability in H21.
+                destruct (sqtype Tx) eqn: Hsqtypex; try discriminate.
+                unfold confinement_invariant_precise in Hconfined.
+                destruct Hconfined as [Henv_respects Hheap_respects].
+                unfold env_respects_protected_set in Henv_respects.
+                specialize (Henv_respects x loc_x Tx H12 H).
+                assert (Hin_locx : Ensembles.In Loc (protected_locset CT h loc_x) loc_x).
+                {
+                  unfold protected_locset.
+                  apply reachable_abs_heap.
+                  apply runtime_getObj_dom in H4.
+                  exact H4.
+                }
+                specialize (Henv_respects Hin_locx).
+                unfold is_safe_mode in Henv_respects.
+                destruct Henv_respects as [Hrd | Hlost].
+                --- rewrite Hrd in Hsqtypex. discriminate.
+                --- rewrite Hlost in Hsqtypex. discriminate.
+              ** (* Final case *)
+                unfold sf_assignability_rel in *.
+                destruct H18 as [fdef_write [Hlookup_write Hassign_write]].
+                destruct Hfinal as [fdef_prot [Hlookup_prot Hassign_prot]].
+                assert (fdef_prot = fdef_write).
+                {
+                  eapply field_lookup_deterministic_rel; eauto.
+                  eapply field_inheritance_subtyping; eauto.
+                }
+                subst fdef_prot.
+                rewrite Hassign_prot in Hassign_write.
+                rewrite <- Hassign_write in H21.
+                unfold vpa_assignability in H21.
+                destruct (sqtype Tx); try discriminate.
+            + (* k ≠ f: protected field unchanged *)
+              assert (Hloc_dom : loc_x < dom h) by (apply runtime_getObj_dom in H0; exact H0).
+              apply reachable_abs_step with
+                  (any := any) (C := C) (vals := update f val_y vals) (k := k).
+              * rewrite update_field_length; exact H3.            (* dom unchanged *)
+              * unfold update_field; rewrite H0; simpl.
+                rewrite runtime_getObj_update_same. exact Hloc_dom.
+                rewrite H0 in H4. inversion H4. easy.
+              *  
+                rewrite update_diff. symmetry. exact Hkf. exact H5. (* nth_error preserved *)
+              * exact H6.
+              * exact H7.
+
+          - (* l0 ≠ loc_x: object untouched by the update *)
+            apply reachable_abs_step with (any := any) (C := C) (vals := vals) (k := k).
+            unfold update_field.
+            destruct (runtime_getObj h loc_x); try exact H3.
+            + rewrite update_length. exact H3.
+            + 
+              unfold update_field.
+              destruct (runtime_getObj h loc_x).
+              rewrite runtime_getObj_update_diff.
+              symmetry. exact Hl0.
+              exact H4.
+              exact H4.
+            + exact H5.
+            + exact H6.
+            + exact H7. 
+        }
+        + (* reachable_abs_trans *)
+          eapply reachable_abs_trans.
+          eapply reachable_abs_trans; eauto.
+          * exact (IHHreach1 Hdom_root Hconfined).
+          *
+          apply IHHreach2.
+          -- apply reachable_abs_dom in Hreach1. exact Hreach1.
+          -- eapply confinement_invariant_weaken; eauto.
+          * 
+          apply reachable_abs_heap.
+          apply reachable_abs_dom in Hreach2. 
+          rewrite update_field_length.
+          exact Hreach2.
+
+      - (* Backward direction: update_field h → h *)
+        induction Hreach.
+        + (* reachable_abs_heap *)
+          apply reachable_abs_heap.
+          rewrite update_field_length in H3.
+          exact H3.
+        + (* reachable_abs_step *)
+          destruct (Nat.eq_dec l0 loc_x) as [Heq | Hneq].
+          *
+            subst loc_x.
+            inversion Htyping; subst.
+            specialize (runtime_getObj_Some h l0 Hdom_root) as [C' [values' Hhsome]].
+            remember (update_field h l0 f val_y) as h'.
+            destruct (Nat.eq_dec k f) as [Heq_k | Hneq_k].
+            --
+              exfalso. (* your existing contradiction proof *)
+              subst k.
+              (* From H6/H7: field f is RDM/Imm and RDA/Final (protected) *)
+              (* But from typing: field f must be writable *)
+              (* H13: sf_assignability_rel CT C f a for some writable a *)
+              unfold wf_r_config in Hwf.
+              destruct Hwf as [_ [_ [Hrenv [_ [Hlen Htypable]]]]].
+
+              (* Get receiver info *)
+              destruct Hrenv as [_ [Hreceiver _]].
+              destruct Hreceiver as [iot [Hget_iot Hiot_dom]].
+
+              (* Get receiver mutability *)
+              assert (HOutterReceiverMutability: exists qcontext, r_muttype h iot = Some qcontext).
+              {
+                eapply receiver_mutability_exists_from_bound; eauto.
+              }
+              destruct HOutterReceiverMutability as [qcontext Hqcontext].
+
+              (* Apply typability correspondence *)
+              assert (Hx_dom : x < dom sΓ').
+              {
+                apply static_getType_dom in H12.
+                exact H12.
+              }
+              specialize (Htypable iot qcontext Hget_iot Hqcontext x Hx_dom Tx H12).
+              rewrite H in Htypable.
+
+              (* Htypable now gives us wf_r_typable for the location *)
+              unfold wf_r_typable in Htypable.
+              unfold r_type in Htypable.
+              rewrite H0 in Htypable.
+              (* rewrite H4 in H0. *)
+
+              (* Htypable now contains: base_subtype CT (sctype Tx) C *)
+              destruct Htypable as [Hbase Hqualifier].
+              have Hh'some : exists vals', runtime_getObj h' l0 = Some {| rt_type := C'; fields_map := vals' |}.
+              {
+                eapply runtime_preserves_r_type_heap with (h := h) (h' := h')(vals := values'); eauto.
+              }
+              assert (rctype (rt_type o) = C).
+              {
+                clear - Hh'some H4 H0 Hhsome.
+                rewrite H0 in Hhsome.
+                destruct Hh'some as [vals'' Hh'some].
+                rewrite H4 in Hh'some.
+                inversion Hh'some; subst.
+                inversion Hhsome; subst.
+                easy.
+              }
+              rewrite H8 in Hbase.
+              destruct H7 as [Hrda | Hfinal].
+              ** (* RDA case *)
+                unfold sf_assignability_rel in *.
+                destruct H18 as [fdef_write [Hlookup_write Hassign_write]].
+                destruct Hrda as [fdef_prot [Hlookup_prot Hassign_prot]].
+
+                assert (fdef_prot = fdef_write).
+                {
+                  eapply field_lookup_deterministic_rel; eauto.
+                  eapply field_inheritance_subtyping; eauto.
+                }
+                subst fdef_prot.
+                rewrite Hassign_prot in Hassign_write.
+                rewrite <- Hassign_write in H21.
+                unfold vpa_assignability in H21.
+                destruct (sqtype Tx) eqn: Hsqtypex; try discriminate.
+                unfold confinement_invariant_precise in Hconfined.
+                destruct Hconfined as [Henv_respects Hheap_respects].
+                unfold env_respects_protected_set in Henv_respects.
+                specialize (Henv_respects x l0 Tx H12 H).
+                assert (Hin_locx : Ensembles.In Loc (protected_locset CT h l0) l0).
+                {
+                  unfold protected_locset.
+                  apply reachable_abs_heap.
+                  exact Hdom_root.
+                }
+                specialize (Henv_respects Hin_locx).
+                unfold is_safe_mode in Henv_respects.
+                destruct Henv_respects as [Hrd | Hlost].
+                --- rewrite Hrd in Hsqtypex. discriminate.
+                --- rewrite Hlost in Hsqtypex. discriminate.
+              ** (* Final case *)
+                unfold sf_assignability_rel in *.
+                destruct H18 as [fdef_write [Hlookup_write Hassign_write]].
+                destruct Hfinal as [fdef_prot [Hlookup_prot Hassign_prot]].
+                assert (fdef_prot = fdef_write).
+                {
+                  eapply field_lookup_deterministic_rel; eauto.
+                  eapply field_inheritance_subtyping; eauto.
+                }
+                subst fdef_prot.
+                rewrite Hassign_prot in Hassign_write.
+                rewrite <- Hassign_write in H21.
+                unfold vpa_assignability in H21.
+                destruct (sqtype Tx); try discriminate.
+            --
+              have Hl1_dom : l1 < dom h.
+              {
+                subst h'.
+                rewrite update_field_length in H3.
+                exact H3.
+              }
+
+              eapply reachable_abs_step with (vals := values')(any := any)(C := C)(k := k); auto.
+              have Hh'some : exists vals', runtime_getObj h' l0 = Some {| rt_type := C'; fields_map := vals' |}.
+              {
+                eapply runtime_preserves_r_type_heap with (h := h) (h' := h')(vals := values'); eauto.
+              }
+              destruct Hh'some as [vals'' Hh'some].
+              rewrite Hh'some in H4.
+              inversion H4; subst; auto.
+              have Hh'some : exists vals', runtime_getObj h' l0 = Some {| rt_type := C'; fields_map := vals' |}.
+              {
+                eapply runtime_preserves_r_type_heap with (h := h) (h' := h')(vals := values'); eauto.
+              }
+              destruct Hh'some as [vals'' Hh'some].
+              rewrite Hh'some in H4.
+              inversion H4; subst.
+              clear - Hh'some Hhsome H5 Hneq_k Hdom_root.
+              unfold update_field in Hh'some.
+              rewrite Hhsome in Hh'some.
+              simpl in Hh'some.
+              rewrite <- H5.
+              rewrite runtime_getObj_update_same in Hh'some; auto.
+              injection Hh'some as H_vals_eq.
+              rewrite <- H_vals_eq.
+              rewrite nth_error_update_neq; auto.
+          *
+            apply reachable_abs_step with (any := any) (C := C) (vals := vals) (k := k).
+            -- rewrite update_field_length in H3. exact H3.
+            -- (* Show runtime_getObj preserved for different location *)
+              unfold update_field in H4.
+              destruct (runtime_getObj h loc_x) eqn:Hgetx.
+              ++ rewrite runtime_getObj_update_diff in H4; auto.
+              ++ exact H4.
+            -- exact H5.
+            -- exact H6.
+            -- exact H7.
+        + (* reachable_abs_trans *)
+          eapply reachable_abs_trans with (l1:=l1).
+          * exact (IHHreach1 Hdom_root Hconfined).
+          *
+            eapply IHHreach2.
+            apply reachable_abs_dom in Hreach1.
+            rewrite update_field_length in Hreach1; auto.
+            eapply confinement_invariant_weaken; eauto.
+            exact (IHHreach1 Hdom_root Hconfined).
+    }
+ 
+    + (* Invariant preserved *)
+      inversion Htyping; subst sΓ'; subst.
+      unfold confinement_invariant_precise in *.
+      destruct Hconfined as [Henv_respects Hheap_respects].
+      split.
+      *
+        exact Henv_respects.
+      *
+        unfold heap_respects_protected_set.
+        intros l_src C anyrq vals k l_dst Hdom_dst Hlsrc_new Hin_dst Hobj_src Hnth.
+        unfold update_field in Hobj_src.
+
+        (* Case split on whether l_src = loc_x *)
+        destruct (Nat.eq_dec l_src loc_x) as [Heq | Hneq].
+        -- (* Case: l_src = loc_x (the written object) *)
+          subst l_src.
+          simpl in Hobj_src.
+          destruct (runtime_getObj h loc_x) eqn:Hobj_locx; try easy.
+          (* rewrite update_field_length in Hdom_src. *)
+          rewrite runtime_getObj_update_same in Hobj_src; auto.
+          apply runtime_getObj_dom in Hobj_locx; auto.
+          (* Now Hobj_src says that the updated object at loc_x has fields_map = update f val_y vals *)
+          (* injection Hobj_src as _ Hvals'_eq. *)
+          unfold heap_respects_protected_set in Hheap_respects.
+          apply runtime_getObj_dom in Hobj_locx; lia.
+        -- (* Case: l_src ≠ loc_x (different object) *)
+          have Heq : runtime_getObj (update_field h loc_x f val_y) l_src = runtime_getObj h l_src.
+          {
+            unfold update_field.
+            destruct (runtime_getObj h loc_x); try easy.
+            eapply runtime_getObj_update_diff; auto.
+          }
+          rewrite Heq in Hobj_src.
+          assert (dom (update_field h loc_x f val_y) = dom h).
+          {
+            apply update_field_length.
+          }
+          (* rewrite <- H3 in Hdom_src. *)
+          exact (Hheap_respects l_src C anyrq vals k l_dst Hdom_dst Hlsrc_new Hin_dst Hobj_src Hnth).
+  - (* new *)
+    split.
+    +
+    unfold protected_locset.
+    apply Ensembles.Extensionality_Ensembles.
+    unfold Ensembles.Same_set, Ensembles.Included.
+    split; intros l_target Hreach.
+    *
+      induction Hreach.
+      --
+        apply reachable_abs_heap.
+        rewrite length_app.
+        lia.
+      --
+        eapply reachable_abs_step with (C := C) (k := k) (vals := vals0) (any := any); eauto.
+        rewrite length_app. lia.
+        eapply runtime_getObj_app_left.
+        apply runtime_getObj_dom in H3; auto.
+        exact H3.
+      --
+        eapply reachable_abs_trans.
+        ---
+           apply IHHreach1.
+           +++ exact Hdom_root.
+           +++ exact Hconfined.
+        ---
+           apply IHHreach2.
+           +++ apply reachable_abs_dom in Hreach1. exact Hreach1.
+           +++ eapply confinement_invariant_weaken. exact Hreach1. exact Hconfined.
+    *
+    induction Hreach.
+    --
+      apply reachable_abs_heap.
+      exact Hdom_root.
+    -- 
+      eapply reachable_abs_step with (C := C) (k := k) (vals := vals0) (any := any); eauto.
+      assert (Hobj_l0_h: runtime_getObj h l0 =
+      Some
+      {|
+      rt_type :=
+      {|
+      rqtype := any; rctype :=
+      C
+      |};
+      fields_map := vals0
+      |}).
+      {
+        unfold runtime_getObj in *.
+        rewrite nth_error_app1 in H3.
+        --- exact Hdom_root.
+        --- (* Prove l0 < length h *)
+          exact H3.
+      }
+      unfold wf_r_config in Hwf.
+      destruct Hwf as [_ [HwfHeap [_ [_ [_ Hcorr]]]]].
+      unfold wf_heap in HwfHeap.
+      specialize (HwfHeap l0 Hdom_root).
+      unfold wf_obj in HwfHeap.
+      rewrite Hobj_l0_h in HwfHeap.
+      destruct HwfHeap as [Hwftype Hfields_wf].
+      destruct Hfields_wf as [fieldsCollection Hfield_types].
+      destruct Hfield_types as [HCollectFields Hfield_types].
+      destruct Hfield_types as [Hlength Hfield_types].
+      simpl in Hlength.
+      have HfieldDef: exists fDef, nth_error fieldsCollection k = Some fDef.
+      {
+        apply nth_error_Some_exists.
+        clear - H4 Hlength.
+        rewrite <- Hlength.
+        apply nth_error_Some.
+        rewrite H4.
+        discriminate.
+      }
+      destruct HfieldDef as [fDef HfieldDef].
+      eapply Forall2_nth_error with (i := k) (a := Iot l2) (b := fDef) in Hfield_types; eauto.
+      destruct (runtime_getObj h l2) eqn:Hobj_l2_h; try easy.
+      apply runtime_getObj_dom in Hobj_l2_h; auto.
+      unfold runtime_getObj in *.
+      rewrite nth_error_app1 in H3.
+      --- exact Hdom_root.
+      --- (* Prove l0 < length h *)
+        exact H3.
+    --
+      have Hreach1_orig : reachable_abs CT h l0 l2 := IHHreach1 Hdom_root Hconfined.
+      have Hdom_l2 : l2 < dom h := reachable_abs_dom CT h l0 l2 Hreach1_orig.
+      have Hconf_l2 : confinement_invariant_precise (protected_locset CT h l2) CT sΓ rΓ h h :=
+        confinement_invariant_weaken CT sΓ rΓ h h l0 l2 Hreach1_orig Hconfined.
+      have Hreach2_orig : reachable_abs CT h l2 l3 := IHHreach2 Hdom_l2 Hconf_l2.
+      exact (reachable_abs_trans CT h l0 l2 l3 Hreach1_orig Hreach2_orig).   
+    + (* Invariant preserved *)
+      inversion Htyping; subst sΓ'; subst.
+      unfold confinement_invariant_precise in *.
+      destruct Hconfined as [Henv_respects Hheap_respects].
+      split.
+      *
+        unfold env_respects_protected_set in *.
+        intros y l_y Ty Hlookup_s Hlookup_r Hin_P.
+        assert (rΓ <| vars := update x (Iot dom h) (vars rΓ) |> = update_r_env_value rΓ x (Iot (dom h))).
+        {
+          destruct rΓ.
+          reflexivity.
+        }
+        rewrite H2 in Hlookup_r.
+        destruct (Nat.eq_dec x y); subst.
+        -- (* y = x *)
+        rewrite runtime_getVal_update_same in Hlookup_r; auto.
+        apply static_getType_dom in Hlookup_s.
+        unfold wf_r_config in Hwf.
+        destruct Hwf as [_ [_[_ [_ [Hlen _]]]]].
+        rewrite Hlen in Hlookup_s.
+        exact Hlookup_s.
+        unfold protected_locset in Hin_P.
+        apply reachable_abs_dom in Hin_P.
+        inversion Hlookup_r; subst l_y.
+        lia.
+        -- (* y <> x *)
+        rewrite runtime_getVal_update_diff in Hlookup_r; auto.
+        eapply Henv_respects; eauto.
+      *
+        unfold heap_respects_protected_set.
+        intros l_src C anyrq vals0 k l_dst Hdom_dst Hlsrc_new Hin_dst Hobj_src Hnth.
+        (* Split into cases: is l_src the new object or an old object? *)
+        destruct (Nat.eq_dec l_src (dom h)) as [Heq_new | Hne_old].
+        -- (* Case: l_src = dom h (the newly created object) *)
+          (* subst l_src. *)
+          (* The new object is at the end of the heap *)
+          rewrite Heq_new in Hobj_src.
+          have Hobj_src_copy := Hobj_src.
+          rewrite runtime_getObj_last in Hobj_src; auto.
+          injection Hobj_src as _ Hfields_eq.
+          subst vals0.
+          subst c.
+          have hwf_constructor: wf_constructor CT C consig.
+          {
+            eapply constructor_lookup_wf; eauto.
+            destruct Hwf as [Hclasstable [_ [_ [_ [Hlen Htypable]]]]]; auto.
+            unfold constructor_sig_lookup in H10.
+            unfold constructor_def_lookup in H10.
+            destruct (find_class CT C) eqn: HfindC; try discriminate.
+            apply find_class_dom in HfindC; auto.
+          }
+          remember (h ++
+          [{|
+          rt_type :=
+          {| rqtype := vpa_mutabilty_object_creation qthisr (cqualifier consig);
+          rctype := C |};
+          fields_map := vals
+          |}]) as h'.
+          have hlsrc_domneq : l_src >= dom h by lia.
+          unfold wf_constructor in hwf_constructor.
+          destruct hwf_constructor as [Hbound [Hwf_constructor_params Hparam_count]].
+          destruct Hparam_count as [HfieldCollection HparameterFieldSubtyping].
+          destruct HparameterFieldSubtyping as [HCollectFields HparameterFieldSubtyping].
+          destruct HparameterFieldSubtyping as [Hlength HparameterFieldSubtyping].
+          unfold env_respects_protected_set in Henv_respects.
+          assert (Hdomeq: dom vals = dom argtypes).
+          {
+            apply runtime_lookup_list_preserves_length in H0.
+            apply static_getType_list_preserves_length in H8.
+            rewrite <- H0 in H8.
+            symmetry.
+            exact H8.
+          }
+          assert (Hk_bound : k < List.length argtypes).
+          {
+            assert (k < List.length vals).
+            apply nth_error_Some.
+            rewrite Hnth.
+            discriminate.
+            rewrite <- Hdomeq.
+            exact H2.
+          }
+          assert (Harg_type : exists argtype, nth_error argtypes k = Some argtype).
+          {
+            apply nth_error_Some_exists.
+            exact Hk_bound.
+          }
+          destruct Harg_type as [argtype Hargtype].
+          assert (HargtypeFromsEnv :
+            exists iArgInSenv,
+              nth_error sΓ iArgInSenv = Some argtype
+          /\ nth_error ys k = Some iArgInSenv).
+          {
+            destruct (static_getType_list_nth_zs sΓ ys argtypes k argtype H8 Hargtype)
+              as [j [Hzs_j Hst_j]].
+            exists j.
+            split.
+            - (* from static_getType to nth_error sΓ' *)
+              unfold static_getType in Hst_j; exact Hst_j.
+            - (* keep the zs fact *)
+              exact Hzs_j.
+          }
+          destruct HargtypeFromsEnv as [iArgInSenv [HargtypeFromsEnv Hzs_iArg]].
+
+          assert (Hi'dom : iArgInSenv < dom sΓ).
+          {
+            apply nth_error_Some.
+            rewrite HargtypeFromsEnv; discriminate.
+          }
+          assert (HargtypeFromrEnv :
+                    nth_error (vars rΓ) iArgInSenv = Some (Iot l_dst)).
+          {
+            destruct (runtime_lookup_list_nth_zs rΓ ys vals k (Iot l_dst) H0 Hnth)
+              as [j [Hzs_j Hget_j]].
+            assert (HiEq : iArgInSenv = j).
+            {
+              (* zs[i'] = Some iArgInSenv and zs[i'] = Some j ⇒ iArgInSenv = j *)
+              rewrite Hzs_iArg in Hzs_j.
+              inversion Hzs_j; reflexivity.
+            }
+            subst iArgInSenv.
+            unfold runtime_getVal in Hget_j.
+            exact Hget_j.
+          } 
+          have Hnth_param : exists param_type, nth_error (cparams consig) k = Some param_type.
+          {
+            apply Forall2_length in H16.
+            apply nth_error_Some_exists.
+            rewrite <- H16.
+            exact Hk_bound.
+          }
+          destruct Hnth_param as [param_type Hparam_type].
+          specialize (Henv_respects iArgInSenv l_dst argtype HargtypeFromsEnv HargtypeFromrEnv Hin_dst).
+          eapply Forall2_nth_error in H16; eauto.
+          assert (is_safe_mode (sqtype param_type)).
+          {
+            eapply subtype_safe_implies_safe with (CT:= CT) (T_sub := argtype); eauto.
+          }
+          have [fdef Hfdef] : exists fdef, nth_error HfieldCollection k = Some fdef.
+          {
+            apply nth_error_Some_exists.
+            apply nth_error_Some in Hk_bound.
+            rewrite <- Hlength.
+            apply nth_error_Some.
+            rewrite Hparam_type; discriminate.
+          }
+          apply Forall2_nth_error with (i:=k) (a:=param_type) (b:=fdef) in HparameterFieldSubtyping; auto.
+          unfold vpa_mutabilty_constructor_fld in HparameterFieldSubtyping.
+          destruct (mutability (ftype fdef)) eqn:Hfld_mut;
+          exists fdef;
+          split;
+          unfold sf_def_rel;
+          try exact (FL_Found CT C HfieldCollection k fdef HCollectFields Hfdef).
+          all: destruct (cqualifier consig) eqn: Hconsig_qual.
+          all: unfold is_safe_mode in H2;
+          apply qualified_type_subtype_q_subtype in HparameterFieldSubtyping;
+          destruct H2 as [Hrd | Hlost].
+          all: try rewrite Hrd in HparameterFieldSubtyping; try inversion HparameterFieldSubtyping; try discriminate.
+          all: try rewrite Hlost in HparameterFieldSubtyping; try inversion HparameterFieldSubtyping; try discriminate.
+          all: try exact Hfld_mut.
+        -- (* Case: l_src < dom h (old object, not the new one) *)
+          (* Heap grew but old objects unchanged *)
+          remember ({| rt_type := {| rqtype := vpa_mutabilty_object_creation qthisr (cqualifier consig); rctype := c |}; fields_map := vals |}) as newobject.
+          assert (l_src < dom h).
+          {
+            (* Extract l_src < dom (h ++ [new_obj]) from Hobj_src *)
+            have Hdom_appended : l_src < dom (h ++ [newobject]).
+            {
+              eapply runtime_getObj_dom; exact Hobj_src.
+            }
+            (* Now simplify: dom (h ++ [obj]) = dom h + 1 *)
+            rewrite length_app in Hdom_appended.
+            simpl in Hdom_appended.
+            (* l_src < dom h + 1 and l_src <> dom h imply l_src < dom h *)
+            lia.
+          }
+          (* Now show that old objects weren't modified *)
+          have Hobj_src_old : runtime_getObj h l_src = runtime_getObj (h ++ [newobject]) l_src.
+          {
+            eapply runtime_getObj_app_left_equal.
+            exact H2.
+          }
+          rewrite <- Hobj_src_old in Hobj_src.
+          exact (Hheap_respects l_src C anyrq vals0 k l_dst Hdom_dst Hlsrc_new Hin_dst Hobj_src Hnth).
+  - (* call *)
+    inversion Htyping; subst sΓ'; subst.
+    have Hwfcopy := Hwf.
+    unfold wf_r_config in Hwf.
+    destruct Hwf as [Hclasstable [Hheap [Hrenv [Hsenv [Henv_len Htypable]]]]].
+    unfold confinement_invariant_precise in *.
+    destruct Hconfined as [Henv_respects Hheap_respects].
+    specialize (IHHeval Hdom_root (eq_refl)).
+    destruct H1 as [mdeflookup getmbody].
+    remember (msignature mdef) as msig.
+    inversion mdeflookup; revert getmbody; subst; intro getmbody.
+    +
+    assert (Hwfmethod: wf_method CT cy mdef).
+    {
+      eapply method_lookup_wf_class; eauto.
+      eapply r_basetype_in_dom; eauto.
+      unfold gget_method in H3.
+      apply find_some in H3.
+      destruct H3.
+      exact H2.
+    }
+    unfold wf_method in Hwfmethod;
+    destruct Hwfmethod as [sΓmethodend [mbodyreturntype [Hmethodbody_typing [HmethodReturnBound [HmethodReturnType [HmethodReturnSubtype HMethodoverride]]]]]];
+    remember (mreceiver (msignature mdef) :: mparams (msignature mdef)) as sΓmethodinit;
+    remember {| vars := Iot ly :: vals |} as rΓmethodinit;
+    remember (rΓ <| vars := update x retval (vars rΓ) |>) as rΓ'''.
+    assert(Hwf_method_frame : wf_r_config CT sΓmethodinit rΓmethodinit h).
+    {
+      (* Method inner config wellformed.*)
+        have Hclass := Hclasstable.
+        unfold  wf_class_table in Hclass.
+        destruct Hclass as [Hclass [Hobjexist [Hotherclasses Hcname_consistent]]].
+        repeat split.
+        exact Hclass.
+        exact Hobjexist.
+        exact Hotherclasses.
+        apply Hcname_consistent.
+        apply Hcname_consistent.
+        exact Hheap.
+        rewrite HeqrΓmethodinit.
+        simpl.
+        lia.
+        unfold wf_renv in Hrenv.
+        destruct Hrenv as [HrEnvLen [Hreceiverval Hallvals]].
+        exists ly.
+        split.
+        rewrite HeqrΓmethodinit.
+        simpl.
+        reflexivity.
+        unfold runtime_getVal in H.
+        destruct (nth_error (vars rΓ) y) as [v|] eqn:Hnth_y; [|discriminate].
+        injection H as H1_eq.
+        subst v.
+        eapply Forall_nth_error in Hallvals; eauto.
+        simpl in Hallvals.
+        destruct (runtime_getObj h ly) as [obj|] eqn:Hobjly; [|contradiction].
+        apply runtime_getObj_dom in Hobjly.
+        exact Hobjly.
+
+        (* Inner runtime env is wellformed *)
+        rewrite HeqrΓmethodinit.
+        simpl.
+        constructor.
+        simpl.
+        unfold runtime_getVal in H.
+        destruct (nth_error (vars rΓ) y) as [v|] eqn:Hnth_y; [|discriminate].
+        injection H as H1_eq.
+        subst v.
+        unfold runtime_getVal in Hnth_y.
+        unfold wf_renv in Hrenv.
+        destruct Hrenv as [_ [_ Hallvals]].
+        eapply Forall_nth_error in Hallvals; eauto.
+        simpl in Hallvals.
+        exact Hallvals.
+        eapply runtime_lookup_list_preserves_wf_values; eauto.
+
+        (* Inner Static Environment's length is more than 0 *)
+        rewrite HeqsΓmethodinit.
+        simpl.
+        lia.
+
+        (* Inner static env's elements are wellformed typeuse *)
+        rewrite HeqsΓmethodinit.
+        constructor.
+        (* subst.
+        assert (parent < dom CT). {
+          assert (cy < dom CT). {
+            eapply find_class_dom; eauto.
+          }
+          assert (parent < cy). {
+            eapply parent_implies_strict_ordering with (C:= cy) (D:=parent); eauto.
+          }
+          lia.
+        } *)
+
+        (* Receiver type is well-formed *)
+        eapply method_sig_wf_receiver_by_find; eauto.
+        assert (Hcydom: cy < dom CT). {
+            eapply find_class_dom; eauto.
+        }
+        exact Hcydom.
+        (* assert (parent < dom CT). {
+          assert (cy < dom CT). {
+            eapply find_class_dom; eauto.
+          }
+          assert (parent < cy). {
+            eapply parent_implies_strict_ordering with (C:= cy) (D:=parent); eauto.
+          }
+          lia.
+        } *)
+        eapply method_sig_wf_parameters_by_find; eauto.
+        assert (Hcydom: cy < dom CT). {
+            eapply find_class_dom; eauto.
+        }
+        exact Hcydom.
+
+        apply static_getType_list_preserves_length in H11.
+        apply runtime_lookup_list_preserves_length in H4.
+        rewrite HeqsΓmethodinit.
+        rewrite HeqrΓmethodinit.
+        simpl.
+        f_equal.
+        apply Forall2_length in H20.
+        assert (Hy_dom : y < dom sΓ).
+        {
+          apply static_getType_dom in H10.
+          exact H10.
+        }
+        assert (HOutterReceiverAddr: exists lOutterReceiver, get_this_var_mapping (vars rΓ) = Some lOutterReceiver).
+        {
+          eapply get_this_exists_from_wf_r_config; eauto.
+
+        }
+        destruct HOutterReceiverAddr as [lOutterReceiver HOutterReceiverAddr].
+        assert (HOutterReceiverMutability: exists qcontext, r_muttype h lOutterReceiver = Some qcontext).
+        {
+          eapply receiver_mutability_exists_wf_renv; eauto.
+        }
+        destruct HOutterReceiverMutability as [OutterReceiverMutability HOutterReceiverMutabilityType].
+        have Hcorr := Htypable.
+        have Hcorrcopy := Hcorr.
+        specialize (Hcorr lOutterReceiver OutterReceiverMutability HOutterReceiverAddr HOutterReceiverMutabilityType y Hy_dom Ty H10).
+        unfold wf_r_typable in Hcorr.
+        unfold r_basetype in H0.
+        unfold r_type.
+        destruct (runtime_getObj h ly) as [obj|] eqn:Hobjy; [|discriminate].
+        injection H0 as Hcy_eq.
+        subst cy.
+        destruct obj as [rt_obj fields_obj].
+        destruct rt_obj as [rq_obj rc_obj].
+
+        unfold wf_renv in Hrenv.
+        destruct Hrenv as [_ [Hreceiver _]].
+        destruct Hreceiver as [iot [Hget_iot _]].
+        unfold get_this_var_mapping.
+        unfold gget in Hget_iot.
+        destruct (vars rΓ) as [|v0 vs] eqn:Hvars; [discriminate|].
+
+        unfold r_type in Hcorr.
+        rewrite H in Hcorr.
+        rewrite Hobjy in Hcorr.
+        simpl in Hcorr.
+        destruct Hcorr as [Hbasesubtype HyQualifierTypablility].
+        assert (msignature mdef = msignature mdef0).
+        {
+          eapply method_signature_consistent_subtype; eauto.
+        }
+        rewrite H0.
+        rewrite H4.
+        rewrite <- H20.
+        exact H11.
+
+        (* Correspondence holds for inner environment *)
+        intros ι qinner HreceiverAddr Hqcontext i Hi sqt Hnth.
+        rewrite HeqsΓmethodinit in Hnth, Hi.
+        rewrite HeqrΓmethodinit.
+        simpl in *.
+        assert (Hy_dom : y < dom sΓ).
+        {
+          apply static_getType_dom in H10.
+          exact H10.
+        }
+        assert (HOutterReceiverAddr: exists lOutterReceiver, get_this_var_mapping (vars rΓ) = Some lOutterReceiver).
+        {
+          eapply get_this_exists_from_wf_r_config; eauto.
+        }
+        destruct HOutterReceiverAddr as [lOutterReceiver HOutterReceiverAddr].
+        assert (HOutterReceiverMutability: exists qcontext, r_muttype h lOutterReceiver = Some qcontext).
+        {
+          eapply receiver_mutability_exists_wf_renv; eauto.
+        }
+        destruct HOutterReceiverMutability as [OutterReceiverMutability HOutterReceiverMutabilityType].
+        have Hcorr := Htypable.
+        have Hcorrcopy := Hcorr.
+        specialize (Hcorr lOutterReceiver OutterReceiverMutability HOutterReceiverAddr HOutterReceiverMutabilityType y Hy_dom Ty H10).
+        unfold wf_r_typable in Hcorr.
+        unfold r_basetype in H0.
+        unfold r_type.
+        destruct (runtime_getObj h ly) as [obj|] eqn:Hobjy; [|discriminate].
+        injection H0 as Hcy_eq.
+        subst cy.
+        destruct obj as [rt_obj fields_obj].
+        destruct rt_obj as [rq_obj rc_obj].
+
+        have Hrenvcopy := Hrenv.
+        unfold wf_renv in Hrenv.
+        destruct Hrenv as [_ [Hreceiver _]].
+        destruct Hreceiver as [iot [Hget_iot _]].
+        unfold get_this_var_mapping.
+        unfold gget in Hget_iot.
+        destruct (vars rΓ) as [|v0 vs] eqn:Hvars; [discriminate|].
+
+        unfold r_type in Hcorr.
+        rewrite H in Hcorr.
+        rewrite Hobjy in Hcorr.
+        simpl in Hcorr.
+        destruct Hcorr as [Hbasesubtype HyQualifierTypablility].
+        
+        assert (Hmsigeq: msignature mdef = msignature mdef0).
+        {
+          eapply method_signature_consistent_subtype; eauto.
+        }
+        destruct i as [|i'].
+
+        (* Reciever index - 0 *)
+        simpl in Hnth.
+        injection Hnth as Hsqt_eq.
+        subst sqt.
+        simpl.
+        unfold wf_r_typable.
+        unfold r_type.
+
+        rewrite Hobjy.
+        simpl.
+        split.
+
+        (* Base type subtyping *)
+        rewrite Hmsigeq.
+        apply qualified_type_subtype_base_subtype in H19.
+        (* rewrite (vpa_mutabilty_tt_sctype Tthis Ty) in H23. *)
+        rewrite (vpa_mutabilty_tt_sctype Ty (mreceiver (msignature mdef0))) in H19.
+        eapply base_trans; eauto.
+
+        (* Qualifier typbility *)
+        1: 
+        {
+          apply qualified_type_subtype_q_subtype in H19.
+          specialize (Hcorrcopy lOutterReceiver OutterReceiverMutability HOutterReceiverAddr HOutterReceiverMutabilityType).
+          apply get_this_qualified_type_nth_error in H12.
+          unfold wf_senv in Hsenv.
+          destruct Hsenv as [Hsenvdom _].
+          specialize (Hcorrcopy 0 Hsenvdom Tthis H12).
+          rewrite <- Hvars in HOutterReceiverAddr.
+          apply get_this_var_mapping_runtime_getVal in HOutterReceiverAddr.
+          rewrite HOutterReceiverAddr in Hcorrcopy.
+          unfold wf_r_typable in Hcorrcopy.
+          unfold r_type in Hcorrcopy.
+          destruct (runtime_getObj h lOutterReceiver) as [outterreceiverobj|] eqn:Houtterobj; [|easy].
+          destruct Hcorrcopy as [_ Houtter_qualifier_typable].
+
+          assert (rqtype (rt_type outterreceiverobj) = OutterReceiverMutability).
+          {
+            unfold r_muttype in HOutterReceiverMutabilityType.
+            rewrite Houtterobj in HOutterReceiverMutabilityType.
+            simpl in HOutterReceiverMutabilityType.
+            inversion HOutterReceiverMutabilityType; subst OutterReceiverMutability.
+            reflexivity.
+          }
+          subst OutterReceiverMutability.
+
+          assert (ly = ι). 
+          {
+            rewrite HeqrΓmethodinit in HreceiverAddr.
+            unfold get_this_var_mapping in HreceiverAddr.
+            simpl in HreceiverAddr.
+            inversion HreceiverAddr; reflexivity.
+          }
+          subst ι.
+
+          assert (r_muttype h ly = Some rq_obj).
+          {
+            unfold r_muttype.
+            rewrite Hobjy.
+            simpl.
+            reflexivity.
+          }
+
+          assert (rq_obj = qinner).
+          {
+            rewrite H0 in Hqcontext.
+            inversion Hqcontext; subst qinner.
+            reflexivity.
+          }
+          subst rq_obj.
+
+          unfold qualifier_typable_context.
+          unfold qualifier_typable_context in HyQualifierTypablility.
+          unfold qualifier_typable_context in Houtter_qualifier_typable.
+          unfold vpa_mutabilty_rs.
+          unfold vpa_mutabilty_rs in HyQualifierTypablility.
+          unfold vpa_mutabilty_rs in Houtter_qualifier_typable.
+          unfold vpa_mutabilty_tt in H19.
+          rewrite <- Hmsigeq in H19.
+
+          destruct qinner eqn:HInnerReceiverMutability;
+          destruct (sqtype (mreceiver (msignature mdef))) eqn:HMethodReceiverDeclaredType;
+          try trivial.
+          all: destruct (rqtype (rt_type outterreceiverobj)) eqn:HOutterReceiverMutability;
+          destruct (sqtype Ty) eqn:HTyStaticMutability;
+          try trivial.
+          all: destruct (sqtype Tthis) eqn:HTthisStaticMutability;
+          try rewrite HTyStaticMutability in H19;
+          simpl in H19;
+          try rewrite HMethodReceiverDeclaredType in H19;
+          try inversion H19; try trivial.
+          all: try inversion H19; try easy.
+        }
+        (* clear_dups. amazing.... *)
+
+  (* -------------------------------------------------- *)
+  (* Other index - > 1 *)
+        apply qualified_type_subtype_q_subtype in H18.
+        unfold runtime_getVal.
+        simpl.
+        destruct (nth_error vals i') as [v|] eqn:Hval_i.
+          - (* Parameter i' exists *)
+            destruct v as [|loc]; [trivial|].
+            (* Use H23 to get the subtyping relationship *)
+            assert (Hi'_bound : i' < List.length argtypes).
+            {
+              apply Forall2_length in H20.
+              simpl in Hi.
+              simpl in Hnth.
+              rewrite Hmsigeq in Hnth.
+              rewrite H20.
+              apply nth_error_Some.
+              intros Hnone.
+              rewrite Hnth in Hnone.
+              discriminate.
+            }
+            assert (Harg_type : exists argtype, nth_error argtypes i' = Some argtype).
+            {
+              apply nth_error_Some_exists.
+              exact Hi'_bound.
+            }
+            assert (loc < dom h).
+            {
+              assert (Hvals_wf :
+              Forall
+                (fun v =>
+                  match v with
+                  | Null_a => True
+                  | Iot loc =>
+                      match runtime_getObj h loc with
+                      | Some _ => True
+                      | None => False
+                      end
+                  end) vals).
+              {
+                eapply runtime_lookup_list_preserves_wf_values; eauto.
+              }
+              eapply Forall_nth_error in Hvals_wf; eauto.
+              simpl in Hvals_wf.
+              destruct (runtime_getObj h loc) as [argobj|] eqn:Hargobjloc; [|contradiction].
+              apply runtime_getObj_dom in Hargobjloc.
+              exact Hargobjloc.
+            }
+            destruct Harg_type as [argtype Hargtype].
+            unfold wf_r_typable.
+            unfold r_type.
+            destruct (runtime_getObj h loc) as [argobj|] eqn:Hargobjloc; [|apply runtime_getObj_not_dom in Hargobjloc; lia].
+            assert (HargtypeFromsEnv :
+              exists iArgInSenv,
+                nth_error sΓ iArgInSenv = Some argtype
+            /\ nth_error zs i' = Some iArgInSenv).
+            {
+              destruct (static_getType_list_nth_zs sΓ zs argtypes i' argtype H11 Hargtype)
+                as [j [Hzs_j Hst_j]].
+              exists j.
+              split.
+              - (* from static_getType to nth_error sΓ' *)
+                unfold static_getType in Hst_j; exact Hst_j.
+              - (* keep the zs fact *)
+                exact Hzs_j.
+            }
+            destruct HargtypeFromsEnv as [iArgInSenv [HargtypeFromsEnv Hzs_iArg]].
+
+            assert (Hi'dom : iArgInSenv < dom sΓ).
+            {
+              apply nth_error_Some.
+              rewrite HargtypeFromsEnv; discriminate.
+            }
+            assert (HargtypeFromrEnv :
+                      nth_error (vars rΓ) iArgInSenv = Some (Iot loc)).
+            {
+              destruct (runtime_lookup_list_nth_zs rΓ zs vals i' (Iot loc) H4 Hval_i)
+                as [j [Hzs_j Hget_j]].
+              assert (HiEq : iArgInSenv = j).
+              {
+                (* zs[i'] = Some iArgInSenv and zs[i'] = Some j ⇒ iArgInSenv = j *)
+                rewrite Hzs_iArg in Hzs_j.
+                inversion Hzs_j; reflexivity.
+              }
+              subst iArgInSenv.
+              unfold runtime_getVal in Hget_j.
+              exact Hget_j.
+            }
+            have Hcorrcopy_2 := Hcorrcopy.
+            specialize (Hcorrcopy lOutterReceiver OutterReceiverMutability HOutterReceiverAddr HOutterReceiverMutabilityType iArgInSenv Hi'dom argtype HargtypeFromsEnv).
+            unfold runtime_getVal in Hcorrcopy.
+            rewrite HargtypeFromrEnv in Hcorrcopy.
+            unfold wf_r_typable in Hcorrcopy.
+            unfold r_type in Hcorrcopy.
+            rewrite Hargobjloc in Hcorrcopy.
+            destruct Hcorrcopy as [Harg_basesubtype Harg_qualifiertypability].
+            split.
+
+            (* base subtype *)
+            rewrite nth_error_cons_succ in Hnth.
+            rewrite Hmsigeq in Hnth.
+            eapply Forall2_nth_error in H20; eauto.
+            apply qualified_type_subtype_base_subtype in H20.
+            rewrite (vpa_mutabilty_tt_sctype Ty sqt) in H20.
+            eapply base_trans; eauto.
+
+            (* Qualifier Typability *)
+            rewrite Hmsigeq in Hnth.
+            eapply Forall2_nth_error in H20; eauto.
+            apply qualified_type_subtype_q_subtype in H20.
+            rewrite sq_vpa_tt_eq_qq in H20.
+            specialize (Hcorrcopy_2 lOutterReceiver OutterReceiverMutability HOutterReceiverAddr HOutterReceiverMutabilityType).
+            unfold wf_senv in Hsenv.
+            destruct Hsenv as [Hsenvdom _].
+            apply get_this_qualified_type_nth_error in H12.
+            specialize (Hcorrcopy_2 0 Hsenvdom Tthis H12).
+            rewrite <- Hvars in Hget_iot.
+            apply get_this_var_mapping_runtime_getVal in Hget_iot.
+            rewrite Hget_iot in Hcorrcopy_2.
+            unfold wf_r_typable in Hcorrcopy_2.
+            unfold r_type in Hcorrcopy_2.
+            destruct (runtime_getObj h iot) as [outterreceiverobj|] eqn:Houtterobj; [|easy].
+            destruct Hcorrcopy_2 as [_ HOutterReceiverQualifierTypablility].
+            assert (rqtype (rt_type outterreceiverobj) = OutterReceiverMutability).
+            {
+              clear - Houtterobj HOutterReceiverMutabilityType HOutterReceiverAddr Hget_iot Hvars.
+              rewrite <- Hvars in HOutterReceiverAddr.
+              apply get_this_var_mapping_runtime_getVal in HOutterReceiverAddr.
+              rewrite Hget_iot in HOutterReceiverAddr.
+              inversion HOutterReceiverAddr; subst lOutterReceiver.
+              unfold r_muttype in HOutterReceiverMutabilityType.
+              rewrite Houtterobj in HOutterReceiverMutabilityType.
+              simpl in HOutterReceiverMutabilityType.
+              inversion HOutterReceiverMutabilityType; reflexivity.
+            }
+            subst OutterReceiverMutability.
+            assert (ι = ly).
+            {
+              unfold get_this_var_mapping in HreceiverAddr.
+              rewrite HeqrΓmethodinit in HreceiverAddr.
+              simpl in HreceiverAddr.
+              inversion HreceiverAddr; reflexivity.
+            }
+            subst ι.
+            assert(rq_obj = qinner).
+            {
+              unfold r_muttype in Hqcontext.
+              rewrite Hobjy in Hqcontext.
+              simpl in Hqcontext.
+              inversion Hqcontext.
+              easy.
+            }
+            subst rq_obj.
+            clear - H20 Harg_qualifiertypability HyQualifierTypablility HOutterReceiverQualifierTypablility.
+
+            destruct (rqtype (rt_type argobj)) eqn:Hargobjmutability; move Hargobjmutability at bottom;
+            destruct (sqtype sqt) eqn:HParameterStaticDeclearedMutability; move HParameterStaticDeclearedMutability at bottom;
+            destruct qinner eqn:HInnerReceiverMutability; move HInnerReceiverMutability at bottom;
+            try solve_qualifier_typable_correct_concrete.
+
+            all: destruct (sqtype Ty) eqn:HTyStaticMutability;
+            destruct (sqtype argtype) eqn:HArgTypeStaticMutability;
+            simpl in H20;
+            try solve_q_subtype_wrong.
+
+            all: 
+            destruct (rqtype (rt_type outterreceiverobj)) eqn:HOutterReceiverMutability;
+            try solve_qualifier_typable_wrong_concrete.
+
+          - (* Parameter i' doesn't exist - contradiction *)
+            exfalso.
+            apply nth_error_None in Hval_i.
+            apply runtime_lookup_list_preserves_length in H4.
+            apply static_getType_list_preserves_length in H11.
+            apply Forall2_length in H20.
+            rewrite H4 in Hval_i.
+            rewrite <- H11 in Hval_i.
+            rewrite H20 in Hval_i.
+            simpl in Hi.
+            simpl in Hnth.
+            rewrite <- Hmsigeq in Hval_i.
+            lia.
+    }
+    specialize (IHHeval Heval sΓmethodend sΓmethodinit).
+    assert (HenvInvariant: env_respects_protected_set (protected_locset CT h l_root)
+    sΓmethodinit rΓmethodinit).
+    {
+      unfold env_respects_protected_set.
+      intros z l_z Tz Hlookup_s Hlookup_r Hin_P.
+      rewrite HeqsΓmethodinit in Hlookup_s.
+      rewrite HeqrΓmethodinit in Hlookup_r.
+      unfold static_getType in Hlookup_s.
+      unfold runtime_getVal in Hlookup_r.
+      simpl in Hlookup_s, Hlookup_r.
+      destruct z as [| z'].
+      - simpl in Hlookup_s, Hlookup_r.
+      injection Hlookup_s as <-. injection Hlookup_r as <-.
+      unfold is_safe_mode.
+      have Hty_safe : is_safe_mode (sqtype Ty).
+      {
+        unfold env_respects_protected_set in Henv_respects.
+        specialize (Henv_respects y ly Ty H10 H Hin_P).
+        exact Henv_respects.
+      }
+      unfold is_safe_mode in Hty_safe.
+      unfold vpa_mutabilty_tt.
+      apply qualified_type_subtype_q_subtype in H19.
+      clear - Hty_safe H19.
+      unfold vpa_mutabilty_tt in H19.
+      destruct Hty_safe as [HRd | HLost].
+      + (* Case: sqtype Ty = Rd *)
+        rewrite HRd in H19.
+        simpl in H19.
+        inversion H19; easy.
+      + (* Case: sqtype Ty = Lost *)
+        rewrite HLost in H19.
+        simpl in H19.
+        inversion H19; easy.
+      -
+        assert (Hy_dom : y < dom sΓ).
+        {
+          apply static_getType_dom in H10.
+          exact H10.
+        }
+
+        unfold wf_renv in Hrenv.
+        destruct Hrenv as [_ [Hreceiver _]].
+        destruct Hreceiver as [iot [Hget_iot Hiot_dom]].
+        assert (HOutterReceiverMutability: exists qcontext, r_muttype h iot = Some qcontext).
+        {
+          eapply receiver_mutability_exists_from_bound; eauto.
+        }
+        destruct HOutterReceiverMutability as [qoutter Hqoutter].
+        (* Apply correspondence to get wf_r_typable *)
+        specialize (Htypable iot qoutter Hget_iot Hqoutter y Hy_dom Ty H10).
+        unfold wf_r_typable in Htypable.
+        unfold r_basetype in H1.
+        unfold r_type.
+        destruct (runtime_getObj h ly) as [obj|] eqn:Hobjy.
+        2:{
+          unfold r_basetype in H0.
+          rewrite Hobjy in H0.
+          discriminate.
+        }
+        destruct obj as [rt_obj fields_obj].
+        destruct rt_obj as [rq_obj rc_obj].
+
+        unfold r_type in Htypable.
+        rewrite H in Htypable.
+        rewrite Hobjy in Htypable.
+        simpl in Htypable.
+        destruct Htypable as [Hsubtype Hqualifier].
+        simpl in Hobjy.
+
+        simpl in H1.
+        inversion H1.
+        assert (Hrc_obj_eq: rc_obj = cy).
+        {
+          unfold r_basetype in H0.
+          rewrite Hobjy in H0.
+          inversion H0.
+          easy.
+        }
+        subst rc_obj.
+        assert (Hsigeq: msignature mdef = msignature mdef0).
+        {
+          eapply method_signature_consistent_subtype; eauto.
+        }
+        have Hnth_param_type : nth_error (mparams (msignature mdef)) z' = Some Tz.
+        {
+          simpl in Hlookup_s.
+          easy.
+        }
+
+        have Hnth_param_val : nth_error vals z' = Some (Iot l_z).
+        {
+          simpl in Hlookup_r.
+          easy.
+        }
+        assert (Hi'_bound : z' < List.length argtypes).
+        {
+          apply Forall2_length in H20.
+          rewrite <- Hsigeq in H20.
+          assert (H_bound_params : z' < dom (mparams (msignature mdef))).
+          {
+            apply nth_error_Some. (* Converts "index < len" to "lookup <> None" *)
+            rewrite Hnth_param_type.   (* lookup is Some Tz *)
+            discriminate.         (* Some <> None *)
+          }
+
+          (* 2. Convert to bound for argtypes using the equality *)
+          rewrite <- H20 in H_bound_params. (* Replace length of params with length of argtypes *)
+
+          (* 3. Solve the goal *)
+          exact H_bound_params.
+        }
+
+        have Hnth_arg: exists T_arg, nth_error argtypes z' = Some T_arg.
+        {
+          apply nth_error_Some_exists.
+          exact Hi'_bound.
+        }
+
+        destruct Hnth_arg as [T_arg Hnth_arg].
+        eapply Forall2_nth_error with (i := z') (a := T_arg) (b := Tz) in H20; [|auto|rewrite <- Hsigeq; exact Hnth_param_type].
+        (* apply qualified_type_subtype_q_subtype in H20. *)
+        unfold env_respects_protected_set in Henv_respects.
+        apply adapated_subtype_safe_implies_safe in H20; auto.
+
+        have HargtypeFromsEnv :
+          exists z_outter,
+            static_getType sΓ z_outter = Some T_arg /\
+            nth_error zs z' = Some z_outter.
+        {
+          destruct (static_getType_list_nth_zs sΓ zs argtypes z' T_arg H11 Hnth_arg)
+            as [j [Hzs_j Hst_j]].
+          exists j.
+          split.
+          - unfold static_getType. exact Hst_j.
+          - exact Hzs_j.
+        }
+
+        destruct HargtypeFromsEnv as [z_outter [HgetZ_type Hzs_z_outter]].
+
+        have HgetZ_val : runtime_getVal rΓ z_outter = Some (Iot l_z).
+        {
+          destruct (runtime_lookup_list_nth_zs rΓ zs vals z' (Iot l_z) H4 Hnth_param_val)
+            as [j [Hzs_j Hget_j]].
+          assert (HzEq : z_outter = j) by (
+            rewrite Hzs_z_outter in Hzs_j;
+            inversion Hzs_j; reflexivity
+          ).
+          subst j.
+          exact Hget_j.
+        }
+        specialize (Henv_respects z_outter l_z T_arg HgetZ_type HgetZ_val Hin_P); auto.
+    }
+    assert (HMethodInnerInvariant: env_respects_protected_set (protected_locset CT h l_root)
+    sΓmethodinit rΓmethodinit /\ heap_respects_protected_set (protected_locset CT h l_root) h h CT).
+    {
+      split.
+      exact HenvInvariant.
+      exact Hheap_respects.
+    }
+    specialize (IHHeval HMethodInnerInvariant Hwf_method_frame).
+    rewrite <- getmbody in Hmethodbody_typing.
+    specialize (IHHeval Hmethodbody_typing).
+    destruct IHHeval as [Htopology Hconfinement].
+    destruct Hconfinement as [Henv_respects' Hheap_respects'].
+    split.
+    exact Htopology.
+    split.
+    assert (Henv_respects'': env_respects_protected_set (protected_locset CT h l_root) sΓ rΓ''' ).
+    {
+      rewrite HeqrΓ'''.
+      unfold env_respects_protected_set.
+      intros z l_z T_z Hlookup_s Hlookup_r Hin_P.
+      destruct (Nat.eq_dec x z); subst.
+      -- (* CASE: z = x (New Variable) *)
+        assert (T_z = Tx). 
+        {
+          rewrite H9 in Hlookup_s. 
+          injection Hlookup_s as H_eq_T. subst T_z.
+          reflexivity.
+        }
+        subst T_z.
+        unfold env_respects_protected_set in Henv_respects'.
+        have HGetMethodReturnType: static_getType sΓmethodend (mreturn (Syntax.mbody mdef)) = Some mbodyreturntype.
+        {
+          unfold static_getType; auto.
+        }
+        assert (Hy_dom : y < dom sΓ).
+        {
+          apply static_getType_dom in H10.
+          exact H10.
+        }
+
+        unfold wf_renv in Hrenv.
+        destruct Hrenv as [_ [Hreceiver _]].
+        destruct Hreceiver as [iot [Hget_iot Hiot_dom]].
+        assert (HOutterReceiverMutability: exists qcontext, r_muttype h iot = Some qcontext).
+        {
+          eapply receiver_mutability_exists_from_bound; eauto.
+        }
+        destruct HOutterReceiverMutability as [qoutter Hqoutter].
+        (* Apply correspondence to get wf_r_typable *)
+        specialize (Htypable iot qoutter Hget_iot Hqoutter y Hy_dom Ty H10).
+        unfold wf_r_typable in Htypable.
+        unfold r_basetype in H1.
+        unfold r_type.
+        destruct (runtime_getObj h ly) as [obj|] eqn:Hobjy.
+        2:{
+          unfold r_basetype in H0.
+          rewrite Hobjy in H0.
+          discriminate.
+        }
+        destruct obj as [rt_obj fields_obj].
+        destruct rt_obj as [rq_obj rc_obj].
+
+        unfold r_type in Htypable.
+        rewrite H in Htypable.
+        rewrite Hobjy in Htypable.
+        simpl in Htypable.
+        destruct Htypable as [Hsubtype Hqualifier].
+        simpl in Hobjy.
+
+        simpl in H1.
+        inversion H1.
+        assert (Hrc_obj_eq: rc_obj = cy).
+        {
+          unfold r_basetype in H0.
+          rewrite Hobjy in H0.
+          inversion H0.
+          easy.
+        }
+        subst rc_obj.
+        assert (Hsigeq: msignature mdef = msignature mdef0).
+        {
+          eapply method_signature_consistent_subtype; eauto.
+        }
+        have Hdom_z : z < dom (vars rΓ). 
+        { 
+          apply runtime_getVal_dom in Hlookup_r.
+          rewrite update_length in Hlookup_r.
+          exact Hlookup_r.
+        }
+        have Hlookup_r_copy := Hlookup_r.
+        unfold runtime_getVal in Hlookup_r.
+        rewrite update_same in Hlookup_r. lia.   (* or by exact Hdom_x *)
+        inversion Hlookup_r; subst.
+        specialize (Henv_respects' (mreturn (Syntax.mbody mdef)) l_z mbodyreturntype HGetMethodReturnType H6 Hin_P).
+        rewrite <- Hsigeq in H18.
+        apply subtype_safe_implies_safe in HmethodReturnSubtype; auto.
+        apply subtype_safe_implies_safe_adapted in H18; auto.
+      -- (* CASE: z <> x (Old Variables) *)
+      (* Just use the original invariant *)
+      assert (rΓ <| vars := update x retval (vars rΓ) |> = update_r_env_value rΓ x retval).
+      {
+        destruct rΓ.
+        reflexivity.
+      }
+      rewrite H2 in Hlookup_r.
+      rewrite runtime_getVal_update_diff in Hlookup_r; auto.
+      eapply Henv_respects; eauto.
+    }
+    exact Henv_respects''.
+    exact Hheap_respects'.
+    +
+    assert (Hwfmethod: exists D ddef, base_subtype CT cy D /\ find_class CT D = Some ddef /\ In mdef (methods (body ddef)) /\ wf_method CT D mdef).
+    {
+      eapply method_lookup_in_wellformed_inherited; eauto.
+      eapply r_basetype_in_dom; eauto.
+    }
+    destruct Hwfmethod as [D Hwfmethod].
+    destruct Hwfmethod as [ddef Hwfmethod].
+    destruct Hwfmethod as [Hbasecyd [HfindD [HmdefinD Hwfmethod]]].
+
+    unfold wf_method in Hwfmethod;
+    destruct Hwfmethod as [sΓmethodend [mbodyreturntype [Hmethodbody_typing [HmethodReturnBound [HmethodReturnType [HmethodReturnSubtype HMethodoverride]]]]]];
+    remember (mreceiver (msignature mdef) :: mparams (msignature mdef)) as sΓmethodinit;
+    remember {| vars := Iot ly :: vals |} as rΓmethodinit;
+    remember (rΓ <| vars := update x retval (vars rΓ) |>) as rΓ'''.
+    assert(Hwf_method_frame : wf_r_config CT sΓmethodinit rΓmethodinit h).
+    {
+      (* Method inner config wellformed.*)
+        have Hclass := Hclasstable.
+        unfold  wf_class_table in Hclass.
+        destruct Hclass as [Hclass [Hobjexist [Hotherclasses Hcname_consistent]]].
+        repeat split.
+        exact Hclass.
+        exact Hobjexist.
+        exact Hotherclasses.
+        apply Hcname_consistent.
+        apply Hcname_consistent.
+        exact Hheap.
+        rewrite HeqrΓmethodinit.
+        simpl.
+        lia.
+        unfold wf_renv in Hrenv.
+        destruct Hrenv as [HrEnvLen [Hreceiverval Hallvals]].
+        exists ly.
+        split.
+        rewrite HeqrΓmethodinit.
+        simpl.
+        reflexivity.
+        unfold runtime_getVal in H.
+        destruct (nth_error (vars rΓ) y) as [v|] eqn:Hnth_y; [|discriminate].
+        injection H as H1_eq.
+        subst v.
+        eapply Forall_nth_error in Hallvals; eauto.
+        simpl in Hallvals.
+        destruct (runtime_getObj h ly) as [obj|] eqn:Hobjly; [|contradiction].
+        apply runtime_getObj_dom in Hobjly.
+        exact Hobjly.
+
+        (* Inner runtime env is wellformed *)
+        rewrite HeqrΓmethodinit.
+        simpl.
+        constructor.
+        simpl.
+        unfold runtime_getVal in H.
+        destruct (nth_error (vars rΓ) y) as [v|] eqn:Hnth_y; [|discriminate].
+        injection H as H1_eq.
+        subst v.
+        unfold runtime_getVal in Hnth_y.
+        unfold wf_renv in Hrenv.
+        destruct Hrenv as [_ [_ Hallvals]].
+        eapply Forall_nth_error in Hallvals; eauto.
+        simpl in Hallvals.
+        exact Hallvals.
+        eapply runtime_lookup_list_preserves_wf_values; eauto.
+
+        (* Inner Static Environment's length is more than 0 *)
+        rewrite HeqsΓmethodinit.
+        simpl.
+        lia.
+
+        (* Inner static env's elements are wellformed typeuse *)
+        rewrite HeqsΓmethodinit.
+        constructor.
+
+        (* Receiver type is well-formed *)
+        eapply method_sig_wf_receiver_by_find; eauto.
+        (* assert (Hcydom: cy < dom CT). {
+            eapply find_class_dom; eauto.
+        }
+        exact Hcydom. *)
+        assert (Hparentdom: parent < dom CT). {
+          assert (cy < dom CT). {
+            eapply find_class_dom; eauto.
+          }
+          assert (parent < cy). {
+            eapply parent_implies_strict_ordering with (C:= cy) (D:=parent); eauto.
+          }
+          lia.
+        }
+        exact Hparentdom. 
+        eapply method_sig_wf_parameters_by_find; eauto.
+        assert (Hparentdom: parent < dom CT). {
+          assert (cy < dom CT). {
+            eapply find_class_dom; eauto.
+          }
+          assert (parent < cy). {
+            eapply parent_implies_strict_ordering with (C:= cy) (D:=parent); eauto.
+          }
+          lia.
+        }
+        exact Hparentdom. 
+        apply static_getType_list_preserves_length in H11.
+        apply runtime_lookup_list_preserves_length in H4.
+        rewrite HeqsΓmethodinit.
+        rewrite HeqrΓmethodinit.
+        simpl.
+        f_equal.
+        apply Forall2_length in H20.
+        assert (Hy_dom : y < dom sΓ).
+        {
+          apply static_getType_dom in H10.
+          exact H10.
+        }
+        assert (HOutterReceiverAddr: exists lOutterReceiver, get_this_var_mapping (vars rΓ) = Some lOutterReceiver).
+        {
+          eapply get_this_exists_from_wf_r_config; eauto.
+
+        }
+        destruct HOutterReceiverAddr as [lOutterReceiver HOutterReceiverAddr].
+        assert (HOutterReceiverMutability: exists qcontext, r_muttype h lOutterReceiver = Some qcontext).
+        {
+          eapply receiver_mutability_exists_wf_renv; eauto.
+        }
+        destruct HOutterReceiverMutability as [OutterReceiverMutability HOutterReceiverMutabilityType].
+        have Hcorr := Htypable.
+        have Hcorrcopy := Hcorr.
+        specialize (Hcorr lOutterReceiver OutterReceiverMutability HOutterReceiverAddr HOutterReceiverMutabilityType y Hy_dom Ty H10).
+        unfold wf_r_typable in Hcorr.
+        unfold r_basetype in H0.
+        unfold r_type.
+        destruct (runtime_getObj h ly) as [obj|] eqn:Hobjy; [|discriminate].
+        injection H0 as Hcy_eq.
+        subst cy.
+        destruct obj as [rt_obj fields_obj].
+        destruct rt_obj as [rq_obj rc_obj].
+
+        unfold wf_renv in Hrenv.
+        destruct Hrenv as [_ [Hreceiver _]].
+        destruct Hreceiver as [iot [Hget_iot _]].
+        unfold get_this_var_mapping.
+        unfold gget in Hget_iot.
+        destruct (vars rΓ) as [|v0 vs] eqn:Hvars; [discriminate|].
+
+        unfold r_type in Hcorr.
+        rewrite H in Hcorr.
+        rewrite Hobjy in Hcorr.
+        simpl in Hcorr.
+        destruct Hcorr as [Hbasesubtype HyQualifierTypablility].
+        assert (msignature mdef = msignature mdef0).
+        {
+          eapply method_signature_consistent_subtype; eauto.
+        }
+        rewrite H0.
+        rewrite H4.
+        rewrite <- H20.
+        exact H11.
+
+        (* Correspondence holds for inner environment *)
+        intros ι qinner HreceiverAddr Hqcontext i Hi sqt Hnth.
+        rewrite HeqsΓmethodinit in Hnth, Hi.
+        rewrite HeqrΓmethodinit.
+        simpl in *.
+        assert (Hy_dom : y < dom sΓ).
+        {
+          apply static_getType_dom in H10.
+          exact H10.
+        }
+        assert (HOutterReceiverAddr: exists lOutterReceiver, get_this_var_mapping (vars rΓ) = Some lOutterReceiver).
+        {
+          eapply get_this_exists_from_wf_r_config; eauto.
+        }
+        destruct HOutterReceiverAddr as [lOutterReceiver HOutterReceiverAddr].
+        assert (HOutterReceiverMutability: exists qcontext, r_muttype h lOutterReceiver = Some qcontext).
+        {
+          eapply receiver_mutability_exists_wf_renv; eauto.
+        }
+        destruct HOutterReceiverMutability as [OutterReceiverMutability HOutterReceiverMutabilityType].
+        have Hcorr := Htypable.
+        have Hcorrcopy := Hcorr.
+        specialize (Hcorr lOutterReceiver OutterReceiverMutability HOutterReceiverAddr HOutterReceiverMutabilityType y Hy_dom Ty H10).
+        unfold wf_r_typable in Hcorr.
+        unfold r_basetype in H0.
+        unfold r_type.
+        destruct (runtime_getObj h ly) as [obj|] eqn:Hobjy; [|discriminate].
+        injection H0 as Hcy_eq.
+        subst cy.
+        destruct obj as [rt_obj fields_obj].
+        destruct rt_obj as [rq_obj rc_obj].
+
+        have Hrenvcopy := Hrenv.
+        unfold wf_renv in Hrenv.
+        destruct Hrenv as [_ [Hreceiver _]].
+        destruct Hreceiver as [iot [Hget_iot _]].
+        unfold get_this_var_mapping.
+        unfold gget in Hget_iot.
+        destruct (vars rΓ) as [|v0 vs] eqn:Hvars; [discriminate|].
+
+        unfold r_type in Hcorr.
+        rewrite H in Hcorr.
+        rewrite Hobjy in Hcorr.
+        simpl in Hcorr.
+        destruct Hcorr as [Hbasesubtype HyQualifierTypablility].
+        
+        assert (Hmsigeq: msignature mdef = msignature mdef0).
+        {
+          eapply method_signature_consistent_subtype; eauto.
+        }
+        destruct i as [|i'].
+
+        (* Reciever index - 0 *)
+        simpl in Hnth.
+        injection Hnth as Hsqt_eq.
+        subst sqt.
+        simpl.
+        unfold wf_r_typable.
+        unfold r_type.
+
+        rewrite Hobjy.
+        simpl.
+        split.
+
+        (* Base type subtyping *)
+        rewrite Hmsigeq.
+        apply qualified_type_subtype_base_subtype in H19.
+        (* rewrite (vpa_mutabilty_tt_sctype Tthis Ty) in H23. *)
+        rewrite (vpa_mutabilty_tt_sctype Ty (mreceiver (msignature mdef0))) in H19.
+        eapply base_trans; eauto.
+
+        (* Qualifier typbility *)
+        1: 
+        {
+          apply qualified_type_subtype_q_subtype in H19.
+          specialize (Hcorrcopy lOutterReceiver OutterReceiverMutability HOutterReceiverAddr HOutterReceiverMutabilityType).
+          apply get_this_qualified_type_nth_error in H12.
+          unfold wf_senv in Hsenv.
+          destruct Hsenv as [Hsenvdom _].
+          specialize (Hcorrcopy 0 Hsenvdom Tthis H12).
+          rewrite <- Hvars in HOutterReceiverAddr.
+          apply get_this_var_mapping_runtime_getVal in HOutterReceiverAddr.
+          rewrite HOutterReceiverAddr in Hcorrcopy.
+          unfold wf_r_typable in Hcorrcopy.
+          unfold r_type in Hcorrcopy.
+          destruct (runtime_getObj h lOutterReceiver) as [outterreceiverobj|] eqn:Houtterobj; [|easy].
+          destruct Hcorrcopy as [_ Houtter_qualifier_typable].
+
+          assert (rqtype (rt_type outterreceiverobj) = OutterReceiverMutability).
+          {
+            unfold r_muttype in HOutterReceiverMutabilityType.
+            rewrite Houtterobj in HOutterReceiverMutabilityType.
+            simpl in HOutterReceiverMutabilityType.
+            inversion HOutterReceiverMutabilityType; subst OutterReceiverMutability.
+            reflexivity.
+          }
+          subst OutterReceiverMutability.
+
+          assert (ly = ι). 
+          {
+            rewrite HeqrΓmethodinit in HreceiverAddr.
+            unfold get_this_var_mapping in HreceiverAddr.
+            simpl in HreceiverAddr.
+            inversion HreceiverAddr; reflexivity.
+          }
+          subst ι.
+
+          assert (r_muttype h ly = Some rq_obj).
+          {
+            unfold r_muttype.
+            rewrite Hobjy.
+            simpl.
+            reflexivity.
+          }
+
+          assert (rq_obj = qinner).
+          {
+            rewrite H0 in Hqcontext.
+            inversion Hqcontext; subst qinner.
+            reflexivity.
+          }
+          subst rq_obj.
+
+          unfold qualifier_typable_context.
+          unfold qualifier_typable_context in HyQualifierTypablility.
+          unfold qualifier_typable_context in Houtter_qualifier_typable.
+          unfold vpa_mutabilty_rs.
+          unfold vpa_mutabilty_rs in HyQualifierTypablility.
+          unfold vpa_mutabilty_rs in Houtter_qualifier_typable.
+          unfold vpa_mutabilty_tt in H19.
+          rewrite <- Hmsigeq in H19.
+
+          destruct qinner eqn:HInnerReceiverMutability;
+          destruct (sqtype (mreceiver (msignature mdef))) eqn:HMethodReceiverDeclaredType;
+          try trivial.
+          all: destruct (rqtype (rt_type outterreceiverobj)) eqn:HOutterReceiverMutability;
+          destruct (sqtype Ty) eqn:HTyStaticMutability;
+          try trivial.
+          all: destruct (sqtype Tthis) eqn:HTthisStaticMutability;
+          try rewrite HTyStaticMutability in H19;
+          simpl in H19;
+          try rewrite HMethodReceiverDeclaredType in H19;
+          try inversion H19; try trivial.
+          all: try inversion H19; try easy.
+        }
+        (* clear_dups. amazing.... *)
+
+  (* -------------------------------------------------- *)
+  (* Other index - > 1 *)
+        apply qualified_type_subtype_q_subtype in H18.
+        unfold runtime_getVal.
+        simpl.
+        destruct (nth_error vals i') as [v|] eqn:Hval_i.
+          - (* Parameter i' exists *)
+            destruct v as [|loc]; [trivial|].
+            (* Use H23 to get the subtyping relationship *)
+            assert (Hi'_bound : i' < List.length argtypes).
+            {
+              apply Forall2_length in H20.
+              simpl in Hi.
+              simpl in Hnth.
+              rewrite Hmsigeq in Hnth.
+              rewrite H20.
+              apply nth_error_Some.
+              intros Hnone.
+              rewrite Hnth in Hnone.
+              discriminate.
+            }
+            assert (Harg_type : exists argtype, nth_error argtypes i' = Some argtype).
+            {
+              apply nth_error_Some_exists.
+              exact Hi'_bound.
+            }
+            assert (loc < dom h).
+            {
+              assert (Hvals_wf :
+              Forall
+                (fun v =>
+                  match v with
+                  | Null_a => True
+                  | Iot loc =>
+                      match runtime_getObj h loc with
+                      | Some _ => True
+                      | None => False
+                      end
+                  end) vals).
+              {
+                eapply runtime_lookup_list_preserves_wf_values; eauto.
+              }
+              eapply Forall_nth_error in Hvals_wf; eauto.
+              simpl in Hvals_wf.
+              destruct (runtime_getObj h loc) as [argobj|] eqn:Hargobjloc; [|contradiction].
+              apply runtime_getObj_dom in Hargobjloc.
+              exact Hargobjloc.
+            }
+            destruct Harg_type as [argtype Hargtype].
+            unfold wf_r_typable.
+            unfold r_type.
+            destruct (runtime_getObj h loc) as [argobj|] eqn:Hargobjloc; [|apply runtime_getObj_not_dom in Hargobjloc; lia].
+            assert (HargtypeFromsEnv :
+              exists iArgInSenv,
+                nth_error sΓ iArgInSenv = Some argtype
+            /\ nth_error zs i' = Some iArgInSenv).
+            {
+              destruct (static_getType_list_nth_zs sΓ zs argtypes i' argtype H11 Hargtype)
+                as [j [Hzs_j Hst_j]].
+              exists j.
+              split.
+              - (* from static_getType to nth_error sΓ' *)
+                unfold static_getType in Hst_j; exact Hst_j.
+              - (* keep the zs fact *)
+                exact Hzs_j.
+            }
+            destruct HargtypeFromsEnv as [iArgInSenv [HargtypeFromsEnv Hzs_iArg]].
+
+            assert (Hi'dom : iArgInSenv < dom sΓ).
+            {
+              apply nth_error_Some.
+              rewrite HargtypeFromsEnv; discriminate.
+            }
+            assert (HargtypeFromrEnv :
+                      nth_error (vars rΓ) iArgInSenv = Some (Iot loc)).
+            {
+              destruct (runtime_lookup_list_nth_zs rΓ zs vals i' (Iot loc) H4 Hval_i)
+                as [j [Hzs_j Hget_j]].
+              assert (HiEq : iArgInSenv = j).
+              {
+                (* zs[i'] = Some iArgInSenv and zs[i'] = Some j ⇒ iArgInSenv = j *)
+                rewrite Hzs_iArg in Hzs_j.
+                inversion Hzs_j; reflexivity.
+              }
+              subst iArgInSenv.
+              unfold runtime_getVal in Hget_j.
+              exact Hget_j.
+            }
+            have Hcorrcopy_2 := Hcorrcopy.
+            specialize (Hcorrcopy lOutterReceiver OutterReceiverMutability HOutterReceiverAddr HOutterReceiverMutabilityType iArgInSenv Hi'dom argtype HargtypeFromsEnv).
+            unfold runtime_getVal in Hcorrcopy.
+            rewrite HargtypeFromrEnv in Hcorrcopy.
+            unfold wf_r_typable in Hcorrcopy.
+            unfold r_type in Hcorrcopy.
+            rewrite Hargobjloc in Hcorrcopy.
+            destruct Hcorrcopy as [Harg_basesubtype Harg_qualifiertypability].
+            split.
+
+            (* base subtype *)
+            rewrite nth_error_cons_succ in Hnth.
+            rewrite Hmsigeq in Hnth.
+            eapply Forall2_nth_error in H20; eauto.
+            apply qualified_type_subtype_base_subtype in H20.
+            rewrite (vpa_mutabilty_tt_sctype Ty sqt) in H20.
+            eapply base_trans; eauto.
+
+            (* Qualifier Typability *)
+            rewrite Hmsigeq in Hnth.
+            eapply Forall2_nth_error in H20; eauto.
+            apply qualified_type_subtype_q_subtype in H20.
+            rewrite sq_vpa_tt_eq_qq in H20.
+            specialize (Hcorrcopy_2 lOutterReceiver OutterReceiverMutability HOutterReceiverAddr HOutterReceiverMutabilityType).
+            unfold wf_senv in Hsenv.
+            destruct Hsenv as [Hsenvdom _].
+            apply get_this_qualified_type_nth_error in H12.
+            specialize (Hcorrcopy_2 0 Hsenvdom Tthis H12).
+            rewrite <- Hvars in Hget_iot.
+            apply get_this_var_mapping_runtime_getVal in Hget_iot.
+            rewrite Hget_iot in Hcorrcopy_2.
+            unfold wf_r_typable in Hcorrcopy_2.
+            unfold r_type in Hcorrcopy_2.
+            destruct (runtime_getObj h iot) as [outterreceiverobj|] eqn:Houtterobj; [|easy].
+            destruct Hcorrcopy_2 as [_ HOutterReceiverQualifierTypablility].
+            assert (rqtype (rt_type outterreceiverobj) = OutterReceiverMutability).
+            {
+              clear - Houtterobj HOutterReceiverMutabilityType HOutterReceiverAddr Hget_iot Hvars.
+              rewrite <- Hvars in HOutterReceiverAddr.
+              apply get_this_var_mapping_runtime_getVal in HOutterReceiverAddr.
+              rewrite Hget_iot in HOutterReceiverAddr.
+              inversion HOutterReceiverAddr; subst lOutterReceiver.
+              unfold r_muttype in HOutterReceiverMutabilityType.
+              rewrite Houtterobj in HOutterReceiverMutabilityType.
+              simpl in HOutterReceiverMutabilityType.
+              inversion HOutterReceiverMutabilityType; reflexivity.
+            }
+            subst OutterReceiverMutability.
+            assert (ι = ly).
+            {
+              unfold get_this_var_mapping in HreceiverAddr.
+              rewrite HeqrΓmethodinit in HreceiverAddr.
+              simpl in HreceiverAddr.
+              inversion HreceiverAddr; reflexivity.
+            }
+            subst ι.
+            assert(rq_obj = qinner).
+            {
+              unfold r_muttype in Hqcontext.
+              rewrite Hobjy in Hqcontext.
+              simpl in Hqcontext.
+              inversion Hqcontext.
+              easy.
+            }
+            subst rq_obj.
+            clear - H20 Harg_qualifiertypability HyQualifierTypablility HOutterReceiverQualifierTypablility.
+
+            destruct (rqtype (rt_type argobj)) eqn:Hargobjmutability; move Hargobjmutability at bottom;
+            destruct (sqtype sqt) eqn:HParameterStaticDeclearedMutability; move HParameterStaticDeclearedMutability at bottom;
+            destruct qinner eqn:HInnerReceiverMutability; move HInnerReceiverMutability at bottom;
+            try solve_qualifier_typable_correct_concrete.
+
+            all: destruct (sqtype Ty) eqn:HTyStaticMutability;
+            destruct (sqtype argtype) eqn:HArgTypeStaticMutability;
+            simpl in H20;
+            try solve_q_subtype_wrong.
+
+            all: 
+            destruct (rqtype (rt_type outterreceiverobj)) eqn:HOutterReceiverMutability;
+            try solve_qualifier_typable_wrong_concrete.
+
+          - (* Parameter i' doesn't exist - contradiction *)
+            exfalso.
+            apply nth_error_None in Hval_i.
+            apply runtime_lookup_list_preserves_length in H4.
+            apply static_getType_list_preserves_length in H11.
+            apply Forall2_length in H20.
+            rewrite H4 in Hval_i.
+            rewrite <- H11 in Hval_i.
+            rewrite H20 in Hval_i.
+            simpl in Hi.
+            simpl in Hnth.
+            rewrite <- Hmsigeq in Hval_i.
+            lia.
+    }
+    specialize (IHHeval Heval sΓmethodend sΓmethodinit).
+    assert (HenvInvariant: env_respects_protected_set (protected_locset CT h l_root)
+    sΓmethodinit rΓmethodinit).
+    {
+      unfold env_respects_protected_set.
+      intros z l_z Tz Hlookup_s Hlookup_r Hin_P.
+      rewrite HeqsΓmethodinit in Hlookup_s.
+      rewrite HeqrΓmethodinit in Hlookup_r.
+      unfold static_getType in Hlookup_s.
+      unfold runtime_getVal in Hlookup_r.
+      simpl in Hlookup_s, Hlookup_r.
+      destruct z as [| z'].
+      - simpl in Hlookup_s, Hlookup_r.
+      injection Hlookup_s as <-. injection Hlookup_r as <-.
+      unfold is_safe_mode.
+      have Hty_safe : is_safe_mode (sqtype Ty).
+      {
+        unfold env_respects_protected_set in Henv_respects.
+        specialize (Henv_respects y ly Ty H10 H Hin_P).
+        exact Henv_respects.
+      }
+      unfold is_safe_mode in Hty_safe.
+      unfold vpa_mutabilty_tt.
+      apply qualified_type_subtype_q_subtype in H19.
+      clear - Hty_safe H19.
+      unfold vpa_mutabilty_tt in H19.
+      destruct Hty_safe as [HRd | HLost].
+      + (* Case: sqtype Ty = Rd *)
+        rewrite HRd in H19.
+        simpl in H19.
+        inversion H19; easy.
+      + (* Case: sqtype Ty = Lost *)
+        rewrite HLost in H19.
+        simpl in H19.
+        inversion H19; easy.
+      -
+        assert (Hy_dom : y < dom sΓ).
+        {
+          apply static_getType_dom in H10.
+          exact H10.
+        }
+
+        unfold wf_renv in Hrenv.
+        destruct Hrenv as [_ [Hreceiver _]].
+        destruct Hreceiver as [iot [Hget_iot Hiot_dom]].
+        assert (HOutterReceiverMutability: exists qcontext, r_muttype h iot = Some qcontext).
+        {
+          eapply receiver_mutability_exists_from_bound; eauto.
+        }
+        destruct HOutterReceiverMutability as [qoutter Hqoutter].
+        (* Apply correspondence to get wf_r_typable *)
+        specialize (Htypable iot qoutter Hget_iot Hqoutter y Hy_dom Ty H10).
+        unfold wf_r_typable in Htypable.
+        unfold r_basetype in H1.
+        unfold r_type.
+        destruct (runtime_getObj h ly) as [obj|] eqn:Hobjy.
+        2:{
+          unfold r_basetype in H0.
+          rewrite Hobjy in H0.
+          discriminate.
+        }
+        destruct obj as [rt_obj fields_obj].
+        destruct rt_obj as [rq_obj rc_obj].
+
+        unfold r_type in Htypable.
+        rewrite H in Htypable.
+        rewrite Hobjy in Htypable.
+        simpl in Htypable.
+        destruct Htypable as [Hsubtype Hqualifier].
+        simpl in Hobjy.
+
+        simpl in H1.
+        inversion H1.
+        assert (Hrc_obj_eq: rc_obj = cy).
+        {
+          unfold r_basetype in H0.
+          rewrite Hobjy in H0.
+          inversion H0.
+          easy.
+        }
+        subst rc_obj.
+        assert (Hsigeq: msignature mdef = msignature mdef0).
+        {
+          eapply method_signature_consistent_subtype; eauto.
+        }
+        have Hnth_param_type : nth_error (mparams (msignature mdef)) z' = Some Tz.
+        {
+          simpl in Hlookup_s.
+          easy.
+        }
+
+        have Hnth_param_val : nth_error vals z' = Some (Iot l_z).
+        {
+          simpl in Hlookup_r.
+          easy.
+        }
+        assert (Hi'_bound : z' < List.length argtypes).
+        {
+          apply Forall2_length in H20.
+          rewrite <- Hsigeq in H20.
+          assert (H_bound_params : z' < dom (mparams (msignature mdef))).
+          {
+            apply nth_error_Some. (* Converts "index < len" to "lookup <> None" *)
+            rewrite Hnth_param_type.   (* lookup is Some Tz *)
+            discriminate.         (* Some <> None *)
+          }
+
+          (* 2. Convert to bound for argtypes using the equality *)
+          rewrite <- H20 in H_bound_params. (* Replace length of params with length of argtypes *)
+
+          (* 3. Solve the goal *)
+          exact H_bound_params.
+        }
+
+        have Hnth_arg: exists T_arg, nth_error argtypes z' = Some T_arg.
+        {
+          apply nth_error_Some_exists.
+          exact Hi'_bound.
+        }
+
+        destruct Hnth_arg as [T_arg Hnth_arg].
+        eapply Forall2_nth_error with (i := z') (a := T_arg) (b := Tz) in H20; [|auto|rewrite <- Hsigeq; exact Hnth_param_type].
+        (* apply qualified_type_subtype_q_subtype in H20. *)
+        unfold env_respects_protected_set in Henv_respects.
+        apply adapated_subtype_safe_implies_safe in H20; auto.
+
+        have HargtypeFromsEnv :
+          exists z_outter,
+            static_getType sΓ z_outter = Some T_arg /\
+            nth_error zs z' = Some z_outter.
+        {
+          destruct (static_getType_list_nth_zs sΓ zs argtypes z' T_arg H11 Hnth_arg)
+            as [j [Hzs_j Hst_j]].
+          exists j.
+          split.
+          - unfold static_getType. exact Hst_j.
+          - exact Hzs_j.
+        }
+
+        destruct HargtypeFromsEnv as [z_outter [HgetZ_type Hzs_z_outter]].
+
+        have HgetZ_val : runtime_getVal rΓ z_outter = Some (Iot l_z).
+        {
+          destruct (runtime_lookup_list_nth_zs rΓ zs vals z' (Iot l_z) H4 Hnth_param_val)
+            as [j [Hzs_j Hget_j]].
+          assert (HzEq : z_outter = j) by (
+            rewrite Hzs_z_outter in Hzs_j;
+            inversion Hzs_j; reflexivity
+          ).
+          subst j.
+          exact Hget_j.
+        }
+        specialize (Henv_respects z_outter l_z T_arg HgetZ_type HgetZ_val Hin_P); auto.
+    }
+    assert (HMethodInnerInvariant: env_respects_protected_set (protected_locset CT h l_root)
+    sΓmethodinit rΓmethodinit /\ heap_respects_protected_set (protected_locset CT h l_root) h h CT).
+    {
+      split.
+      exact HenvInvariant.
+      exact Hheap_respects.
+    }
+    specialize (IHHeval HMethodInnerInvariant Hwf_method_frame).
+    rewrite <- getmbody in Hmethodbody_typing.
+    specialize (IHHeval Hmethodbody_typing).
+    destruct IHHeval as [Htopology Hconfinement].
+    destruct Hconfinement as [Henv_respects' Hheap_respects'].
+    split.
+    exact Htopology.
+    split.
+    assert (Henv_respects'': env_respects_protected_set (protected_locset CT h l_root) sΓ rΓ''' ).
+    {
+      rewrite HeqrΓ'''.
+      unfold env_respects_protected_set.
+      intros z l_z T_z Hlookup_s Hlookup_r Hin_P.
+      destruct (Nat.eq_dec x z) eqn: Heqxz.
+        --- (* CASE: z = x (New Variable) *)
+        subst z.
+        assert (T_z = Tx). 
+        {
+          rewrite H9 in Hlookup_s. 
+          injection Hlookup_s as H_eq_T. subst T_z.
+          reflexivity.
+        }
+        subst T_z.
+        unfold env_respects_protected_set in Henv_respects'.
+        have HGetMethodReturnType: static_getType sΓmethodend (mreturn (Syntax.mbody mdef)) = Some mbodyreturntype.
+        {
+          unfold static_getType; auto.
+        }
+        assert (Hy_dom : y < dom sΓ).
+        {
+          apply static_getType_dom in H10.
+          exact H10.
+        }
+
+        unfold wf_renv in Hrenv.
+        destruct Hrenv as [_ [Hreceiver _]].
+        destruct Hreceiver as [iot [Hget_iot Hiot_dom]].
+        assert (HOutterReceiverMutability: exists qcontext, r_muttype h iot = Some qcontext).
+        {
+          eapply receiver_mutability_exists_from_bound; eauto.
+        }
+        destruct HOutterReceiverMutability as [qoutter Hqoutter].
+        (* Apply correspondence to get wf_r_typable *)
+        specialize (Htypable iot qoutter Hget_iot Hqoutter y Hy_dom Ty H10).
+        unfold wf_r_typable in Htypable.
+        unfold r_basetype in H1.
+        unfold r_type.
+        destruct (runtime_getObj h ly) as [obj|] eqn:Hobjy.
+        2:{
+          unfold r_basetype in H0.
+          rewrite Hobjy in H0.
+          discriminate.
+        }
+        destruct obj as [rt_obj fields_obj].
+        destruct rt_obj as [rq_obj rc_obj].
+
+        unfold r_type in Htypable.
+        rewrite H in Htypable.
+        rewrite Hobjy in Htypable.
+        simpl in Htypable.
+        destruct Htypable as [Hsubtype Hqualifier].
+        simpl in Hobjy.
+
+        simpl in H1.
+        inversion H1.
+        assert (Hrc_obj_eq: rc_obj = cy).
+        {
+          unfold r_basetype in H0.
+          rewrite Hobjy in H0.
+          inversion H0.
+          easy.
+        }
+        subst rc_obj.
+        assert (Hsigeq: msignature mdef = msignature mdef0).
+        {
+          eapply method_signature_consistent_subtype; eauto.
+        }
+        rewrite getmbody in H6.
+        have Hdom_x : x < dom (vars rΓ). 
+        { 
+          apply runtime_getVal_dom in Hlookup_r.
+          rewrite update_length in Hlookup_r.
+          exact Hlookup_r.
+        }
+        have Hlookup_r_copy := Hlookup_r.
+        rewrite <- HeqrΓ''' in Hlookup_r_copy.
+        unfold runtime_getVal in Hlookup_r.
+        rewrite update_same in Hlookup_r. lia.   (* or by exact Hdom_x *)
+        inversion Hlookup_r; subst.
+        specialize (Henv_respects' (mreturn (Syntax.mbody mdef)) l_z mbodyreturntype HGetMethodReturnType H6 Hin_P).
+        rewrite <- Hsigeq in H18.
+        apply subtype_safe_implies_safe in HmethodReturnSubtype; auto.
+        apply subtype_safe_implies_safe_adapted in H18; auto.
+        --- (* CASE: z <> x (Old Variables) *)
+        (* Just use the original invariant *)
+        assert (rΓ <| vars := update x retval (vars rΓ) |> = update_r_env_value rΓ x retval).
+        {
+          destruct rΓ.
+          reflexivity.
+        }
+        rewrite H2 in Hlookup_r.
+        rewrite runtime_getVal_update_diff in Hlookup_r; auto.
+        eapply Henv_respects; eauto.
+    }
+    exact Henv_respects''.
+    exact Hheap_respects'.
+Admitted.
+
+Theorem deep_readonly_preservation :
+  forall CT sΓ rΓ h l_root stmt rΓ' h' sΓ' l C anyrq vals vals' f
+         (* 1. Initialize P based on the START state *)
+         (* (HP_def : P = protected_locset CT h l_root) *)
+         
+         (* 2. Pre-condition: Invariant holds for P *)
+         (* (Note: env_respects is trivial by def of P; heap_respects needs wf) *)
+         (Hdom_root : l_root < dom h)
+         (Hconfined : confinement_invariant_precise (protected_locset CT h l_root) CT sΓ rΓ h h)
+         (Hwf : wf_r_config CT sΓ rΓ h)
+         
+         (* 3. Execution *)
+         (Htyping : stmt_typing CT sΓ stmt sΓ')
+         (Heval : eval_stmt OK CT rΓ h stmt OK rΓ' h')
+         
+    (* CONCLUSION: *)
+    (* 1. The Invariant is preserved (Safety) *)
+    (* confinement_invariant_precise P CT sΓ' rΓ' h' /\ *)
+    
+    (* 2. The Protected Set P is physically unmodified (Deep Immutability) *)
+    (* (forall l C anyrq vals vals' f, *)
+       (Hlocalset : Ensembles.In Loc (protected_locset CT h l_root) l)
+       (Hobj : runtime_getObj h l = Some (mkObj (mkruntime_type anyrq C) vals))
+       (Hobj' : runtime_getObj h' l = Some (mkObj (mkruntime_type anyrq C) vals'))
+       (* Only protected fields need to be equal, as discussed *)
+       (* forall f,  *)
+       (Hassignability : (sf_assignability_rel CT C f Final \/ sf_assignability_rel CT C f RDA)),
+       nth_error vals f = nth_error vals' f.
+Proof.
+  intros.
+  remember OK as ok.
+  generalize dependent sΓ.
+  generalize dependent sΓ'.
+  generalize dependent vals. 
+  generalize dependent vals'.
+  induction Heval; intros; subst; try discriminate.
+  - (* Skip *) 
+    rewrite Hobj in Hobj'.
+    inversion Hobj'; subst.
+    reflexivity.
+  - (* Local *)
+    rewrite Hobj in Hobj'.
+    inversion Hobj'; subst.
+    reflexivity.
+  - (* VarAss *)
+    rewrite Hobj in Hobj'.
+    inversion Hobj'; subst.
+    reflexivity.
+  - (* FldWrite *)
+    + (* Protected objects unchanged *)
+    {
+    (* intros l C anyrq vals vals' Hin Hobj Hobj' f0 Hprotected.   *)
+    destruct (Nat.eq_dec loc_x l) as [Halias | Hno_alias].
+    -
+      subst loc_x.
+      destruct (Nat.eq_dec f f0) as [Heq_f | Hneq_f].
+      + (* Same field case: contradiction *)
+        subst f0.
+        (* Now: x points to l, and l ∈ P *)
+        (* Strategy: Show x must be Safe, but field write requires x to be Mut → contradiction *)
+        
+        (* Extract x's static type from typing *)
+        inversion Htyping; subst.
+        (* After inversion: static_getType sΓ x = Some Tx, and sqtype Tx should allow write *)
+        
+        (* Unfold confinement to get env_respects_protected_set *)
+        unfold confinement_invariant_precise in Hconfined.
+        destruct Hconfined as [Henv_respects _].
+        
+        (* Apply the lemma: if x points to l ∈ P, then x is Safe *)
+        have Hx_safe := mut_var_cannot_point_to_P sΓ' rΓ x Tx l (protected_locset CT h l_root) H7 H Henv_respects Hlocalset.
+        
+        (* But from ST_FldWrite typing, we need sqtype Tx to allow writes *)
+        (* H15: vpa_assignability (sqtype Tx) a = Assignable *)
+        
+        (* Case on assignability *)
+        apply vpa_assingability_assign_cases in H16.
+        unfold wf_r_config in Hwf.
+        destruct Hwf as [Hclasstable [_[Hrenv [_ [_ Htypable]]]]].
+        unfold wf_renv in Hrenv.
+        (* try destruct (extract_receiver_from_wf_config CT sΓ rΓ h Hwf) as [iot [qcontext [Hget_iot[Hiot_dom Hqcontext]]]]. *)
+        destruct Hrenv as [_ [Hreceiver _]].
+        destruct Hreceiver as [iot [Hget_iot Hiot_dom]].
+        assert (HOutterReceiverMutability: exists qcontext, r_muttype h iot = Some qcontext).
+        {
+          eapply receiver_mutability_exists_from_bound; eauto.
+        }
+        destruct HOutterReceiverMutability as [qcontext Hqcontext].
+        (* Apply correspondence to get wf_r_typable *)
+        specialize (Htypable iot qcontext Hget_iot Hqcontext x).
+        have H7copy := H7.
+        apply static_getType_dom in H7.
+        unfold static_getType in H7copy.
+        specialize (Htypable H7 Tx H7copy).
+        rewrite H in Htypable.
+        unfold wf_r_typable in Htypable.
+        unfold r_type in Htypable.
+        rewrite Hobj in Htypable.
+        destruct Htypable as [base qualifier].
+        simpl in base.
+        destruct H16 as [Ha_assign | [Hx_mut Ha_rda]].
+        
+        ++ (* Case: a = Assignable *)
+          destruct Hassignability as [HFinal | HRDA].
+          * (* Case: sf_assignability_rel CT C f Final *)
+          assert (Heq : Final = a).
+          {
+            eapply sf_assignability_consistent_subtype with (f := f) (C := C) (D := sctype Tx); eauto.
+          }
+          rewrite <- Heq in Ha_assign.
+          discriminate Ha_assign.
+          *
+          assert (Heq : RDA = a).
+          {
+            eapply sf_assignability_consistent_subtype with (f := f) (C := C) (D := sctype Tx); eauto.
+          }
+          rewrite <- Heq in Ha_assign.
+          discriminate Ha_assign.
+        ++ (* Case: sqtype Tx = Mut ∧ a = RDA *)
+          exfalso.
+          apply Hx_safe.
+          exact Hx_mut.
+      + (* Different field case: trivial *)
+        unfold update_field in Hobj'.
+        rewrite H0 in Hobj'.
+        simpl in Hobj'.
+
+        (* Extract the domain bound for l *)
+        assert (Hdom : l < dom h).
+        {
+          apply runtime_getObj_dom in H0.
+          exact H0.
+        }
+
+        (* After update_field, the object at l has fields updated at f0 *)
+        rewrite runtime_getObj_update_same in Hobj'; auto.
+
+        injection Hobj' as _ Hvals'_eq.
+        rewrite H0 in Hobj.
+        injection Hobj as Hvals_eq.
+
+        (* vals' is just vals with f0 updated, so f is unchanged *)
+        rewrite <- Hvals'_eq.
+        rewrite update_diff.
+        --
+         symmetry; exact Hneq_f.
+        -- 
+        assert (Hfields : fields_map o = vals).
+        {
+          rewrite Hvals_eq.
+          reflexivity.
+        }
+        rewrite Hfields.
+        reflexivity.
+    -
+      (* No aliasing case: trivial *)
+      unfold update_field in Hobj'.
+      have Heq : runtime_getObj 
+        (match runtime_getObj h loc_x with
+        | Some o => [loc_x ↦ o <| fields_map := update f0 val_y (fields_map o) |>] h
+        | None => h
+        end) l = runtime_getObj h l.
+      {
+        destruct (runtime_getObj h loc_x).
+        - apply runtime_getObj_update_diff; auto.
+        - reflexivity.
+      }
+      rewrite Heq in Hobj'.
+      rewrite Hobj in Hobj'.
+      inversion Hobj'.
+      reflexivity.
+    }
+  - (* New *)
+    (* intros l C anyrq vals0 vals' Hin Hobj Hobj' f Hprotected. *)
+    unfold protected_locset in Hlocalset.
+
+    (* Extract l < dom h from reachable_abs *)
+    assert(Hl_old : l < dom h).
+    {
+      apply runtime_getObj_dom in Hobj.
+      exact Hobj.
+    }
+    
+    rewrite runtime_getObj_last2 in Hobj'; auto.
+  - (* Call *)
+    inversion Htyping; subst sΓ'; subst.
+    have Hwfcopy := Hwf.
+    unfold wf_r_config in Hwf.
+    destruct Hwf as [Hclasstable [Hheap [Hrenv [Hsenv [_ Htypable]]]]].
+    unfold confinement_invariant_precise in *.
+    destruct Hconfined as [Henv_respects Hheap_respects].
+    specialize (IHHeval Hdom_root (eq_refl)).
+    destruct H1 as [mdeflookup getmbody].
+    remember (msignature mdef) as msig.
+    inversion mdeflookup; revert getmbody; subst; intro getmbody.
+    assert (Hwfmethod: wf_method CT cy mdef).
+    {
+      eapply method_lookup_wf_class; eauto.
+      eapply r_basetype_in_dom; eauto.
+      unfold gget_method in H3.
+      apply find_some in H3.
+      destruct H3.
+      exact H2.
+    }
+    unfold wf_method in Hwfmethod;
+    destruct Hwfmethod as [sΓmethodend [mbodyreturntype [Hmethodbody_typing [HmethodReturnBound [HmethodReturnType [HmethodReturnSubtype HMethodoverride]]]]]];
+    remember (mreceiver (msignature mdef) :: mparams (msignature mdef)) as sΓmethodinit;
+    remember {| vars := Iot ly :: vals |} as rΓmethodinit;
+    remember (rΓ <| vars := update x retval (vars rΓ) |>) as rΓ'''.
+    assert(Hwf_method_frame : wf_r_config CT sΓmethodinit rΓmethodinit h).
+    {
+      (* Method inner config wellformed.*)
+        have Hclass := Hclasstable.
+        unfold  wf_class_table in Hclass.
+        destruct Hclass as [Hclass [Hobjexist [Hotherclasses Hcname_consistent]]].
+        repeat split.
+        exact Hclass.
+        exact Hobjexist.
+        exact Hotherclasses.
+        apply Hcname_consistent.
+        apply Hcname_consistent.
+        exact Hheap.
+        rewrite HeqrΓmethodinit.
+        simpl.
+        lia.
+        unfold wf_renv in Hrenv.
+        destruct Hrenv as [HrEnvLen [Hreceiverval Hallvals]].
+        exists ly.
+        split.
+        rewrite HeqrΓmethodinit.
+        simpl.
+        reflexivity.
+        unfold runtime_getVal in H.
+        destruct (nth_error (vars rΓ) y) as [v|] eqn:Hnth_y; [|discriminate].
+        injection H as H1_eq.
+        subst v.
+        eapply Forall_nth_error in Hallvals; eauto.
+        simpl in Hallvals.
+        destruct (runtime_getObj h ly) as [obj|] eqn:Hobjly; [|contradiction].
+        apply runtime_getObj_dom in Hobjly.
+        exact Hobjly.
+
+        (* Inner runtime env is wellformed *)
+        rewrite HeqrΓmethodinit.
+        simpl.
+        constructor.
+        simpl.
+        unfold runtime_getVal in H.
+        destruct (nth_error (vars rΓ) y) as [v|] eqn:Hnth_y; [|discriminate].
+        injection H as H1_eq.
+        subst v.
+        unfold runtime_getVal in Hnth_y.
+        unfold wf_renv in Hrenv.
+        destruct Hrenv as [_ [_ Hallvals]].
+        eapply Forall_nth_error in Hallvals; eauto.
+        simpl in Hallvals.
+        exact Hallvals.
+        eapply runtime_lookup_list_preserves_wf_values with (zs := zs) (vals0:=vals); eauto.
+
+        (* Inner Static Environment's length is more than 0 *)
+        rewrite HeqsΓmethodinit.
+        simpl.
+        lia.
+
+        (* Inner static env's elements are wellformed typeuse *)
+        rewrite HeqsΓmethodinit.
+        constructor.
+
+        (* Receiver type is well-formed *)
+        eapply method_sig_wf_receiver_by_find; eauto.
+        assert (Hcydom: cy < dom CT). {
+            eapply find_class_dom; eauto.
+        }
+        exact Hcydom.
+        (* assert (parent < dom CT). {
+          assert (cy < dom CT). {
+            eapply find_class_dom; eauto.
+          }
+          assert (parent < cy). {
+            eapply parent_implies_strict_ordering with (C:= cy) (D:=parent); eauto.
+          }
+          lia.
+        } *)
+        eapply method_sig_wf_parameters_by_find; eauto.
+        assert (Hcydom: cy < dom CT). {
+            eapply find_class_dom; eauto.
+        }
+        exact Hcydom.
+
+        apply static_getType_list_preserves_length in H11.
+        apply runtime_lookup_list_preserves_length in H4.
+        rewrite HeqsΓmethodinit.
+        rewrite HeqrΓmethodinit.
+        simpl.
+        f_equal.
+        apply Forall2_length in H20.
+        assert (Hy_dom : y < dom sΓ).
+        {
+          apply static_getType_dom in H10.
+          exact H10.
+        }
+        assert (HOutterReceiverAddr: exists lOutterReceiver, get_this_var_mapping (vars rΓ) = Some lOutterReceiver).
+        {
+          eapply get_this_exists_from_wf_r_config; eauto.
+
+        }
+        destruct HOutterReceiverAddr as [lOutterReceiver HOutterReceiverAddr].
+        assert (HOutterReceiverMutability: exists qcontext, r_muttype h lOutterReceiver = Some qcontext).
+        {
+          eapply receiver_mutability_exists_wf_renv; eauto.
+        }
+        destruct HOutterReceiverMutability as [OutterReceiverMutability HOutterReceiverMutabilityType].
+        have Hcorr := Htypable.
+        have Hcorrcopy := Hcorr.
+        specialize (Hcorr lOutterReceiver OutterReceiverMutability HOutterReceiverAddr HOutterReceiverMutabilityType y Hy_dom Ty H10).
+        unfold wf_r_typable in Hcorr.
+        unfold r_basetype in H0.
+        unfold r_type.
+        destruct (runtime_getObj h ly) as [obj|] eqn:Hobjy; [|discriminate].
+        injection H0 as Hcy_eq.
+        subst cy.
+        destruct obj as [rt_obj fields_obj].
+        destruct rt_obj as [rq_obj rc_obj].
+
+        unfold wf_renv in Hrenv.
+        destruct Hrenv as [_ [Hreceiver _]].
+        destruct Hreceiver as [iot [Hget_iot _]].
+        unfold get_this_var_mapping.
+        unfold gget in Hget_iot.
+        destruct (vars rΓ) as [|v0 vs] eqn:Hvars; [discriminate|].
+
+        unfold r_type in Hcorr.
+        rewrite H in Hcorr.
+        rewrite Hobjy in Hcorr.
+        simpl in Hcorr.
+        destruct Hcorr as [Hbasesubtype HyQualifierTypablility].
+        assert (msignature mdef = msignature mdef0).
+        {
+          eapply method_signature_consistent_subtype; eauto.
+        }
+        rewrite H0.
+        rewrite H4.
+        rewrite <- H20.
+        exact H11.
+
+        (* Correspondence holds for inner environment *)
+        intros ι qinner HreceiverAddr Hqcontext i Hi sqt Hnth.
+        rewrite HeqsΓmethodinit in Hnth, Hi.
+        rewrite HeqrΓmethodinit.
+        simpl in *.
+        assert (Hy_dom : y < dom sΓ).
+        {
+          apply static_getType_dom in H10.
+          exact H10.
+        }
+        assert (HOutterReceiverAddr: exists lOutterReceiver, get_this_var_mapping (vars rΓ) = Some lOutterReceiver).
+        {
+          eapply get_this_exists_from_wf_r_config; eauto.
+        }
+        destruct HOutterReceiverAddr as [lOutterReceiver HOutterReceiverAddr].
+        assert (HOutterReceiverMutability: exists qcontext, r_muttype h lOutterReceiver = Some qcontext).
+        {
+          eapply receiver_mutability_exists_wf_renv; eauto.
+        }
+        destruct HOutterReceiverMutability as [OutterReceiverMutability HOutterReceiverMutabilityType].
+        have Hcorr := Htypable.
+        have Hcorrcopy := Hcorr.
+        specialize (Hcorr lOutterReceiver OutterReceiverMutability HOutterReceiverAddr HOutterReceiverMutabilityType y Hy_dom Ty H10).
+        unfold wf_r_typable in Hcorr.
+        unfold r_basetype in H0.
+        unfold r_type.
+        destruct (runtime_getObj h ly) as [obj|] eqn:Hobjy; [|discriminate].
+        injection H0 as Hcy_eq.
+        subst cy.
+        destruct obj as [rt_obj fields_obj].
+        destruct rt_obj as [rq_obj rc_obj].
+
+        have Hrenvcopy := Hrenv.
+        unfold wf_renv in Hrenv.
+        destruct Hrenv as [_ [Hreceiver _]].
+        destruct Hreceiver as [iot [Hget_iot _]].
+        unfold get_this_var_mapping.
+        unfold gget in Hget_iot.
+        destruct (vars rΓ) as [|v0 vs] eqn:Hvars; [discriminate|].
+
+        unfold r_type in Hcorr.
+        rewrite H in Hcorr.
+        rewrite Hobjy in Hcorr.
+        simpl in Hcorr.
+        destruct Hcorr as [Hbasesubtype HyQualifierTypablility].
+        
+        assert (Hmsigeq: msignature mdef = msignature mdef0).
+        {
+          eapply method_signature_consistent_subtype; eauto.
+        }
+        destruct i as [|i'].
+
+        (* Reciever index - 0 *)
+        simpl in Hnth.
+        injection Hnth as Hsqt_eq.
+        subst sqt.
+        simpl.
+        unfold wf_r_typable.
+        unfold r_type.
+
+        rewrite Hobjy.
+        simpl.
+        split.
+
+        (* Base type subtyping *)
+        rewrite Hmsigeq.
+        apply qualified_type_subtype_base_subtype in H19.
+        (* rewrite (vpa_mutabilty_tt_sctype Tthis Ty) in H23. *)
+        rewrite (vpa_mutabilty_tt_sctype Ty (mreceiver (msignature mdef0))) in H19.
+        eapply base_trans; eauto.
+
+        (* Qualifier typbility *)
+        1: 
+        {
+          apply qualified_type_subtype_q_subtype in H19.
+          specialize (Hcorrcopy lOutterReceiver OutterReceiverMutability HOutterReceiverAddr HOutterReceiverMutabilityType).
+          apply get_this_qualified_type_nth_error in H12.
+          unfold wf_senv in Hsenv.
+          destruct Hsenv as [Hsenvdom _].
+          specialize (Hcorrcopy 0 Hsenvdom Tthis H12).
+          rewrite <- Hvars in HOutterReceiverAddr.
+          apply get_this_var_mapping_runtime_getVal in HOutterReceiverAddr.
+          rewrite HOutterReceiverAddr in Hcorrcopy.
+          unfold wf_r_typable in Hcorrcopy.
+          unfold r_type in Hcorrcopy.
+          destruct (runtime_getObj h lOutterReceiver) as [outterreceiverobj|] eqn:Houtterobj; [|easy].
+          destruct Hcorrcopy as [_ Houtter_qualifier_typable].
+
+          assert (rqtype (rt_type outterreceiverobj) = OutterReceiverMutability).
+          {
+            unfold r_muttype in HOutterReceiverMutabilityType.
+            rewrite Houtterobj in HOutterReceiverMutabilityType.
+            simpl in HOutterReceiverMutabilityType.
+            inversion HOutterReceiverMutabilityType; subst OutterReceiverMutability.
+            reflexivity.
+          }
+          subst OutterReceiverMutability.
+
+          assert (ly = ι). 
+          {
+            rewrite HeqrΓmethodinit in HreceiverAddr.
+            unfold get_this_var_mapping in HreceiverAddr.
+            simpl in HreceiverAddr.
+            inversion HreceiverAddr; reflexivity.
+          }
+          subst ι.
+
+          assert (r_muttype h ly = Some rq_obj).
+          {
+            unfold r_muttype.
+            rewrite Hobjy.
+            simpl.
+            reflexivity.
+          }
+
+          assert (rq_obj = qinner).
+          {
+            rewrite H0 in Hqcontext.
+            inversion Hqcontext; subst qinner.
+            reflexivity.
+          }
+          subst rq_obj.
+
+          unfold qualifier_typable_context.
+          unfold qualifier_typable_context in HyQualifierTypablility.
+          unfold qualifier_typable_context in Houtter_qualifier_typable.
+          unfold vpa_mutabilty_rs.
+          unfold vpa_mutabilty_rs in HyQualifierTypablility.
+          unfold vpa_mutabilty_rs in Houtter_qualifier_typable.
+          unfold vpa_mutabilty_tt in H19.
+          rewrite <- Hmsigeq in H19.
+
+          destruct qinner eqn:HInnerReceiverMutability;
+          destruct (sqtype (mreceiver (msignature mdef))) eqn:HMethodReceiverDeclaredType;
+          try trivial.
+          all: destruct (rqtype (rt_type outterreceiverobj)) eqn:HOutterReceiverMutability;
+          destruct (sqtype Ty) eqn:HTyStaticMutability;
+          try trivial.
+          all: destruct (sqtype Tthis) eqn:HTthisStaticMutability;
+          try rewrite HTyStaticMutability in H19;
+          simpl in H19;
+          try rewrite HMethodReceiverDeclaredType in H19;
+          try inversion H19; try trivial.
+          all: try inversion H19; try easy.
+        }
+        (* clear_dups. amazing.... *)
+
+  (* -------------------------------------------------- *)
+  (* Other index - > 1 *)
+        apply qualified_type_subtype_q_subtype in H18.
+        unfold runtime_getVal.
+        simpl.
+        destruct (nth_error vals i') as [v|] eqn:Hval_i.
+          - (* Parameter i' exists *)
+            destruct v as [|loc]; [trivial|].
+            (* Use H23 to get the subtyping relationship *)
+            assert (Hi'_bound : i' < List.length argtypes).
+            {
+              apply Forall2_length in H20.
+              simpl in Hi.
+              simpl in Hnth.
+              rewrite Hmsigeq in Hnth.
+              rewrite H20.
+              apply nth_error_Some.
+              intros Hnone.
+              rewrite Hnth in Hnone.
+              discriminate.
+            }
+            assert (Harg_type : exists argtype, nth_error argtypes i' = Some argtype).
+            {
+              apply nth_error_Some_exists.
+              exact Hi'_bound.
+            }
+            assert (loc < dom h).
+            {
+              assert (Hvals_wf :
+              Forall
+                (fun v =>
+                  match v with
+                  | Null_a => True
+                  | Iot loc =>
+                      match runtime_getObj h loc with
+                      | Some _ => True
+                      | None => False
+                      end
+                  end) vals).
+              {
+                eapply runtime_lookup_list_preserves_wf_values; eauto.
+              }
+              eapply Forall_nth_error in Hvals_wf; eauto.
+              simpl in Hvals_wf.
+              destruct (runtime_getObj h loc) as [argobj|] eqn:Hargobjloc; [|contradiction].
+              apply runtime_getObj_dom in Hargobjloc.
+              exact Hargobjloc.
+            }
+            destruct Harg_type as [argtype Hargtype].
+            unfold wf_r_typable.
+            unfold r_type.
+            destruct (runtime_getObj h loc) as [argobj|] eqn:Hargobjloc; [|apply runtime_getObj_not_dom in Hargobjloc; lia].
+            assert (HargtypeFromsEnv :
+              exists iArgInSenv,
+                nth_error sΓ iArgInSenv = Some argtype
+            /\ nth_error zs i' = Some iArgInSenv).
+            {
+              destruct (static_getType_list_nth_zs sΓ zs argtypes i' argtype H11 Hargtype)
+                as [j [Hzs_j Hst_j]].
+              exists j.
+              split.
+              - (* from static_getType to nth_error sΓ' *)
+                unfold static_getType in Hst_j; exact Hst_j.
+              - (* keep the zs fact *)
+                exact Hzs_j.
+            }
+            destruct HargtypeFromsEnv as [iArgInSenv [HargtypeFromsEnv Hzs_iArg]].
+
+            assert (Hi'dom : iArgInSenv < dom sΓ).
+            {
+              apply nth_error_Some.
+              rewrite HargtypeFromsEnv; discriminate.
+            }
+            assert (HargtypeFromrEnv :
+                      nth_error (vars rΓ) iArgInSenv = Some (Iot loc)).
+            {
+              destruct (runtime_lookup_list_nth_zs rΓ zs vals i' (Iot loc) H4 Hval_i)
+                as [j [Hzs_j Hget_j]].
+              assert (HiEq : iArgInSenv = j).
+              {
+                (* zs[i'] = Some iArgInSenv and zs[i'] = Some j ⇒ iArgInSenv = j *)
+                rewrite Hzs_iArg in Hzs_j.
+                inversion Hzs_j; reflexivity.
+              }
+              subst iArgInSenv.
+              unfold runtime_getVal in Hget_j.
+              exact Hget_j.
+            }
+            have Hcorrcopy_2 := Hcorrcopy.
+            specialize (Hcorrcopy lOutterReceiver OutterReceiverMutability HOutterReceiverAddr HOutterReceiverMutabilityType iArgInSenv Hi'dom argtype HargtypeFromsEnv).
+            unfold runtime_getVal in Hcorrcopy.
+            rewrite HargtypeFromrEnv in Hcorrcopy.
+            unfold wf_r_typable in Hcorrcopy.
+            unfold r_type in Hcorrcopy.
+            rewrite Hargobjloc in Hcorrcopy.
+            destruct Hcorrcopy as [Harg_basesubtype Harg_qualifiertypability].
+            split.
+
+            (* base subtype *)
+            rewrite nth_error_cons_succ in Hnth.
+            rewrite Hmsigeq in Hnth.
+            eapply Forall2_nth_error in H20; eauto.
+            apply qualified_type_subtype_base_subtype in H20.
+            rewrite (vpa_mutabilty_tt_sctype Ty sqt) in H20.
+            eapply base_trans; eauto.
+
+            (* Qualifier Typability *)
+            rewrite Hmsigeq in Hnth.
+            eapply Forall2_nth_error in H20; eauto.
+            apply qualified_type_subtype_q_subtype in H20.
+            rewrite sq_vpa_tt_eq_qq in H20.
+            specialize (Hcorrcopy_2 lOutterReceiver OutterReceiverMutability HOutterReceiverAddr HOutterReceiverMutabilityType).
+            unfold wf_senv in Hsenv.
+            destruct Hsenv as [Hsenvdom _].
+            apply get_this_qualified_type_nth_error in H12.
+            specialize (Hcorrcopy_2 0 Hsenvdom Tthis H12).
+            rewrite <- Hvars in Hget_iot.
+            apply get_this_var_mapping_runtime_getVal in Hget_iot.
+            rewrite Hget_iot in Hcorrcopy_2.
+            unfold wf_r_typable in Hcorrcopy_2.
+            unfold r_type in Hcorrcopy_2.
+            destruct (runtime_getObj h iot) as [outterreceiverobj|] eqn:Houtterobj; [|easy].
+            destruct Hcorrcopy_2 as [_ HOutterReceiverQualifierTypablility].
+            assert (rqtype (rt_type outterreceiverobj) = OutterReceiverMutability).
+            {
+              clear - Houtterobj HOutterReceiverMutabilityType HOutterReceiverAddr Hget_iot Hvars.
+              rewrite <- Hvars in HOutterReceiverAddr.
+              apply get_this_var_mapping_runtime_getVal in HOutterReceiverAddr.
+              rewrite Hget_iot in HOutterReceiverAddr.
+              inversion HOutterReceiverAddr; subst lOutterReceiver.
+              unfold r_muttype in HOutterReceiverMutabilityType.
+              rewrite Houtterobj in HOutterReceiverMutabilityType.
+              simpl in HOutterReceiverMutabilityType.
+              inversion HOutterReceiverMutabilityType; reflexivity.
+            }
+            subst OutterReceiverMutability.
+            assert (ι = ly).
+            {
+              unfold get_this_var_mapping in HreceiverAddr.
+              rewrite HeqrΓmethodinit in HreceiverAddr.
+              simpl in HreceiverAddr.
+              inversion HreceiverAddr; reflexivity.
+            }
+            subst ι.
+            assert(rq_obj = qinner).
+            {
+              unfold r_muttype in Hqcontext.
+              rewrite Hobjy in Hqcontext.
+              simpl in Hqcontext.
+              inversion Hqcontext.
+              easy.
+            }
+            subst rq_obj.
+            clear - H20 Harg_qualifiertypability HyQualifierTypablility HOutterReceiverQualifierTypablility.
+
+            destruct (rqtype (rt_type argobj)) eqn:Hargobjmutability; move Hargobjmutability at bottom;
+            destruct (sqtype sqt) eqn:HParameterStaticDeclearedMutability; move HParameterStaticDeclearedMutability at bottom;
+            destruct qinner eqn:HInnerReceiverMutability; move HInnerReceiverMutability at bottom;
+            try solve_qualifier_typable_correct_concrete.
+
+            all: destruct (sqtype Ty) eqn:HTyStaticMutability;
+            destruct (sqtype argtype) eqn:HArgTypeStaticMutability;
+            simpl in H20;
+            try solve_q_subtype_wrong.
+
+            all: 
+            destruct (rqtype (rt_type outterreceiverobj)) eqn:HOutterReceiverMutability;
+            try solve_qualifier_typable_wrong_concrete.
+
+          - (* Parameter i' doesn't exist - contradiction *)
+            exfalso.
+            apply nth_error_None in Hval_i.
+            apply runtime_lookup_list_preserves_length in H4.
+            apply static_getType_list_preserves_length in H11.
+            apply Forall2_length in H20.
+            rewrite H4 in Hval_i.
+            rewrite <- H11 in Hval_i.
+            rewrite H20 in Hval_i.
+            simpl in Hi.
+            simpl in Hnth.
+            rewrite <- Hmsigeq in Hval_i.
+            lia.
+    }
+    specialize (IHHeval Hlocalset Hassignability vals' Hobj' vals0 Hobj sΓmethodend sΓmethodinit).
+    assert (HenvInvariant: env_respects_protected_set (protected_locset CT h l_root)
+    sΓmethodinit rΓmethodinit).
+    {
+      unfold env_respects_protected_set.
+      intros z l_z Tz Hlookup_s Hlookup_r Hin_P.
+      rewrite HeqsΓmethodinit in Hlookup_s.
+      rewrite HeqrΓmethodinit in Hlookup_r.
+      unfold static_getType in Hlookup_s.
+      unfold runtime_getVal in Hlookup_r.
+      simpl in Hlookup_s, Hlookup_r.
+      destruct z as [| z'].
+      - simpl in Hlookup_s, Hlookup_r.
+      injection Hlookup_s as <-. injection Hlookup_r as <-.
+      unfold is_safe_mode.
+      have Hty_safe : is_safe_mode (sqtype Ty).
+      {
+        unfold env_respects_protected_set in Henv_respects.
+        specialize (Henv_respects y ly Ty H10 H Hin_P).
+        exact Henv_respects.
+      }
+      unfold is_safe_mode in Hty_safe.
+      unfold vpa_mutabilty_tt.
+      apply qualified_type_subtype_q_subtype in H19.
+      clear - Hty_safe H19.
+      unfold vpa_mutabilty_tt in H19.
+      destruct Hty_safe as [HRd | HLost].
+      + (* Case: sqtype Ty = Rd *)
+        rewrite HRd in H19.
+        simpl in H19.
+        inversion H19; easy.
+      + (* Case: sqtype Ty = Lost *)
+        rewrite HLost in H19.
+        simpl in H19.
+        inversion H19; easy.
+      -
+        assert (Hy_dom : y < dom sΓ).
+        {
+          apply static_getType_dom in H10.
+          exact H10.
+        }
+
+        unfold wf_renv in Hrenv.
+        destruct Hrenv as [_ [Hreceiver _]].
+        destruct Hreceiver as [iot [Hget_iot Hiot_dom]].
+        assert (HOutterReceiverMutability: exists qcontext, r_muttype h iot = Some qcontext).
+        {
+          eapply receiver_mutability_exists_from_bound; eauto.
+        }
+        destruct HOutterReceiverMutability as [qoutter Hqoutter].
+        (* Apply correspondence to get wf_r_typable *)
+        specialize (Htypable iot qoutter Hget_iot Hqoutter y Hy_dom Ty H10).
+        unfold wf_r_typable in Htypable.
+        unfold r_basetype in H1.
+        unfold r_type.
+        destruct (runtime_getObj h ly) as [obj|] eqn:Hobjy.
+        2:{
+          unfold r_basetype in H0.
+          rewrite Hobjy in H0.
+          discriminate.
+        }
+        destruct obj as [rt_obj fields_obj].
+        destruct rt_obj as [rq_obj rc_obj].
+
+        unfold r_type in Htypable.
+        rewrite H in Htypable.
+        rewrite Hobjy in Htypable.
+        simpl in Htypable.
+        destruct Htypable as [Hsubtype Hqualifier].
+        simpl in Hobjy.
+
+        simpl in H1.
+        inversion H1.
+        assert (Hrc_obj_eq: rc_obj = cy).
+        {
+          unfold r_basetype in H0.
+          rewrite Hobjy in H0.
+          inversion H0.
+          easy.
+        }
+        subst rc_obj.
+        assert (Hsigeq: msignature mdef = msignature mdef0).
+        {
+          eapply method_signature_consistent_subtype; eauto.
+        }
+        have Hnth_param_type : nth_error (mparams (msignature mdef)) z' = Some Tz.
+        {
+          simpl in Hlookup_s.
+          easy.
+        }
+
+        have Hnth_param_val : nth_error vals z' = Some (Iot l_z).
+        {
+          simpl in Hlookup_r.
+          easy.
+        }
+        assert (Hi'_bound : z' < List.length argtypes).
+        {
+          apply Forall2_length in H20.
+          rewrite <- Hsigeq in H20.
+          assert (H_bound_params : z' < dom (mparams (msignature mdef))).
+          {
+            apply nth_error_Some. (* Converts "index < len" to "lookup <> None" *)
+            rewrite Hnth_param_type.   (* lookup is Some Tz *)
+            discriminate.         (* Some <> None *)
+          }
+
+          (* 2. Convert to bound for argtypes using the equality *)
+          rewrite <- H20 in H_bound_params. (* Replace length of params with length of argtypes *)
+
+          (* 3. Solve the goal *)
+          exact H_bound_params.
+        }
+
+        have Hnth_arg: exists T_arg, nth_error argtypes z' = Some T_arg.
+        {
+          apply nth_error_Some_exists.
+          exact Hi'_bound.
+        }
+
+        destruct Hnth_arg as [T_arg Hnth_arg].
+        eapply Forall2_nth_error with (i := z') (a := T_arg) (b := Tz) in H20; [|auto|rewrite <- Hsigeq; exact Hnth_param_type].
+        (* apply qualified_type_subtype_q_subtype in H20. *)
+        unfold env_respects_protected_set in Henv_respects.
+        apply adapated_subtype_safe_implies_safe in H20; auto.
+
+        have HargtypeFromsEnv :
+          exists z_outter,
+            static_getType sΓ z_outter = Some T_arg /\
+            nth_error zs z' = Some z_outter.
+        {
+          destruct (static_getType_list_nth_zs sΓ zs argtypes z' T_arg H11 Hnth_arg)
+            as [j [Hzs_j Hst_j]].
+          exists j.
+          split.
+          - unfold static_getType. exact Hst_j.
+          - exact Hzs_j.
+        }
+
+        destruct HargtypeFromsEnv as [z_outter [HgetZ_type Hzs_z_outter]].
+
+        have HgetZ_val : runtime_getVal rΓ z_outter = Some (Iot l_z).
+        {
+          destruct (runtime_lookup_list_nth_zs rΓ zs vals z' (Iot l_z) H4 Hnth_param_val)
+            as [j [Hzs_j Hget_j]].
+          assert (HzEq : z_outter = j) by (
+            rewrite Hzs_z_outter in Hzs_j;
+            inversion Hzs_j; reflexivity
+          ).
+          subst j.
+          exact Hget_j.
+        }
+        specialize (Henv_respects z_outter l_z T_arg HgetZ_type HgetZ_val Hin_P); auto.
+    }
+    assert (HMethodInnerInvariant: env_respects_protected_set (protected_locset CT h l_root)
+    sΓmethodinit rΓmethodinit /\ heap_respects_protected_set (protected_locset CT h l_root) h h CT).
+    {
+      split.
+      exact HenvInvariant.
+      exact Hheap_respects.
+    }
+    specialize (IHHeval HMethodInnerInvariant Hwf_method_frame).
+    rewrite <- getmbody in Hmethodbody_typing.
+    specialize (IHHeval Hmethodbody_typing); auto.
+    +
+    assert (Hwfmethod: exists D ddef, base_subtype CT cy D /\ find_class CT D = Some ddef /\ In mdef (methods (body ddef)) /\ wf_method CT D mdef).
+    {
+      eapply method_lookup_in_wellformed_inherited; eauto.
+      eapply r_basetype_in_dom; eauto.
+    }
+    destruct Hwfmethod as [D Hwfmethod].
+    destruct Hwfmethod as [ddef Hwfmethod].
+    destruct Hwfmethod as [Hbasecyd [HfindD [HmdefinD Hwfmethod]]].
+
+    unfold wf_method in Hwfmethod;
+    destruct Hwfmethod as [sΓmethodend [mbodyreturntype [Hmethodbody_typing [HmethodReturnBound [HmethodReturnType [HmethodReturnSubtype HMethodoverride]]]]]];
+    remember (mreceiver (msignature mdef) :: mparams (msignature mdef)) as sΓmethodinit;
+    remember {| vars := Iot ly :: vals |} as rΓmethodinit;
+    remember (rΓ <| vars := update x retval (vars rΓ) |>) as rΓ'''.
+    assert(Hwf_method_frame : wf_r_config CT sΓmethodinit rΓmethodinit h).
+    {
+      (* Method inner config wellformed.*)
+        have Hclass := Hclasstable.
+        unfold  wf_class_table in Hclass.
+        destruct Hclass as [Hclass [Hobjexist [Hotherclasses Hcname_consistent]]].
+        repeat split.
+        exact Hclass.
+        exact Hobjexist.
+        exact Hotherclasses.
+        apply Hcname_consistent.
+        apply Hcname_consistent.
+        exact Hheap.
+        rewrite HeqrΓmethodinit.
+        simpl.
+        lia.
+        unfold wf_renv in Hrenv.
+        destruct Hrenv as [HrEnvLen [Hreceiverval Hallvals]].
+        exists ly.
+        split.
+        rewrite HeqrΓmethodinit.
+        simpl.
+        reflexivity.
+        unfold runtime_getVal in H.
+        destruct (nth_error (vars rΓ) y) as [v|] eqn:Hnth_y; [|discriminate].
+        injection H as H1_eq.
+        subst v.
+        eapply Forall_nth_error in Hallvals; eauto.
+        simpl in Hallvals.
+        destruct (runtime_getObj h ly) as [obj|] eqn:Hobjly; [|contradiction].
+        apply runtime_getObj_dom in Hobjly.
+        exact Hobjly.
+
+        (* Inner runtime env is wellformed *)
+        rewrite HeqrΓmethodinit.
+        simpl.
+        constructor.
+        simpl.
+        unfold runtime_getVal in H.
+        destruct (nth_error (vars rΓ) y) as [v|] eqn:Hnth_y; [|discriminate].
+        injection H as H1_eq.
+        subst v.
+        unfold runtime_getVal in Hnth_y.
+        unfold wf_renv in Hrenv.
+        destruct Hrenv as [_ [_ Hallvals]].
+        eapply Forall_nth_error in Hallvals; eauto.
+        simpl in Hallvals.
+        exact Hallvals.
+        eapply runtime_lookup_list_preserves_wf_values with (zs:= zs) (vals0:=vals); eauto.
+
+        (* Inner Static Environment's length is more than 0 *)
+        rewrite HeqsΓmethodinit.
+        simpl.
+        lia.
+
+        (* Inner static env's elements are wellformed typeuse *)
+        rewrite HeqsΓmethodinit.
+        constructor.
+
+        (* Receiver type is well-formed *)
+        eapply method_sig_wf_receiver_by_find; eauto.
+        (* assert (Hcydom: cy < dom CT). {
+            eapply find_class_dom; eauto.
+        }
+        exact Hcydom. *)
+        assert (Hparentdom: parent < dom CT). {
+          assert (cy < dom CT). {
+            eapply find_class_dom; eauto.
+          }
+          assert (parent < cy). {
+            eapply parent_implies_strict_ordering with (C:= cy) (D:=parent); eauto.
+          }
+          lia.
+        }
+        exact Hparentdom. 
+        eapply method_sig_wf_parameters_by_find; eauto.
+        assert (Hparentdom: parent < dom CT). {
+          assert (cy < dom CT). {
+            eapply find_class_dom; eauto.
+          }
+          assert (parent < cy). {
+            eapply parent_implies_strict_ordering with (C:= cy) (D:=parent); eauto.
+          }
+          lia.
+        }
+        exact Hparentdom. 
+        apply static_getType_list_preserves_length in H11.
+        apply runtime_lookup_list_preserves_length in H4.
+        rewrite HeqsΓmethodinit.
+        rewrite HeqrΓmethodinit.
+        simpl.
+        f_equal.
+        apply Forall2_length in H20.
+        assert (Hy_dom : y < dom sΓ).
+        {
+          apply static_getType_dom in H10.
+          exact H10.
+        }
+        assert (HOutterReceiverAddr: exists lOutterReceiver, get_this_var_mapping (vars rΓ) = Some lOutterReceiver).
+        {
+          eapply get_this_exists_from_wf_r_config; eauto.
+
+        }
+        destruct HOutterReceiverAddr as [lOutterReceiver HOutterReceiverAddr].
+        assert (HOutterReceiverMutability: exists qcontext, r_muttype h lOutterReceiver = Some qcontext).
+        {
+          eapply receiver_mutability_exists_wf_renv; eauto.
+        }
+        destruct HOutterReceiverMutability as [OutterReceiverMutability HOutterReceiverMutabilityType].
+        have Hcorr := Htypable.
+        have Hcorrcopy := Hcorr.
+        specialize (Hcorr lOutterReceiver OutterReceiverMutability HOutterReceiverAddr HOutterReceiverMutabilityType y Hy_dom Ty H10).
+        unfold wf_r_typable in Hcorr.
+        unfold r_basetype in H0.
+        unfold r_type.
+        destruct (runtime_getObj h ly) as [obj|] eqn:Hobjy; [|discriminate].
+        injection H0 as Hcy_eq.
+        subst cy.
+        destruct obj as [rt_obj fields_obj].
+        destruct rt_obj as [rq_obj rc_obj].
+
+        unfold wf_renv in Hrenv.
+        destruct Hrenv as [_ [Hreceiver _]].
+        destruct Hreceiver as [iot [Hget_iot _]].
+        unfold get_this_var_mapping.
+        unfold gget in Hget_iot.
+        destruct (vars rΓ) as [|v0 vs] eqn:Hvars; [discriminate|].
+
+        unfold r_type in Hcorr.
+        rewrite H in Hcorr.
+        rewrite Hobjy in Hcorr.
+        simpl in Hcorr.
+        destruct Hcorr as [Hbasesubtype HyQualifierTypablility].
+        assert (msignature mdef = msignature mdef0).
+        {
+          eapply method_signature_consistent_subtype; eauto.
+        }
+        rewrite H0.
+        rewrite H4.
+        rewrite <- H20.
+        exact H11.
+
+        (* Correspondence holds for inner environment *)
+        intros ι qinner HreceiverAddr Hqcontext i Hi sqt Hnth.
+        rewrite HeqsΓmethodinit in Hnth, Hi.
+        rewrite HeqrΓmethodinit.
+        simpl in *.
+        assert (Hy_dom : y < dom sΓ).
+        {
+          apply static_getType_dom in H10.
+          exact H10.
+        }
+        assert (HOutterReceiverAddr: exists lOutterReceiver, get_this_var_mapping (vars rΓ) = Some lOutterReceiver).
+        {
+          eapply get_this_exists_from_wf_r_config; eauto.
+        }
+        destruct HOutterReceiverAddr as [lOutterReceiver HOutterReceiverAddr].
+        assert (HOutterReceiverMutability: exists qcontext, r_muttype h lOutterReceiver = Some qcontext).
+        {
+          eapply receiver_mutability_exists_wf_renv; eauto.
+        }
+        destruct HOutterReceiverMutability as [OutterReceiverMutability HOutterReceiverMutabilityType].
+        have Hcorr := Htypable.
+        have Hcorrcopy := Hcorr.
+        specialize (Hcorr lOutterReceiver OutterReceiverMutability HOutterReceiverAddr HOutterReceiverMutabilityType y Hy_dom Ty H10).
+        unfold wf_r_typable in Hcorr.
+        unfold r_basetype in H0.
+        unfold r_type.
+        destruct (runtime_getObj h ly) as [obj|] eqn:Hobjy; [|discriminate].
+        injection H0 as Hcy_eq.
+        subst cy.
+        destruct obj as [rt_obj fields_obj].
+        destruct rt_obj as [rq_obj rc_obj].
+
+        have Hrenvcopy := Hrenv.
+        unfold wf_renv in Hrenv.
+        destruct Hrenv as [_ [Hreceiver _]].
+        destruct Hreceiver as [iot [Hget_iot _]].
+        unfold get_this_var_mapping.
+        unfold gget in Hget_iot.
+        destruct (vars rΓ) as [|v0 vs] eqn:Hvars; [discriminate|].
+
+        unfold r_type in Hcorr.
+        rewrite H in Hcorr.
+        rewrite Hobjy in Hcorr.
+        simpl in Hcorr.
+        destruct Hcorr as [Hbasesubtype HyQualifierTypablility].
+        
+        assert (Hmsigeq: msignature mdef = msignature mdef0).
+        {
+          eapply method_signature_consistent_subtype; eauto.
+        }
+        destruct i as [|i'].
+
+        (* Reciever index - 0 *)
+        simpl in Hnth.
+        injection Hnth as Hsqt_eq.
+        subst sqt.
+        simpl.
+        unfold wf_r_typable.
+        unfold r_type.
+
+        rewrite Hobjy.
+        simpl.
+        split.
+
+        (* Base type subtyping *)
+        rewrite Hmsigeq.
+        apply qualified_type_subtype_base_subtype in H19.
+        (* rewrite (vpa_mutabilty_tt_sctype Tthis Ty) in H23. *)
+        rewrite (vpa_mutabilty_tt_sctype Ty (mreceiver (msignature mdef0))) in H19.
+        eapply base_trans; eauto.
+
+        (* Qualifier typbility *)
+        1: 
+        {
+          apply qualified_type_subtype_q_subtype in H19.
+          specialize (Hcorrcopy lOutterReceiver OutterReceiverMutability HOutterReceiverAddr HOutterReceiverMutabilityType).
+          apply get_this_qualified_type_nth_error in H12.
+          unfold wf_senv in Hsenv.
+          destruct Hsenv as [Hsenvdom _].
+          specialize (Hcorrcopy 0 Hsenvdom Tthis H12).
+          rewrite <- Hvars in HOutterReceiverAddr.
+          apply get_this_var_mapping_runtime_getVal in HOutterReceiverAddr.
+          rewrite HOutterReceiverAddr in Hcorrcopy.
+          unfold wf_r_typable in Hcorrcopy.
+          unfold r_type in Hcorrcopy.
+          destruct (runtime_getObj h lOutterReceiver) as [outterreceiverobj|] eqn:Houtterobj; [|easy].
+          destruct Hcorrcopy as [_ Houtter_qualifier_typable].
+
+          assert (rqtype (rt_type outterreceiverobj) = OutterReceiverMutability).
+          {
+            unfold r_muttype in HOutterReceiverMutabilityType.
+            rewrite Houtterobj in HOutterReceiverMutabilityType.
+            simpl in HOutterReceiverMutabilityType.
+            inversion HOutterReceiverMutabilityType; subst OutterReceiverMutability.
+            reflexivity.
+          }
+          subst OutterReceiverMutability.
+
+          assert (ly = ι). 
+          {
+            rewrite HeqrΓmethodinit in HreceiverAddr.
+            unfold get_this_var_mapping in HreceiverAddr.
+            simpl in HreceiverAddr.
+            inversion HreceiverAddr; reflexivity.
+          }
+          subst ι.
+
+          assert (r_muttype h ly = Some rq_obj).
+          {
+            unfold r_muttype.
+            rewrite Hobjy.
+            simpl.
+            reflexivity.
+          }
+
+          assert (rq_obj = qinner).
+          {
+            rewrite H0 in Hqcontext.
+            inversion Hqcontext; subst qinner.
+            reflexivity.
+          }
+          subst rq_obj.
+
+          unfold qualifier_typable_context.
+          unfold qualifier_typable_context in HyQualifierTypablility.
+          unfold qualifier_typable_context in Houtter_qualifier_typable.
+          unfold vpa_mutabilty_rs.
+          unfold vpa_mutabilty_rs in HyQualifierTypablility.
+          unfold vpa_mutabilty_rs in Houtter_qualifier_typable.
+          unfold vpa_mutabilty_tt in H19.
+          rewrite <- Hmsigeq in H19.
+
+          destruct qinner eqn:HInnerReceiverMutability;
+          destruct (sqtype (mreceiver (msignature mdef))) eqn:HMethodReceiverDeclaredType;
+          try trivial.
+          all: destruct (rqtype (rt_type outterreceiverobj)) eqn:HOutterReceiverMutability;
+          destruct (sqtype Ty) eqn:HTyStaticMutability;
+          try trivial.
+          all: destruct (sqtype Tthis) eqn:HTthisStaticMutability;
+          try rewrite HTyStaticMutability in H19;
+          simpl in H19;
+          try rewrite HMethodReceiverDeclaredType in H19;
+          try inversion H19; try trivial.
+          all: try inversion H19; try easy.
+        }
+        (* clear_dups. amazing.... *)
+
+  (* -------------------------------------------------- *)
+  (* Other index - > 1 *)
+        apply qualified_type_subtype_q_subtype in H18.
+        unfold runtime_getVal.
+        simpl.
+        destruct (nth_error vals i') as [v|] eqn:Hval_i.
+          - (* Parameter i' exists *)
+            destruct v as [|loc]; [trivial|].
+            (* Use H23 to get the subtyping relationship *)
+            assert (Hi'_bound : i' < List.length argtypes).
+            {
+              apply Forall2_length in H20.
+              simpl in Hi.
+              simpl in Hnth.
+              rewrite Hmsigeq in Hnth.
+              rewrite H20.
+              apply nth_error_Some.
+              intros Hnone.
+              rewrite Hnth in Hnone.
+              discriminate.
+            }
+            assert (Harg_type : exists argtype, nth_error argtypes i' = Some argtype).
+            {
+              apply nth_error_Some_exists.
+              exact Hi'_bound.
+            }
+            assert (loc < dom h).
+            {
+              assert (Hvals_wf :
+              Forall
+                (fun v =>
+                  match v with
+                  | Null_a => True
+                  | Iot loc =>
+                      match runtime_getObj h loc with
+                      | Some _ => True
+                      | None => False
+                      end
+                  end) vals).
+              {
+                eapply runtime_lookup_list_preserves_wf_values; eauto.
+              }
+              eapply Forall_nth_error in Hvals_wf; eauto.
+              simpl in Hvals_wf.
+              destruct (runtime_getObj h loc) as [argobj|] eqn:Hargobjloc; [|contradiction].
+              apply runtime_getObj_dom in Hargobjloc.
+              exact Hargobjloc.
+            }
+            destruct Harg_type as [argtype Hargtype].
+            unfold wf_r_typable.
+            unfold r_type.
+            destruct (runtime_getObj h loc) as [argobj|] eqn:Hargobjloc; [|apply runtime_getObj_not_dom in Hargobjloc; lia].
+            assert (HargtypeFromsEnv :
+              exists iArgInSenv,
+                nth_error sΓ iArgInSenv = Some argtype
+            /\ nth_error zs i' = Some iArgInSenv).
+            {
+              destruct (static_getType_list_nth_zs sΓ zs argtypes i' argtype H11 Hargtype)
+                as [j [Hzs_j Hst_j]].
+              exists j.
+              split.
+              - (* from static_getType to nth_error sΓ' *)
+                unfold static_getType in Hst_j; exact Hst_j.
+              - (* keep the zs fact *)
+                exact Hzs_j.
+            }
+            destruct HargtypeFromsEnv as [iArgInSenv [HargtypeFromsEnv Hzs_iArg]].
+
+            assert (Hi'dom : iArgInSenv < dom sΓ).
+            {
+              apply nth_error_Some.
+              rewrite HargtypeFromsEnv; discriminate.
+            }
+            assert (HargtypeFromrEnv :
+                      nth_error (vars rΓ) iArgInSenv = Some (Iot loc)).
+            {
+              destruct (runtime_lookup_list_nth_zs rΓ zs vals i' (Iot loc) H4 Hval_i)
+                as [j [Hzs_j Hget_j]].
+              assert (HiEq : iArgInSenv = j).
+              {
+                (* zs[i'] = Some iArgInSenv and zs[i'] = Some j ⇒ iArgInSenv = j *)
+                rewrite Hzs_iArg in Hzs_j.
+                inversion Hzs_j; reflexivity.
+              }
+              subst iArgInSenv.
+              unfold runtime_getVal in Hget_j.
+              exact Hget_j.
+            }
+            have Hcorrcopy_2 := Hcorrcopy.
+            specialize (Hcorrcopy lOutterReceiver OutterReceiverMutability HOutterReceiverAddr HOutterReceiverMutabilityType iArgInSenv Hi'dom argtype HargtypeFromsEnv).
+            unfold runtime_getVal in Hcorrcopy.
+            rewrite HargtypeFromrEnv in Hcorrcopy.
+            unfold wf_r_typable in Hcorrcopy.
+            unfold r_type in Hcorrcopy.
+            rewrite Hargobjloc in Hcorrcopy.
+            destruct Hcorrcopy as [Harg_basesubtype Harg_qualifiertypability].
+            split.
+
+            (* base subtype *)
+            rewrite nth_error_cons_succ in Hnth.
+            rewrite Hmsigeq in Hnth.
+            eapply Forall2_nth_error in H20; eauto.
+            apply qualified_type_subtype_base_subtype in H20.
+            rewrite (vpa_mutabilty_tt_sctype Ty sqt) in H20.
+            eapply base_trans; eauto.
+
+            (* Qualifier Typability *)
+            rewrite Hmsigeq in Hnth.
+            eapply Forall2_nth_error in H20; eauto.
+            apply qualified_type_subtype_q_subtype in H20.
+            rewrite sq_vpa_tt_eq_qq in H20.
+            specialize (Hcorrcopy_2 lOutterReceiver OutterReceiverMutability HOutterReceiverAddr HOutterReceiverMutabilityType).
+            unfold wf_senv in Hsenv.
+            destruct Hsenv as [Hsenvdom _].
+            apply get_this_qualified_type_nth_error in H12.
+            specialize (Hcorrcopy_2 0 Hsenvdom Tthis H12).
+            rewrite <- Hvars in Hget_iot.
+            apply get_this_var_mapping_runtime_getVal in Hget_iot.
+            rewrite Hget_iot in Hcorrcopy_2.
+            unfold wf_r_typable in Hcorrcopy_2.
+            unfold r_type in Hcorrcopy_2.
+            destruct (runtime_getObj h iot) as [outterreceiverobj|] eqn:Houtterobj; [|easy].
+            destruct Hcorrcopy_2 as [_ HOutterReceiverQualifierTypablility].
+            assert (rqtype (rt_type outterreceiverobj) = OutterReceiverMutability).
+            {
+              clear - Houtterobj HOutterReceiverMutabilityType HOutterReceiverAddr Hget_iot Hvars.
+              rewrite <- Hvars in HOutterReceiverAddr.
+              apply get_this_var_mapping_runtime_getVal in HOutterReceiverAddr.
+              rewrite Hget_iot in HOutterReceiverAddr.
+              inversion HOutterReceiverAddr; subst lOutterReceiver.
+              unfold r_muttype in HOutterReceiverMutabilityType.
+              rewrite Houtterobj in HOutterReceiverMutabilityType.
+              simpl in HOutterReceiverMutabilityType.
+              inversion HOutterReceiverMutabilityType; reflexivity.
+            }
+            subst OutterReceiverMutability.
+            assert (ι = ly).
+            {
+              unfold get_this_var_mapping in HreceiverAddr.
+              rewrite HeqrΓmethodinit in HreceiverAddr.
+              simpl in HreceiverAddr.
+              inversion HreceiverAddr; reflexivity.
+            }
+            subst ι.
+            assert(rq_obj = qinner).
+            {
+              unfold r_muttype in Hqcontext.
+              rewrite Hobjy in Hqcontext.
+              simpl in Hqcontext.
+              inversion Hqcontext.
+              easy.
+            }
+            subst rq_obj.
+            clear - H20 Harg_qualifiertypability HyQualifierTypablility HOutterReceiverQualifierTypablility.
+
+            destruct (rqtype (rt_type argobj)) eqn:Hargobjmutability; move Hargobjmutability at bottom;
+            destruct (sqtype sqt) eqn:HParameterStaticDeclearedMutability; move HParameterStaticDeclearedMutability at bottom;
+            destruct qinner eqn:HInnerReceiverMutability; move HInnerReceiverMutability at bottom;
+            try solve_qualifier_typable_correct_concrete.
+
+            all: destruct (sqtype Ty) eqn:HTyStaticMutability;
+            destruct (sqtype argtype) eqn:HArgTypeStaticMutability;
+            simpl in H20;
+            try solve_q_subtype_wrong.
+
+            all: 
+            destruct (rqtype (rt_type outterreceiverobj)) eqn:HOutterReceiverMutability;
+            try solve_qualifier_typable_wrong_concrete.
+
+          - (* Parameter i' doesn't exist - contradiction *)
+            exfalso.
+            apply nth_error_None in Hval_i.
+            apply runtime_lookup_list_preserves_length in H4.
+            apply static_getType_list_preserves_length in H11.
+            apply Forall2_length in H20.
+            rewrite H4 in Hval_i.
+            rewrite <- H11 in Hval_i.
+            rewrite H20 in Hval_i.
+            simpl in Hi.
+            simpl in Hnth.
+            rewrite <- Hmsigeq in Hval_i.
+            lia.
+    }
+    specialize (IHHeval Hlocalset Hassignability vals' Hobj' vals0 Hobj sΓmethodend sΓmethodinit).
+    assert (HenvInvariant: env_respects_protected_set (protected_locset CT h l_root)
+    sΓmethodinit rΓmethodinit).
+    {
+      unfold env_respects_protected_set.
+      intros z l_z Tz Hlookup_s Hlookup_r Hin_P.
+      rewrite HeqsΓmethodinit in Hlookup_s.
+      rewrite HeqrΓmethodinit in Hlookup_r.
+      unfold static_getType in Hlookup_s.
+      unfold runtime_getVal in Hlookup_r.
+      simpl in Hlookup_s, Hlookup_r.
+      destruct z as [| z'].
+      - simpl in Hlookup_s, Hlookup_r.
+      injection Hlookup_s as <-. injection Hlookup_r as <-.
+      unfold is_safe_mode.
+      have Hty_safe : is_safe_mode (sqtype Ty).
+      {
+        unfold env_respects_protected_set in Henv_respects.
+        specialize (Henv_respects y ly Ty H10 H Hin_P).
+        exact Henv_respects.
+      }
+      unfold is_safe_mode in Hty_safe.
+      unfold vpa_mutabilty_tt.
+      apply qualified_type_subtype_q_subtype in H19.
+      clear - Hty_safe H19.
+      unfold vpa_mutabilty_tt in H19.
+      destruct Hty_safe as [HRd | HLost].
+      + (* Case: sqtype Ty = Rd *)
+        rewrite HRd in H19.
+        simpl in H19.
+        inversion H19; easy.
+      + (* Case: sqtype Ty = Lost *)
+        rewrite HLost in H19.
+        simpl in H19.
+        inversion H19; easy.
+      -
+        assert (Hy_dom : y < dom sΓ).
+        {
+          apply static_getType_dom in H10.
+          exact H10.
+        }
+
+        unfold wf_renv in Hrenv.
+        destruct Hrenv as [_ [Hreceiver _]].
+        destruct Hreceiver as [iot [Hget_iot Hiot_dom]].
+        assert (HOutterReceiverMutability: exists qcontext, r_muttype h iot = Some qcontext).
+        {
+          eapply receiver_mutability_exists_from_bound; eauto.
+        }
+        destruct HOutterReceiverMutability as [qoutter Hqoutter].
+        (* Apply correspondence to get wf_r_typable *)
+        specialize (Htypable iot qoutter Hget_iot Hqoutter y Hy_dom Ty H10).
+        unfold wf_r_typable in Htypable.
+        unfold r_basetype in H1.
+        unfold r_type.
+        destruct (runtime_getObj h ly) as [obj|] eqn:Hobjy.
+        2:{
+          unfold r_basetype in H0.
+          rewrite Hobjy in H0.
+          discriminate.
+        }
+        destruct obj as [rt_obj fields_obj].
+        destruct rt_obj as [rq_obj rc_obj].
+
+        unfold r_type in Htypable.
+        rewrite H in Htypable.
+        rewrite Hobjy in Htypable.
+        simpl in Htypable.
+        destruct Htypable as [Hsubtype Hqualifier].
+        simpl in Hobjy.
+
+        simpl in H1.
+        inversion H1.
+        assert (Hrc_obj_eq: rc_obj = cy).
+        {
+          unfold r_basetype in H0.
+          rewrite Hobjy in H0.
+          inversion H0.
+          easy.
+        }
+        subst rc_obj.
+        assert (Hsigeq: msignature mdef = msignature mdef0).
+        {
+          eapply method_signature_consistent_subtype; eauto.
+        }
+        have Hnth_param_type : nth_error (mparams (msignature mdef)) z' = Some Tz.
+        {
+          simpl in Hlookup_s.
+          easy.
+        }
+
+        have Hnth_param_val : nth_error vals z' = Some (Iot l_z).
+        {
+          simpl in Hlookup_r.
+          easy.
+        }
+        assert (Hi'_bound : z' < List.length argtypes).
+        {
+          apply Forall2_length in H20.
+          rewrite <- Hsigeq in H20.
+          assert (H_bound_params : z' < dom (mparams (msignature mdef))).
+          {
+            apply nth_error_Some. (* Converts "index < len" to "lookup <> None" *)
+            rewrite Hnth_param_type.   (* lookup is Some Tz *)
+            discriminate.         (* Some <> None *)
+          }
+
+          (* 2. Convert to bound for argtypes using the equality *)
+          rewrite <- H20 in H_bound_params. (* Replace length of params with length of argtypes *)
+
+          (* 3. Solve the goal *)
+          exact H_bound_params.
+        }
+
+        have Hnth_arg: exists T_arg, nth_error argtypes z' = Some T_arg.
+        {
+          apply nth_error_Some_exists.
+          exact Hi'_bound.
+        }
+
+        destruct Hnth_arg as [T_arg Hnth_arg].
+        eapply Forall2_nth_error with (i := z') (a := T_arg) (b := Tz) in H20; [|auto|rewrite <- Hsigeq; exact Hnth_param_type].
+        (* apply qualified_type_subtype_q_subtype in H20. *)
+        unfold env_respects_protected_set in Henv_respects.
+        apply adapated_subtype_safe_implies_safe in H20; auto.
+
+        have HargtypeFromsEnv :
+          exists z_outter,
+            static_getType sΓ z_outter = Some T_arg /\
+            nth_error zs z' = Some z_outter.
+        {
+          destruct (static_getType_list_nth_zs sΓ zs argtypes z' T_arg H11 Hnth_arg)
+            as [j [Hzs_j Hst_j]].
+          exists j.
+          split.
+          - unfold static_getType. exact Hst_j.
+          - exact Hzs_j.
+        }
+
+        destruct HargtypeFromsEnv as [z_outter [HgetZ_type Hzs_z_outter]].
+
+        have HgetZ_val : runtime_getVal rΓ z_outter = Some (Iot l_z).
+        {
+          destruct (runtime_lookup_list_nth_zs rΓ zs vals z' (Iot l_z) H4 Hnth_param_val)
+            as [j [Hzs_j Hget_j]].
+          assert (HzEq : z_outter = j) by (
+            rewrite Hzs_z_outter in Hzs_j;
+            inversion Hzs_j; reflexivity
+          ).
+          subst j.
+          exact Hget_j.
+        }
+        specialize (Henv_respects z_outter l_z T_arg HgetZ_type HgetZ_val Hin_P); auto.
+    }
+    assert (HMethodInnerInvariant: env_respects_protected_set (protected_locset CT h l_root)
+    sΓmethodinit rΓmethodinit /\ heap_respects_protected_set (protected_locset CT h l_root) h h CT).
+    {
+      split.
+      exact HenvInvariant.
+      exact Hheap_respects.
+    }
+    specialize (IHHeval HMethodInnerInvariant Hwf_method_frame).
+    rewrite <- getmbody in Hmethodbody_typing.
+    specialize (IHHeval Hmethodbody_typing); auto.
+  - (* Seq *)
+    (* Invert typing for SSeq *)
+    inversion Htyping; subst.
+    rename sΓ' into  sΓ''.
+    rename sΓ'0 into sΓ'.
+    
+    (* Extract wellformedness for intermediate state using preservation_pico *)
+    have Hwf' : wf_r_config CT sΓ' rΓ' h'.
+    {
+      eapply preservation_pico; eauto.
+    }
+
+    assert (Heq_protected_set: protected_locset CT h l_root = protected_locset CT h' l_root /\ confinement_invariant_precise (protected_locset CT h l_root) CT sΓ' rΓ' h h').
+    {
+      eapply stmt_preserves_both; eauto.
+    }
+    destruct Heq_protected_set as [Heq_protected_set Hconfined_intermediate].
+
+    specialize (eval_stmt_preserves_heap_domain_simple CT rΓ h s1 rΓ' h' Heval1) as Hh'.
+    assert (Hdom_root': l_root < dom h') by lia.
+    assert (Hldomh': l < dom h') by (apply runtime_getObj_dom in Hobj; lia).
+    specialize (runtime_getObj_Some h' l Hldomh') as [T [values' Hh'some]].
+    specialize (runtime_preserves_r_type_heap CT rΓ h l ({| rqtype := anyrq; rctype := C |})
+    h' vals s1 rΓ' Hobj Heval1) as [vals1 Hrtype].
+    rewrite Hrtype in Hh'some; inversion Hh'some; subst.
+
+    specialize (IHHeval1 Hdom_root eq_refl Hlocalset Hassignability values' Hrtype vals Hobj sΓ' sΓ Hconfined Hwf H4).
+
+    have Hlocalset': Ensembles.In Loc (protected_locset CT h' l_root) l by (rewrite Heq_protected_set in Hlocalset; exact Hlocalset).
+    rewrite Heq_protected_set in Hconfined_intermediate.
+
+    assert (Hconf1_for_ih2 : confinement_invariant_precise (protected_locset CT h' l_root) CT sΓ' rΓ' h' h').
+    {
+      unfold confinement_invariant_precise in Hconfined_intermediate.
+      destruct Hconfined_intermediate as [Henv1 Hheap1].
+      split.
+      + exact Henv1.
+      + unfold heap_respects_protected_set in Hheap1.
+        intros l_src C0 anyrq0 vals0 k l_dst Hdom_src_h' Hlsrc_new Hin_dst Hobj0 Hnth.
+        (* l_dst < dom h' (from Hin_dst via reachable_abs_dom) *)
+        have Hdom_src_h : l_dst < dom h.
+        rewrite <- Heq_protected_set in Hin_dst.
+        have Hin_dst_copy := Hin_dst.
+        apply reachable_abs_dom in Hin_dst_copy.
+        exact Hin_dst_copy.
+        have hdom_src_h : l_src >= dom h by lia.
+        exact (Hheap1 l_src C0 anyrq0 vals0 k l_dst Hdom_src_h hdom_src_h Hin_dst Hobj0 Hnth).
+    }
+
+    specialize (IHHeval2 Hdom_root' eq_refl Hlocalset' Hassignability vals' Hobj' values' Hrtype sΓ'' sΓ' Hconf1_for_ih2 Hwf' H6).
+    rewrite IHHeval2 in IHHeval1; auto.
+Qed.
